@prefix :      <https://w3id.org/i40/sto#> .
@prefix schema: <http://schema.org/> .
@prefix owl:   <http://www.w3.org/2002/07/owl#> .
@prefix xsd:   <http://www.w3.org/2001/XMLSchema#> .
@prefix skos:  <http://www.w3.org/2004/02/skos/core#> .
@prefix rdfs:  <http://www.w3.org/2000/01/rdf-schema#> .
@prefix deo:   <http://purl.org/spar/deo/> .
@prefix geo:   <http://www.geonames.org/ontology#> .
@prefix muto:  <http://purl.org/muto/core#> .
@prefix om2:   <http://www.ontology-of-units-of-measure.org/resource/om-2/> .
@prefix doap:  <http://usefulinc.com/ns/doap#> .
@prefix xml:   <http://www.w3.org/XML/1998/namespace> .
@prefix dcterms: <http://purl.org/dc/terms/> .
@prefix vann:  <http://purl.org/vocab/vann/> .
@prefix prov:  <http://www.w3.org/ns/prov#> .
@prefix foaf:  <http://xmlns.com/foaf/0.1/> .
@prefix cc:    <http://creativecommons.org/ns#> .
@prefix obda:  <https://w3id.org/obda/vocabulary#> .
@prefix voaf:  <http://purl.org/vocommons/voaf#> .
@prefix sto:   <https://w3id.org/i40/sto#> .
@prefix dbo:   <http://dbpedia.org/ontology#> .
@prefix dc11:  <http://purl.org/dc/elements/1.1/> .
@prefix dbr:   <http://dbpedia.org/resource#> .
@prefix rdf:   <http://www.w3.org/1999/02/22-rdf-syntax-ns#> .
@prefix dul:   <http://www.ontologydesignpatterns.org/ont/dul/DUL.owl#> .
@prefix rami:  <https://w3id.org/i40/rami#> .

sto:hasImplementationFormat
        a             owl:DatatypeProperty ;
        rdfs:comment  "Describes the name of the implementation or serialization format of the Publication, e.g., XML, Document, binary, batch"@en ;
        rdfs:domain   sto:Publication ;
        rdfs:label    "has Implementation Format"@en ;
        rdfs:range    rdfs:Literal .

sto:IEC_PAS_63088  a             owl:NamedIndividual , sto:Standard ;
        rdfs:comment             "IEC PAS 63088:2017(E) describes a reference architecture model in the form of a cubic layer model, RAMI model"@en ;
        rdfs:label               "IEC PAS 63088"@en ;
        sto:hasOfficialResource  "https://webstore.iec.ch/publication/30082?lipi=urn%3Ali%3Apage%3Ad_flagship3_pulse_read%3B2vZf0%2FOGS2CeRjny8ARziQ%3D%3D" ;
        sto:hasPublicationDate   "2017-03-07"^^xsd:date ;
        sto:hasPublisher         sto:IEC , sto:ISO ;
        sto:hasTag               "RAMI 4.0" .

sto:IEC_60870_P5_S101_2003
        a                          sto:Standard , owl:NamedIndividual ;
        rdfs:comment               "IEC 60870-5-101:2003+A1:2015 Applies to telecontrol equipment and systems with coded bit serial data transmission for monitoring and controlling geographically widespread processes. Defines a telecontrol companion standard that enables interoperability among compatible telecontrol equipment. The defined telecontrol companion standard utilizes standards of the IEC 60870-5 series of documents. \nThis publication is of high relevance for Smart Grid. This consolidated version consists of the second edition (2003) and its amendment 1 (2015). Therefore, no need to order amendment in addition to this publication."@en ;
        rdfs:label                 "IEC 60870-5-101:2003"@en ;
        sto:hasAvailableLanguage   "English"@en ;
        sto:hasDBpediaResource     <https://dbpedia.org/resource/IEC_60870> , <null//dbpedia.org/resource/IEC_60870> ;
        sto:hasEdition             "2.1"^^xsd:float ;
        sto:hasFileSize            sto:FileSizeIEC_60870_P5_S101_2003 ;
        sto:hasICS                 sto:ICS_33_200 ;
        sto:hasOfficialResource    <https://webstore.iec.ch/publication/23822> , <null//webstore.iec.ch/publication/23822> ;
        sto:hasPages               "360"^^xsd:int ;
        sto:hasPublicationDate     "2015-11-330"^^xsd:date ;
        sto:hasPublisher           sto:IEC ;
        sto:hasStabilityDate       "2018"^^xsd:gYear ;
        sto:hasTag                 "IEC 60870-5-101:2003"@en ;
        sto:hasTechnicalCommittee  sto:TC_57 ;
        sto:hasTitle               "Telecontrol equipment and systems - Part 5-101: Transmissionprotocols - Companion standard for basic telecontrol tasks"@en ;
        sto:hasWikipediaArticle    <https://en.wikipedia.org/wiki/IEC_60870> , <null//en.wikipedia.org/wiki/IEC_60870> .

sto:Communication  a       owl:NamedIndividual , rami:AdminShellSubmodel ;
        sto:isDescribedin  sto:AdministrationShell .

skos:definition  a  owl:AnnotationProperty .

sto:ICS_33_200  a     sto:InternationalClassificationForStandards , owl:NamedIndividual ;
        rdfs:comment  "This is ICS for Telecontrol. Telemetering Including Supervising, Control and Data Acquisition System (SCADA)"@en , "This is ICS for “Telecontrol. Telemetering, including Supervising, Control and Data Acquisition System (SCADA)”"@en ;
        rdfs:label    "ICS 33.200"@en ;
        sto:hasTitle  "Telecontrol. Telemetering Including Supervising, Control and Data Acquisition System (SCADA)"@en , "Telecontrol. Telemetering , including Supervising, Control and Data Acquisition System (SCADA)"@en .

sto:IEC_60027_2006  a                owl:NamedIndividual , sto:Standard ;
        rdfs:comment                 "This part of IEC 60027 is applicable to control technology. It gives names and symbols for quantities, signals and functions, and their units."@en ;
        rdfs:label                   "IEC 60027-6:2006"@en ;
        sto:hasAvailableLanguage     "English/French, Spanish"@en ;
        sto:hasDBpediaResource       <http://dbpedia.org/page/IEC_60027> ;
        sto:hasEdition               "1.0"^^xsd:float ;
        sto:hasFileSize              sto:FileSizeIEC_60027_2006 ;
        sto:hasICS                   sto:ICS_01_060 ;
        sto:hasImplementationFormat  "Document"@en ;
        sto:hasOfficialResource      <https://webstore.iec.ch/publication/96> ;
        sto:hasPages                 29 ;
        sto:hasPublicationDate       "2006-12-14"^^xsd:date ;
        sto:hasPublisher             sto:IEC ;
        sto:hasStabilityDate         "2019"^^xsd:gYear ;
        sto:hasStatus                "Valid"@en ;
        sto:hasTag                   "IEC 60027:2006"@en ;
        sto:hasTechnicalCommittee    sto:TC_25 ;
        sto:hasTitle                 "Letter symbols to be used in electrical technology - Part 6: Control technology"@en ;
        sto:hasWikipediaArticle      <https://en.wikipedia.org/wiki/IEC_60027> .

sto:FileSizeIEC_60381_1978
        a                      owl:NamedIndividual , om2:Measure ;
        rdfs:comment           "Specifies the file size of the document for standard IEC 60381-2:1978"@en ;
        rdfs:label             "FileSize IEC 60381-2:1978"@en ;
        om2:hasNumericalValue  "483.0"^^xsd:float ;
        om2:hasUnit            om2:kilobyte .

sto:BusinessProcessExecution
        a                  owl:NamedIndividual , sto:BusinessCycleSCM ;
        rdfs:comment       "Describes Business Process Execution concept."@en ;
        rdfs:label         "Business Process Execution"@en ;
        sto:isDescribedin  sto:NISTInitiative .

sto:ISO_22745-11  a              sto:Standard , owl:NamedIndividual ;
        rdfs:comment             "ISO 22745-11:2010 provides guidelines that are recommended for the development of terminology for concepts in an open technical dictionary (OTD).Compliance with these guidelines is not required in order for a term or definition to be included in an OTD. These guidelines are provided as a framework for developers of industrial terminology to ensure that definitions are consistent and understandable. Terminology that complies with these guidelines will be marked as such in the OTD. This will allow a user to perform a search that filters terminology based on compliance with ISO 22745-11:2010."@en ;
        rdfs:label               "ISO 22745-11"@en ;
        sto:hasClassification    rami:Assest , sto:ProductCatalogData , rami:Product ;
        sto:hasDomain            sto:IndustrialAutomation ;
        sto:hasOfficialResource  "https://www.iso.org/standard/53999.html" ;
        sto:hasPublicationDate   "2010-02-01"^^xsd:date ;
        sto:hasPublisher         sto:ISO .

sto:IEC_60286_4_2013  a              sto:Standard , owl:NamedIndividual ;
        rdfs:comment                 "IEC 60286-4:2013 is applicable to stick magazines (including end stoppers) intended to be used for storage of electronic components, for transport from the manufacturer to the customer and for in-house use in the manufacturing plant. They are also used to feed automatic placement machines for surface mounting as well as for through-hole mounting of electronic components. This edition includes the following significant technical changes with respect to the previous edition: Clause 4 describes the guidelines for customer specific stick magazine design. It replaces the magazine design rules for IEC outlined components and rules for orientation of components in stick magazines which have been moved to Annexes A to D."@en ;
        rdfs:label                   "IEC 60286-3:2013"@en ;
        sto:hasAvailableLanguage     "English/French"@en ;
        sto:hasEdition               "3.0"^^xsd:float ;
        sto:hasFileSize              sto:FileSizeIEC_60286_4_2013 ;
        sto:hasICS                   sto:ICS_31_020 , sto:ICS_31_240 ;
        sto:hasImplementationFormat  "Document"@en ;
        sto:hasOfficialResource      <https://webstore.iec.ch/publication/1259> ;
        sto:hasPages                 32 ;
        sto:hasPublicationDate       "2013-07-26"^^xsd:date ;
        sto:hasPublisher             sto:IEC ;
        sto:hasStabilityDate         "2022"^^xsd:gYear ;
        sto:hasStatus                "Valid"@en ;
        sto:hasTag                   "IEC 60286-3:2013"@en ;
        sto:hasTechnicalCommittee    sto:TC_40 ;
        sto:hasTitle                 "Packaging of components for automatic handling - Part 4: Stick magazines for electronic components encapsulated in packages of different forms"@en .

sto:BPMN  a                      sto:Standard , owl:NamedIndividual ;
        rdfs:comment             "Business Process Model and Notation is a graphical representation for specifying business processes in a business process model."@en ;
        rdfs:label               "Business Process Model Notation"@en ;
        sto:hasClassification    sto:SCM ;
        sto:hasDBpediaResource   "http://dbpedia.org/page/Business_Process_Model_and_Notation" ;
        sto:hasDeveloper         sto:OMG ;
        sto:hasOfficialResource  "http://www.bpmn.org/" ;
        sto:hasTag               "BPMN"@en ;
        sto:hasWikipediaArticle  "https://en.wikipedia.org/wiki/Business_Process_Model_and_Notation" .

sto:ISO_15531  a                 owl:NamedIndividual , sto:Standard ;
        rdfs:comment             "This Standard models manufacturing management data such as, Resources management data (Resource model); Time related features (Time model); Flow management data in manufacturing (Flow management model)."@en ;
        rdfs:isDefinedBy         "https://www.researchgate.net/publication/220171079_ISO_15531_MANDATE_a_standardised_data_model_for_manufacturing_management" ;
        rdfs:label               "ISO 15531"@en ;
        sto:hasDomain            sto:IndustrialProcessMeasurementControl ;
        sto:hasOfficialResource  "https://www.iso.org/standard/28144.html" ;
        sto:hasPublisher         sto:ISO ;
        sto:hasTag               "MANDATE" .

sto:FileSizeIEC_61334_1996_P4_S32
        a                      om2:Measure , owl:NamedIndividual ;
        rdfs:comment           "Specifies the file size of the document for standard IEC 61334-4-32:1996 "@en ;
        rdfs:label             "FileSize IEC 61334-4-32:1996 "@en ;
        om2:hasNumericalValue  "869.0"^^xsd:float ;
        om2:hasUnit            om2:kilobyte .

sto:IndustrialProcessMeasurementControl
        a               owl:NamedIndividual , sto:Domain ;
        rdfs:comment    "Industrial process measurement and control"@en ;
        sto:domainName  "Industrial process measurement and control"@en .

sto:IEC_60839_P7_5  a              sto:Standard , owl:NamedIndividual ;
        rdfs:comment               "Specifies the requirements for standard interfaces using a two-wire connection employing ISO/IEC 8482 signalling for use between the control and indicating equipment of an alarm system and one or more alarm system transceivers connected to alarm transmission systems."@en ;
        rdfs:label                 "IEC 60839-7-5:2001"@en ;
        sto:hasAvailableLanguage   " English/French"@en , "English"@en ;
        sto:hasEdition             "1.0"^^xsd:float ;
        sto:hasFileSize            sto:FileSizeIEC_60839_P7_5 ;
        sto:hasICS                 sto:ICS_13_320 ;
        sto:hasOfficialResource    <null//webstore.iec.ch/publication/3673> ;
        sto:hasPages               "13"^^xsd:int ;
        sto:hasPublicationDate     "68/03/01"^^xsd:date ;
        sto:hasPublisher           sto:IEC ;
        sto:hasStabilityDate       "2018"^^xsd:gYear ;
        sto:hasTag                 "IEC 60839-7-5:2001"@en ;
        sto:hasTechnicalCommittee  sto:TC_79 ;
        sto:hasTitle               "Alarm systems - Part 7-5: Message formats and protocols for serial data interfaces in alarm transmission systems - Alarm system interfaces employing a two-wire configuration in accordance with ISO/IEC 8482"@en .

sto:IEC_62714  a                 owl:NamedIndividual , sto:Standard ;
        rdfs:comment             "Engineering data exchange format for use in industrial automation systems engineering - Automation markup language - Architecture and general requirements"@en ;
        rdfs:label               "IEC 62714"@en ;
        dcterms:hasLicense       "Open"@en ;
        sto:hasClassification    sto:ProductionSystemEngineering , rami:Information , rami:FieldDevice , rami:Engineering , rami:ControlDevice , rami:Product ;
        sto:hasDBpediaResource   "http://dbpedia.org/resource/AutomationML" ;
        sto:hasOfficialResource  "https://www.automationml.org/" ;
        sto:hasPublisher         sto:IEC ;
        sto:hasTag               "AML"@en , "AutomationML"@en ;
        sto:hasWikipediaArticle  "https://en.wikipedia.org/wiki/AutomationML" ;
        sto:relatedTo            sto:IEC_61360 , sto:eClass , sto:IEC_61987_X , sto:IEC_62541 ;
        sto:uses                 sto:MathML .

dbr:_Texas  a   owl:NamedIndividual .

dcterms:LicenseDocument
        a                 owl:Class ;
        rdfs:comment      "A legal document giving official permission to do something with a Resource."@en ;
        rdfs:isDefinedBy  dcterms: ;
        rdfs:label        "License Document"@en .

sto:FileSizeIEC_60839_P7_1
        a                      om2:Measure , owl:NamedIndividual ;
        rdfs:comment           "Specifies the file size of the document for standard IEC 60839-7-1:2001"@en ;
        rdfs:label             "FileSize IEC 60839-7-1:2001"@en ;
        om2:hasNumericalValue  "1137.0"^^xsd:float ;
        om2:hasUnit            om2:kilobyte .

sto:EndOfLifeReclying
        a       owl:NamedIndividual .

sto:hasPreviousVersion
        a                   owl:ObjectProperty ;
        rdfs:comment        "Indicates the list of Standards that are previous versions of a Standard. For example,IEC 60038:2009 has IEC 60038:1983+AMD1:1994+AMD2:1997,IEC 60038:1983/AMD2:1997,IEC 60038:1983/AMD1:1994,IEC 60038:1983,IEC 60038:1975/AMD1:1977,IEC 60038:1975,IEC 60038:1967,IEC 60038:1954,IEC 60038:1938,IEC 60038:1927 as previous versions."@en ;
        rdfs:label          "has Previous Version"@en ;
        rdfs:subPropertyOf  sto:relatedTo .

sto:FileSizeIEC_60050_1984
        a                      owl:NamedIndividual , om2:Measure ;
        rdfs:comment           "Specifies the file size of the document for standard IEC 60050-101:1998 "@en ;
        rdfs:label             "FileSize IEC 60050-371:1984"@en ;
        om2:hasNumericalValue  "2485.0"^^xsd:float ;
        om2:hasUnit            om2:kilobyte .

sto:TC_57  a          sto:TechnicalCommittee , owl:NamedIndividual ;
        rdfs:comment  "To prepare international standards for power systems control equipment and systems including EMS (Energy Management Systems), SCADA (Supervisory Control And Data Acquisition), distribution automation, teleprotection, and associated information exchange for real-time and non-real-time information, used in the planning, operation and maintenance of power systems. Power systems management comprises control within control centres, substations and individual pieces of primary equipment including telecontrol and interfaces to equipment, systems and databases, which may be outside the scope of TC 57.\n\nThe special conditions in a high voltage environment have to be taken into consideration.\nNote 1: Standards prepared by other technical committees of the IEC and organizations such as ITU and ISO shall be used where applicable.\nNote 2: Although the work of TC 57 is chiefly concerned with standards for electric power systems, these standards may also be useful for application by the relevant bodies to other geographical widespread processes.\nNote 3: Whereas standards related to measuring and protection relays and to the control and monitoring equipment used with these systems are treated by TC 95, TC 57 deals with the interface to the control systems and the transmission aspects for teleprotection systems. Whereas standards related to equipment for electrical measurement and load control are treated by TC 13, TC 57 deals with the interface of equipment for interconnection lines and industrial consumers and producers requiring energy management type interfaces to the control system."@en ;
        rdfs:label    "TC 57"@en ;
        sto:hasTitle  "Power systems management and associated information exchange"@en , "Power systems management and associated information exchange\n"@en .

rami:Other  a   owl:NamedIndividual .

sto:FileSizeIEC_60870_P5_S6_2006
        a                      om2:Measure , owl:NamedIndividual ;
        rdfs:comment           "Specifies the file size of the document for standard IEC 60870-5-6::2006."@en ;
        rdfs:label             "FileSize IEC 60870-5-6:2006"@en ;
        om2:hasNumericalValue  "1342.0"^^xsd:float ;
        om2:hasUnit            om2:kilobyte .

sto:ProductionLifeCycleDataManagement
        a                  owl:NamedIndividual , sto:ProductionSystemLifeCycle ;
        rdfs:comment       "Production lifecycle data management standards define general models of data integration, sharing, exchange, and hand-over for lifecycle support of production facilities."@en ;
        rdfs:label         "Production Life Cycle Data Management"@en ;
        sto:isDescribedin  sto:NISTInitiative .

sto:IEC_61334_P4_S511_2000
        a                          owl:NamedIndividual , sto:Standard ;
        rdfs:comment               "Specifies the data communication protocol (DCP) management requirements. Describes the management services in an abstract way as well as the underlying protocol.\nThis publication is of high relevance for Smart Grid."@en ;
        rdfs:label                 "IEC 61334-4-511:2000"@en ;
        sto:hasAvailableLanguage   "English/French"@en ;
        sto:hasDBpediaResource     <https://dbpedia.org/resource/IEC_61334> , <null//dbpedia.org/resource/IEC_61334> ;
        sto:hasEdition             "1.0"^^xsd:float ;
        sto:hasFileSize            sto:FileSizeIEC_61334_2000_P4_S511 ;
        sto:hasICS                 sto:ICS_33_040_40 , sto:ICS_33_200 ;
        sto:hasOfficialResource    <null//webstore.iec.ch/publication/5305> , <https://webstore.iec.ch/publication/5305> ;
        sto:hasPages               "65"^^xsd:int ;
        sto:hasPublicationDate     "2000-04-109"^^xsd:date ;
        sto:hasPublisher           sto:IEC ;
        sto:hasStabilityDate       "2018"^^xsd:gYear ;
        sto:hasTag                 "IEC 61334-4-511:2000"@en ;
        sto:hasTechnicalCommittee  sto:TC_57 ;
        sto:hasTitle               "Distribution automation using distribution line carrier systems - Part 4-511: Data communication protocols - Systems management - CIASE protocol"@en ;
        sto:hasWikipediaArticle    <null//en.wikipedia.org/wiki/IEC_61334> , <https://en.wikipedia.org/wiki/IEC_61334> .

sto:FileSizeIEC_60870_P6_S701_1998
        a                      om2:Measure , owl:NamedIndividual ;
        rdfs:comment           "Specifies the file size of the document for standard IEC 60870-6-701:1998"@en ;
        rdfs:label             "FileSize IEC 60870-6-701:1998"@en ;
        om2:hasNumericalValue  "130.0"^^xsd:float ;
        om2:hasUnit            om2:kilobyte .

sto:IEC_61334_P4_S41_1996
        a                          owl:NamedIndividual , sto:Standard ;
        rdfs:comment               "Defines the distribution line message specification (DLMS) within the OSI application layer.\nThis publication is of high relevance for Smart Grid."@en ;
        rdfs:label                 "IEC 61334-4-41:1996�"@en ;
        sto:hasAvailableLanguage   "English/French"@en ;
        sto:hasDBpediaResource     <null//dbpedia.org/resource/IEC_61334> , <https://dbpedia.org/resource/IEC_61334> ;
        sto:hasEdition             "1.0"^^xsd:float ;
        sto:hasFileSize            sto:FileSizeIEC_61334_1996_P4_S41 ;
        sto:hasICS                 sto:ICS_29_240_20 , sto:ICS_33_200 ;
        sto:hasOfficialResource    <null//webstore.iec.ch/publication/5303> , <https://webstore.iec.ch/publication/5303> ;
        sto:hasPages               "247"^^xsd:int ;
        sto:hasPublicationDate     "1996-08-13"^^xsd:date ;
        sto:hasPublisher           sto:IEC ;
        sto:hasStabilityDate       "2018"^^xsd:gYear ;
        sto:hasTag                 "IEC 61334-4-41:1996�"@en ;
        sto:hasTechnicalCommittee  sto:TC_57 ;
        sto:hasTitle               "Distribution automation using distribution line carrier systems - Part 4: Data communication protocols - Section 41: Application protocol - Distribution line message specification"@en ;
        sto:hasWikipediaArticle    <null//en.wikipedia.org/wiki/IEC_61334> , <https://en.wikipedia.org/wiki/IEC_61334> .

rami:safety  a  owl:NamedIndividual .

sto:IEC_61334_P4_S33_1998
        a                          sto:Standard , owl:NamedIndividual ;
        rdfs:comment               "Covers the services required by the data communication protocol (DCP) logical link control (LLC) sublayer entity at the logical interfaces with the LLC -user layer and the MAC sublayer, using the connection-oriented LLC procedures.\nThis publication is of high relevance for Smart Grid."@en ;
        rdfs:label                 "IEC 61334-4-33:1998 "@en ;
        sto:hasAvailableLanguage   "English/French"@en ;
        sto:hasDBpediaResource     <https://dbpedia.org/resource/IEC_61334> , <null//dbpedia.org/resource/IEC_61334> ;
        sto:hasEdition             "1.0"^^xsd:float ;
        sto:hasFileSize            sto:FileSizeIEC_61334_1998_P4_S3 ;
        sto:hasICS                 sto:ICS_33_200 , sto:ICS_29_240_20 ;
        sto:hasOfficialResource    <null//webstore.iec.ch/publication/5302> , <https://webstore.iec.ch/publication/5302> ;
        sto:hasPages               "51"^^xsd:int ;
        sto:hasPublicationDate     "1998-07-191"^^xsd:date ;
        sto:hasPublisher           sto:IEC ;
        sto:hasStabilityDate       "2018"^^xsd:gYear ;
        sto:hasTag                 "IEC 61334-4-33:1998 "@en ;
        sto:hasTechnicalCommittee  sto:TC_57 ;
        sto:hasTitle               "Distribution automation using distribution line carrier systems - Part 4-33: Data communication protocols - Data link layer - Connection oriented protocol"@en ;
        sto:hasWikipediaArticle    <null//en.wikipedia.org/wiki/IEC_61334> , <https://en.wikipedia.org/wiki/IEC_61334> .

sto:hasPublisher  a         owl:ObjectProperty ;
        rdfs:comment        "The organization that published this Standard"@en ;
        rdfs:domain         sto:Publication ;
        rdfs:label          "has Publisher"@en ;
        rdfs:range          sto:StandardOrganization ;
        rdfs:subPropertyOf  foaf:maker .

om2:hasUnit  a  owl:AnnotationProperty .

sto:ProductDevelopmentLifeCycle
        a                 owl:Class ;
        rdfs:comment      "PLM is the process of managing the entire lifecycle of a product from inception, through engineering design and manufacture, to service and disposal of manufactured products. Related areas are PLMManagement, Modeling Practice, Product Model Data exchange, Manufacturing Model Data, Product Catalog Data."@en , "Product Development Life-Cycle Phase"@en ;
        rdfs:isDefinedBy  "https://en.wikipedia.org/wiki/Product_lifecycle" ;
        rdfs:label        "Product Development Life Cycle"@en ;
        rdfs:subClassOf   sto:StandardClassification .

sto:ISO_1101  a                  owl:NamedIndividual , sto:Standard ;
        rdfs:comment             "Geometrical product specifications (GPS) -- Geometrical tolerancing -- Tolerances of form, orientation, location and run-out"@en ;
        rdfs:label               "ISO 1101"@en ;
        sto:hasClassification    rami:Asset , sto:ModelingPractice , rami:Product ;
        sto:hasOfficialResource  "https://www.iso.org/standard/66777.html" ;
        sto:hasPublicationDate   "2017-02-01"^^xsd:date ;
        sto:hasPublisher         sto:ISO .

sto:IEC_60870_P6_S501_1995
        a                          sto:Standard , owl:NamedIndividual ;
        rdfs:comment               "Defines the services provided by a telecontrol specific application-service-element - the Telecontrol Application Service Element No. 1 (TASE.1) - for the exchange of process data in telecontrol systems.\nThis publication is of high relevance for Smart Grid."@en ;
        rdfs:label                 "IEC 60870-6-501:1995"@en ;
        sto:hasAvailableLanguage   "English/French"@en ;
        sto:hasDBpediaResource     <https://dbpedia.org/resource/IEC_60870> , <null//dbpedia.org/resource/IEC_60870> ;
        sto:hasEdition             "1.0"^^xsd:float ;
        sto:hasFileSize            sto:FileSizeIEC_60870_P6_S501_1995 ;
        sto:hasICS                 sto:ICS_33_200 ;
        sto:hasOfficialResource    <null//webstore.iec.ch/publication/3758> , <https://webstore.iec.ch/publication/3758> ;
        sto:hasPages               "170"^^xsd:int ;
        sto:hasPublicationDate     "1995-12-352"^^xsd:date ;
        sto:hasPublisher           sto:IEC ;
        sto:hasStabilityDate       "2018"^^xsd:gYear ;
        sto:hasTag                 "IEC 60870-6-501:1995"@en ;
        sto:hasTechnicalCommittee  sto:TC_57 ;
        sto:hasTitle               "Telecontrol equipment and systems - Part 6: Telecontrol protocols compatible with ISO standards and ITU-T recommendations - Section 501: TASE.1 Service definitions"@en ;
        sto:hasWikipediaArticle    <https://en.wikipedia.org/wiki/IEC_60870> , <null//en.wikipedia.org/wiki/IEC_60870> .

sto:domainName  a     owl:DatatypeProperty ;
        rdfs:comment  "Points the Standard with the name of the Industrial Domain"@en ;
        rdfs:domain   sto:Domain ;
        rdfs:label    "has Domain Name"@en ;
        rdfs:range    rdf:PlainLiteral .

sto:relatedTo  a       owl:ObjectProperty , owl:SymmetricProperty , owl:TransitiveProperty ;
        rdfs:comment   "Represent any type of relation that connects two standards."@en ;
        rdfs:domain    sto:Publication ;
        rdfs:label     "related To"@en ;
        rdfs:range     sto:Publication ;
        skos:altLabel  "has Associated Standard"@en .

sto:ConnectivityLayer
        a                 owl:Class ;
        rdfs:comment      "Connectivity Layer of the Internet Connectivity Framework"@en ;
        rdfs:isDefinedBy  "https://www.iiconsortium.org/pdf/IIC_PUB_G5_V1.01_PB_20180228.pdf" ;
        rdfs:label        "Connectivity Layer"@en ;
        rdfs:subClassOf   sto:StandardClassification .

sto:IEC_24760  a                 sto:Standard , owl:NamedIndividual ;
        rdfs:comment             "ISO/IEC 24760: it defines terms for identity management, and also specifies core concepts of identity and identity management and their relationships. It is applicable to any information system that processes identity information. A bibliography of documents describing various aspects of identity information management is provided."@en ;
        rdfs:label               "IEC 24760"@en ;
        sto:hasClassification    rami:Information , rami:ControlDevice , rami:FieldDevice , rami:Safety , rami:Station , rami:Security , sto:ProductModelDataExchange , rami:Product ;
        sto:hasDomain            sto:ITSecurity ;
        sto:hasOfficialResource  "https://www.iso.org/standard/57914.html" ;
        sto:hasPublicationDate   "2011-01-12"^^xsd:date ;
        sto:hasPublisher         sto:IEC ;
        sto:relatedTo            sto:IEC_62443 .

sto:ETSI  a                      owl:NamedIndividual , sto:StandardOrganization ;
        rdfs:comment             "The European Telecommunications Standards Institute (ETSI) is an independent, not-for-profit, standardization organization in the telecommunications industry (equipment makers and network operators) in Europe, headquartered in Sophia-Antipolis, France, with worldwide projection. ETSI produces globally-applicable standards for Information and Communications Technologies (ICT), including fixed, mobile, radio, converged, broadcast and internet technologies."@en ;
        rdfs:label               "ETSI"@en ;
        sto:abbreviation         "ETSI"@en ;
        sto:formationDate        "1988-01-01"^^xsd:date ;
        sto:hasDBpediaResource   "http://dbpedia.org/resource/ETSI" ;
        sto:hasHeadquaterIn      dbr:Valbonne ;
        sto:hasOfficialResource  "http://www.etsi.org/" ;
        sto:hasWikipediaArticle  "https://en.wikipedia.org/wiki/ETSI" ;
        sto:orgName              "European Telecommunications Standards Institute"@en .

cc:attributionName  a  owl:AnnotationProperty .

sto:Domain  a         owl:Class ;
        rdfs:comment  "Represents the Domains in which the Standards can be used"@en ;
        rdfs:label    "Domain"@en .

sto:ISO_8062-4  a                sto:Standard , owl:NamedIndividual ;
        rdfs:comment             "Geometrical product specifications (GPS) -- Dimensional and geometrical tolerances for moulded parts -- General tolerances for castings using profile tolerancing in a general datum system"@en ;
        rdfs:label               "ISO 8062-4"@en ;
        sto:hasClassification    rami:Product , sto:ProductionSystemModelData , rami:Asset ;
        sto:hasOfficialResource  "https://www.iso.org/standard/60774.html" ;
        sto:hasPublicationDate   "2017-07-01"^^xsd:date ;
        sto:hasPublisher         sto:ISO ;
        sto:hasTag               "Automation systems and integration"@en ;
        sto:relatedTo            sto:ISO_10303 .

sto:ProductionSystemLifeCycle
        a                 owl:Class ;
        rdfs:comment      "Collections of machines, equipment, and auxiliary systems organized to create goods and services from various resources."@en ;
        rdfs:isDefinedBy  "http://nvlpubs.nist.gov/nistpubs/ir/2016/NIST.IR.8107.pdf" ;
        rdfs:label        "Production System Life Cycle"@en ;
        rdfs:subClassOf   sto:StandardClassification .

sto:IEC_60255_151_2009
        a                            owl:NamedIndividual , sto:Standard ;
        rdfs:comment                 "IEC 60255-151:2009 specifies minimum requirements for over/under current relays. It includes a specification of the protection function, measurement characteristics and time delay characteristics. Defines the influencing factors that affect the accuracy under steady state conditions and performance characteristics during dynamic conditions."@en ;
        rdfs:label                   "IEC 60255-151:2009 "@en ;
        sto:hasAvailableLanguage     "English/French"@en ;
        sto:hasEdition               "1.0"^^xsd:float ;
        sto:hasFileSize              sto:FileSizeIEC_60255_151_2009 ;
        sto:hasICS                   sto:ICS_29_120_70 ;
        sto:hasImplementationFormat  "Document"@en ;
        sto:hasOfficialResource      <https://webstore.iec.ch/publication/1166> ;
        sto:hasPages                 63 ;
        sto:hasPublicationDate       "2009-08-28"^^xsd:date ;
        sto:hasPublisher             sto:IEC ;
        sto:hasStatus                "Valid"@en ;
        sto:hasTag                   "IEC 60255-151:2009 "@en ;
        sto:hasTechnicalCommittee    sto:TC_95 ;
        sto:hasTitle                 "Measuring relays and protection equipment - Part 151: Functional requirements for over/under current protection"@en .

sto:ISO_5459  a                  sto:Standard , owl:NamedIndividual ;
        rdfs:comment             "Geometrical product specifications (GPS) -- Geometrical tolerancing -- Datums and datum systems--ISO 5459:2011 specifies terminology, rules and methodology for the indication and understanding of datums and datum systems in technical product documentation"@en ;
        rdfs:label               "ISO 5459"@en ;
        sto:hasClassification    rami:Asset , rami:Product , sto:ModelingPractice ;
        sto:hasDomain            sto:M2M ;
        sto:hasOfficialResource  "https://www.iso.org/standard/40358.html" ;
        sto:hasPublicationDate   "2011-08-01"^^xsd:date ;
        sto:hasPublisher         sto:ISO .

sto:IEC_61400  a                 owl:NamedIndividual , sto:Standard ;
        rdfs:comment             "IEC 61334 , known as Distribution automation using distribution line carrier systems, is a standard for low-speed reliable power line communications by electricity meters, water meters and SCADA."@en ;
        rdfs:label               "IEC 61400"@en ;
        sto:hasDBpediaResource   "http://dbpedia.org/page/IEC_61400" ;
        sto:hasOfficialResource  "https://webstore.iec.ch/publication/26603" ;
        sto:hasPublicationDate   "2017-03-03"^^xsd:date ;
        sto:hasPublisher         sto:IEC .

sto:IEC_60255_2013  a                owl:NamedIndividual , sto:Standard ;
        rdfs:comment                 "IEC 60255-27:2013 describes the product safety requirements for measuring relays and protection equipment having a rated a.c. voltage up to 1 000 V with a rated frequency up to 65 Hz, or a rated d.c. voltage up to 1 500 V. Above these limits, IEC 60664-1 is applicable for the determination of clearance, creepage distance and withstand test voltage. This standard details essential safety requirements to minimize the risk of fire and hazards caused by electric shock or injury to the user. This new edition includes the following significant technical changes with respect to the previous edition:- the removal of tables and diagrams which are from other standards and referring instead directly to the source standard;- all aspects of IEC 60255-5 have been covered and this standard will be withdrawn."@en ;
        rdfs:label                   "IEC 60255-27:2013 "@en ;
        sto:hasAvailableLanguage     "English/French"@en ;
        sto:hasEdition               "2.0"^^xsd:float ;
        sto:hasFileSize              sto:FileSizeIEC_60255_2013 ;
        sto:hasICS                   sto:ICS_29_120_70 ;
        sto:hasImplementationFormat  "Document"@en ;
        sto:hasOfficialResource      <https://webstore.iec.ch/publication/1172> ;
        sto:hasPages                 197 ;
        sto:hasPublicationDate       "2013-10-15"^^xsd:date ;
        sto:hasPublisher             sto:IEC ;
        sto:hasStabilityDate         "2018"^^xsd:gYear ;
        sto:hasStatus                "Valid"@en ;
        sto:hasTag                   "IEC 60255-27:2013 "@en ;
        sto:hasTechnicalCommittee    sto:TC_95 ;
        sto:hasTitle                 "Measuring relays and protection equipment - Part 27: Product safety requirements"@en .

dbr:Beijing  a  owl:NamedIndividual .

dcterms:linguisticSystem
        a       owl:Class .

sto:GPLv2  a            owl:NamedIndividual , dcterms:LicenseDocument ;
        rdfs:comment    "Published under Open Content License."@en ;
        rdfs:label      "GNU General Public License"@en ;
        rdfs:seeAlso    "<https://opcfoundation.org/license/gpl.htm>" ;
        skos:prefLabel  "OCL 1.0" .

sto:IEC_60864_P1  a                owl:NamedIndividual , sto:Standard ;
        rdfs:comment               "Applies to all classes of transmitters for sound and television broadcasting. Deals with the interface between a transmitter (or system of transmitters) and the supervisory equipment which is intended to remotely monitor and/or control the transmitter(s). Details the interconnections and facilities to be provided with a view to achieving compatibility between different types and makes of transmitters and supervisory equipment."@en ;
        rdfs:label                 "IEC 60864-1:1986 "@en ;
        sto:hasAvailableLanguage   "English/French"@en ;
        sto:hasEdition             "1.0"^^xsd:float ;
        sto:hasFileSize            <https://w3id.org/i40/sto#FileSizeIEC_60864_P1 > ;
        sto:hasICS                 sto:ICS_33_060_20 , sto:ICS_33_200 ;
        sto:hasOfficialResource    <null//webstore.iec.ch/publication/3727> ;
        sto:hasPages               "43"^^xsd:int ;
        sto:hasPublicationDate     "1986-01-01"^^xsd:date ;
        sto:hasPublisher           sto:IEC ;
        sto:hasStabilityDate       "2020"^^xsd:gYear ;
        sto:hasTag                 "IEC 60864-1:1986 "@en ;
        sto:hasTechnicalCommittee  sto:TC_103 ;
        sto:hasTitle               "Standardization of interconnections between broadcasting transmitters or transmitter systems and supervisory equipment. Part 1: Interface standards for systems using dedicated interconnections"@en .

rami:TypeMaintenance  a  owl:NamedIndividual , rami:RAMILifeCycleLayer ;
        rdfs:label  "Type Maintenance"@en .

rami:Communications  a  owl:NamedIndividual .

sto:IEC_61010_P2_S202_2016
        a                          owl:NamedIndividual , sto:Standard ;
        rdfs:comment               "IEC 61010-2-202:2016 specifies the safety requirements for electric ACTUATORs and SOLENOIDs, as applied to valves, intended to be installed in an industrial process or discrete control environment. \n\nThis publication is to be read in conjunction with IEC 61010-1:2010."@en ;
        rdfs:label                 "IEC 61010-2-202:2016"@en ;
        sto:hasAvailableLanguage   "English/French"@en ;
        sto:hasEdition             "1.0"^^xsd:float ;
        sto:hasFileSize            sto:FileSizeIEC_61010_P2_S202_2016 ;
        sto:hasICS                 sto:19_020 , sto:ICS_13_110 , sto:ICS_17_020 ;
        sto:hasOfficialResource    <https://webstore.iec.ch/publication/25399> , <null//webstore.iec.ch/publication/25399> ;
        sto:hasPages               "25"^^xsd:int ;
        sto:hasPublicationDate     "2016-07-194"^^xsd:date ;
        sto:hasPublisher           sto:IEC ;
        sto:hasStabilityDate       "2019"^^xsd:gYear ;
        sto:hasTag                 "IEC 61010-2-202:2016"@en ;
        sto:hasTechnicalCommittee  sto:TC_65 ;
        sto:hasTitle               "Safety requirements for electrical equipment for measurement, control and laboratory use - Part 2-202: Particular requirements for electrically operated valve actuators"@en .

sto:FileSizeIEC_61334_2001_P4_S512
        a                      om2:Measure , owl:NamedIndividual ;
        rdfs:comment           "Specifies the file size of the document for standard IEC 61334-4-512:2001"@en ;
        rdfs:label             "FileSize IEC 61334-4-512:2001"@en ;
        om2:hasNumericalValue  "459.0"^^xsd:float ;
        om2:hasUnit            om2:kilobyte .

sto:TC_40  a          owl:NamedIndividual , sto:TechnicalCommittee ;
        rdfs:comment  "To prepare international standards for:a) Capacitors, resistors, thermistors and varistors intended for use in electronic equipment.b) Capacitors, resistors and inductors and complete electromagnetic interference (EMI) suppression filter units for EMI suppression (see note).c) Passive integrated circuits or networks containing resistors, capacitors, inductors or their combinations. For the dimensional standardization of the final package, requirements laid down by TC 47 shall be adopted whenever possible.d) Packaging of electronic components for automatic handling, which is an activity undertaken on behalf of all relevant component technical committees.e) Electric double layer capacitors for use in electric and electronic equipment.Note: In this work, use has to be made as far as possible of any relevant work of TC 51 on inductors, the CISPR on the measurement of EMI suppression characteristics and TC 77 on electromagnetic compatibility (EMC). Liaison has also to be maintained with TC 61, TC 66, TC 108 and other appropriate IEC Technical Committees on the safety aspects of EMI suppression components and filter units."@en ;
        rdfs:label    "TC 40"@en ;
        sto:hasTitle  "Capacitors and resistors for electronic equipment"@en .

sto:ISO_9000  a                  owl:NamedIndividual , sto:Standard ;
        rdfs:comment             "The ISO 9000 family of quality management systems standards is designed to help organizations ensure that they meet the needs of customers and other stakeholders while meeting statutory and regulatory requirements related to a product or program."@en ;
        rdfs:label               "ISO 9000"@en ;
        sto:hasClassification    sto:CrossLevel ;
        sto:hasDBpediaResource   "http://dbpedia.org/page/ISO_9000" ;
        sto:hasOfficialResource  "https://www.iso.org/iso-9001-quality-management.html" ;
        sto:hasPublisher         sto:ISO ;
        sto:hasWikipediaArticle  "https://en.wikipedia.org/wiki/ISO_9000" .

sto:ICS_35_240_50  a  sto:InternationalClassificationForStandards , owl:NamedIndividual ;
        rdfs:comment  "This is ICS for IT applications in industry"@en , "This is ICS for “IT applications in industry)”"@en ;
        rdfs:label    "ICS 35.240.50"@en ;
        sto:hasTitle  "IT applications in industry"@en .

sto:IEC_61690_P2_2000
        a                          owl:NamedIndividual , sto:Standard ;
        rdfs:comment               "IEC 61690-2:2000 defines the syntax and semantics for EDIF Version 4 0 0. EDIF Version 4 0 0 addresses EDIF Level 0 and Level 1. EDIF Version 3 0 0 provides support for Connectivity and Schematics; EDIF Version 4 0 0 offers additional capability by providing support for the representation of Printed Circuit Boards (PCBs) and Multi-chip Modules (MCMs) including technology rules and assembly drawings."@en ;
        rdfs:label                 "IEC 61690-2:2000"@en ;
        sto:hasAvailableLanguage   "English"@en , " French"@en ;
        sto:hasEdition             "1.0"^^xsd:float ;
        sto:hasFileSize            sto:FileSizeIEC_61690_P2_2000 ;
        sto:hasICS                 sto:ICS_35_240_50 ;
        sto:hasOfficialResource    <https://webstore.iec.ch/publication/5724> , <null//webstore.iec.ch/publication/5724> ;
        sto:hasPublicationDate     "2000-01-31"^^xsd:date ;
        sto:hasPublisher           sto:IEC ;
        sto:hasStabilityDate       "2018"^^xsd:gYear ;
        sto:hasTag                 "IEC 61690-2:2000"@en ;
        sto:hasTechnicalCommittee  sto:TC_91 ;
        sto:hasTitle               "Electronic design interchange format (EDIF) - Part 2: Version 4 0 0. (This publication is available in electronic HTML format only)"@en .

rami:Conditional_Monitoring
        a       owl:NamedIndividual .

sto:ANSI  a                      sto:StandardOrganization , owl:NamedIndividual ;
        rdfs:comment             "The American National Standards Institute is a private non-profit organization that oversees the development of voluntary consensus standards for products, services, processes, systems, and personnel in the United States. The organization also coordinates U.S. standards with international standards so that American products can be used worldwide. ANSI accredits standards that are developed by representatives of other standards organizations, government agencies, consumer groups, companies, and others. These standards ensure that the characteristics and performance of products are consistent, that people use the same definitions and terms, and that products are tested the same way. ANSI also accredits organizations that carry out product or personnel certification in accordance with requirements defined in international standards."@en ;
        rdfs:label               "ANSI"@en ;
        sto:abbreviation         "ANSI" ;
        sto:formationDate        "1918-05-14"^^xsd:date ;
        sto:hasDBpediaResource   <http://dbpedia.org/resource/American_National_Standards_Institute> ;
        sto:hasHeadquaterIn      <http://dbpedia.org/resource#Washington,_D.C.> ;
        sto:hasOfficialResource  <https://www.ansi.org/> ;
        sto:hasWikipediaArticle  <https://en.wikipedia.org/wiki/American_National_Standards_Institute?oldformat=true> ;
        sto:orgName              "American National Standards Institute"@en .

sto:IEC_62443  a                 sto:Standard , owl:NamedIndividual ;
        rdfs:comment             "ISA/IEC-62443 is a series of standards, technical reports, and related information that define procedures for implementing electronically secure Industrial Automation and Control Systems (IACS). This guidance applies to end-users (i.e. asset owner), system integrators, security practitioners, and control systems manufacturers responsible for manufacturing, designing, implementing, or managing industrial automation and control systems."@en , "Defines procedures for implementing electronically secure Industrial Automation and Control Systems."@en ;
        rdfs:label               "IEC 62443"@en ;
        dcterms:hasLicense       "Private"@en ;
        skos:altLabel            "ISA 99" ;
        skos:note                "TODO" ;
        sto:hasClassification    rami:Security , sto:CrossLevel ;
        sto:hasDBpediaResource   "http://dbpedia.org/page/Cyber_security_standards#ISA/IEC-62443_(formerly_ISA-99)" ;
        sto:hasDeveloper         sto:ANSI , sto:ISA ;
        sto:hasMotivation        "Cyber attacks threat the industry and can cause damage to property and personal injury and affect the image of companies. The Standard allows to define procedures for implementing electronically secure Industrial Automation and Control Systems (IACS). This guidance applies to end-users, system integrators, security practitioners, and control systems manufacturers responsible for manufacturing, designing, implementing, or managing industrial automation and control systems"@en ;
        sto:hasOfficialResource  "https://webstore.iec.ch/publication/7029" , "https://webstore.iec.ch/publication/7033" ;
        sto:hasPublisher         sto:ANSI , sto:IEC , sto:ISA ;
        sto:hasTag               "Electronically secure Industrial Automation and Control Systems"@en , "Network and system security for industrial-process measurement and control"@en ;
        sto:hasWikipediaArticle  <https://en.wikipedia.org/wiki/Cyber_security_standards#ISA.2FIEC-62443_.28formerly_ISA-99.29> .

sto:ManufacturingModelData
        a                  owl:NamedIndividual , sto:ProductDevelopmentLifeCycle ;
        rdfs:comment       "Manufacturing Model Data Standards define the data needed to manufacture a product from a design."@en ;
        rdfs:label         "Manufacturing Model Data"@en ;
        sto:isDescribedin  sto:NISTInitiative .

dul:isComponentOf  a        owl:ObjectProperty ;
        rdfs:comment        "Represents Standards that are component of other Standards. This relation is not transitive"@en ;
        rdfs:domain         sto:Standard ;
        rdfs:isDefinedBy    <http://www.ontologydesignpatterns.org/ont/dul/DUL.owl> ;
        rdfs:label          "is Component Of"@en ;
        rdfs:range          sto:Standard ;
        rdfs:subPropertyOf  sto:relatedTo .

sto:ModBus  a                    owl:NamedIndividual , sto:Standard ;
        rdfs:comment             "Modbus is a serial communications protocol to be used in Programmable logic controllers (PLCs)."@en ;
        rdfs:label               "ModBus"@en ;
        sto:hasClassification    rami:Integration ;
        sto:hasDBpediaResource   "http://dbpedia.org/page/Modbus" ;
        sto:hasOfficialResource  "http://www.modbus.org/" ;
        sto:hasPublisher         sto:SE ;
        sto:hasTag               "Modbus"@en ;
        sto:hasWikipediaArticle  "https://en.wikipedia.org/wiki/Modbus" .

sto:FileSizeIEC_60946
        a                      om2:Measure , owl:NamedIndividual ;
        rdfs:comment           "Specifies the file size of the document for standard IEC 60946"@en ;
        rdfs:label             "FileSize IEC 60946"@en ;
        om2:hasNumericalValue  "546.0"^^xsd:float ;
        om2:hasUnit            om2:kilobyte .

sto:Manufacturing  a  owl:NamedIndividual .

rami:Engineering  a        owl:NamedIndividual , rami:AdminShellSubmodel ;
        sto:isDescribedin  sto:AdministrationShell .

sto:IEC_60050_2013  a                sto:Standard , owl:NamedIndividual ;
        rdfs:comment                 "IEC 60050-351:2013 gives the general terminology used in control technology, as well as general terms pertaining to specific applications and associated technologies. This new edition reviews and complements the previous one. It has the status of a horizontal standard in accordance with IEC Guide 108."@en ;
        rdfs:label                   "IEC 60050-351:2013"@en ;
        sto:hasAvailableLanguage     "English/French"@en ;
        sto:hasEdition               "4.0"^^xsd:float ;
        sto:hasFileSize              sto:FileSizeIEC_60050_2013 ;
        sto:hasICS                   sto:ICS_25_040_40 , sto:ICS_01_040_07 ;
        sto:hasImplementationFormat  "Document"@en ;
        sto:hasOfficialResource      <https://webstore.iec.ch/publication/194> ;
        sto:hasPages                 457 ;
        sto:hasPublicationDate       "2013-11-25"^^xsd:date ;
        sto:hasPublisher             sto:IEC ;
        sto:hasStatus                "Valid"@en ;
        sto:hasTag                   "IEC 60050-351:2013"@en ;
        sto:hasTechnicalCommittee    sto:TC_1 ;
        sto:hasTitle                 "International Electrotechnical Vocabulary - Part 351: Control technology"@en .

sto:IEC_61804  a                 owl:NamedIndividual , sto:Standard ;
        rdfs:comment             "Function blocks (FB) for process control - Overview of system aspects "@en ;
        rdfs:label               "IEC 61804"@en ;
        sto:hasClassification    rami:Configuration , rami:ControlDevice , rami:FieldDevice ;
        sto:hasDBpediaResource   "http://dbpedia.org/resource/Device_Description_Language" ;
        sto:hasOfficialResource  "https://webstore.iec.ch/publication/5953" ;
        sto:hasPublisher         sto:IEC ;
        sto:hasTag               "EDDL"@en ;
        sto:hasWikipediaArticle  "https://en.wikipedia.org/wiki/Device_Description_Language" ;
        sto:relatedTo            sto:IEC_62453 .

sto:IEC_61334_P4_S42_1996
        a                          owl:NamedIndividual , sto:Standard ;
        rdfs:comment               "Describes the rules used to design an application service element, the ISO connectionless ACSE (Application Control Service Element), and the DLMS Application Service Element.\nThis publication is of high relevance for Smart Grid."@en ;
        rdfs:label                 "IEC 61334-4-42:1996"@en ;
        sto:hasAvailableLanguage   "English/French"@en ;
        sto:hasDBpediaResource     <null//dbpedia.org/resource/IEC_61334> , <https://dbpedia.org/resource/IEC_61334> ;
        sto:hasEdition             "1.0"^^xsd:float ;
        sto:hasFileSize            sto:FileSizeIEC_61334_1996_P4_S42 ;
        sto:hasICS                 sto:ICS_29_240_20 , sto:ICS_33_200 ;
        sto:hasOfficialResource    <null//webstore.iec.ch/publication/5304> , <https://webstore.iec.ch/publication/5304> ;
        sto:hasPages               "89"^^xsd:int ;
        sto:hasPublicationDate     "1996-10-283"^^xsd:date ;
        sto:hasPublisher           sto:IEC ;
        sto:hasStabilityDate       "2018"^^xsd:gYear ;
        sto:hasTag                 "IEC 61334-4-42:1996"@en ;
        sto:hasTechnicalCommittee  sto:TC_57 ;
        sto:hasTitle               "Distribution automation using distribution line carrier systems -Part 4: Data communication protocols - Section 42: Applicationprotocols - Application laye"@en ;
        sto:hasWikipediaArticle    <https://en.wikipedia.org/wiki/IEC_61334> , <null//en.wikipedia.org/wiki/IEC_61334> .

sto:IEC_61508  a                 sto:Standard , owl:NamedIndividual ;
        rdfs:comment             "Functional safety is a concept applicable across all industry sectors. It is fundamental to the enabling of complex technology used for safety-related systems. It provides the assurance that the safety-related systems will offer the necessary risk reduction required to achieve safety for the equipment. The oil and gas industry, nuclear plants and the machinery sector, to name but a few, all rely heavily on functional safety to achieve safety for the equipment giving rise to the hazards."@en ;
        rdfs:label               "IEC 60508"@en ;
        dcterms:hasLicense       "Private"@en ;
        sto:hasClassification    rami:Safety ;
        sto:hasDBpediaResource   "http://dbpedia.org/resource/IEC_61508" ;
        sto:hasMotivation        "Defines the functional safety requirements established by IEC 61508 in process industry sector terminology"@en ;
        sto:hasOfficialResource  "http://www.iec.ch/functionalsafety/" ;
        sto:hasPublisher         sto:IEC ;
        sto:hasTag               "Functional Safety of Electrical/Electronic/Programmable Electronic Safety-related Systems"@en ;
        sto:hasWikipediaArticle  "https://en.wikipedia.org/wiki/IEC_61508" ;
        sto:relatedTo            sto:IEC_61511 .

sto:NIST  a                      owl:NamedIndividual , sto:StandardOrganization ;
        rdfs:comment             "The National Institute of Standards and Technology (NIST) is a measurement standards laboratory, and a non-regulatory agency of the United States Department of Commerce."@en ;
        sto:abbreviation         "NIST" ;
        sto:belongsTo            dbr:United_States ;
        sto:formationDate        "1901-01-01"^^xsd:date ;
        sto:hasDBpediaResource   "http://dbpedia.org/page/National_Institute_of_Standards_and_Technology" ;
        sto:hasHeadquaterIn      dbr:_Maryland ;
        sto:hasOfficialResource  "https://www.nist.gov/" ;
        sto:hasWikipediaArticle  "https://en.wikipedia.org/wiki/National_Institute_of_Standards_and_Technology" ;
        sto:orgName              "National Institute of Standards and Technology"@en .

sto:FileSizeIEC_60839_P7_7
        a                      om2:Measure , owl:NamedIndividual ;
        rdfs:comment           "Specifies the file size of the document for standard IEC 60839-7-7:2001"@en ;
        rdfs:label             "FileSize IEC 60839-7-7:2001"@en ;
        om2:hasNumericalValue  "964.0"^^xsd:float ;
        om2:hasUnit            om2:kilobyte .

rami:RAMIITLayer  a          owl:Class ;
        rdfs:label           "RAMI IT Layer"@en ;
        rdfs:subClassOf      sto:StandardClassification ;
        owl:equivalentClass  [ a          owl:Class ;
                               owl:oneOf  ( rami:Asset rami:Business rami:Communication rami:Functional rami:Information rami:Integration )
                             ] .

sto:FileSizeIEC_60870_P5_S5_1995
        a                      om2:Measure , owl:NamedIndividual ;
        rdfs:comment           "Specifies the file size of the document for standard IEC 60870-5-5:1995"@en ;
        rdfs:label             "FileSize IEC 60870-5-5:1995"@en ;
        om2:hasNumericalValue  "3347.0"^^xsd:float ;
        om2:hasUnit            om2:kilobyte .

sto:FileSizeIEC_60864_P2
        a                      om2:Measure , owl:NamedIndividual ;
        rdfs:comment           "Specifies the file size of the document for standard IEC 60864-2:1997"@en ;
        rdfs:label             "FileSize IEC 60864-2:1997"@en ;
        om2:hasNumericalValue  "283.0"^^xsd:float ;
        om2:hasUnit            om2:kilobyte .

sto:IEC_60870_P6_S502_1995
        a                          owl:NamedIndividual , sto:Standard ;
        rdfs:comment               "Specifies the protocol for the services provided by an application-service-element - the Telecontrol Application Service Element No. 1 (TASE.1) - to support the exchange of process data between telecontrol systems.\nThis publication is of high relevance for Smart Grid."@en ;
        rdfs:label                 "IEC 60870-6-502:1995"@en ;
        sto:hasAvailableLanguage   "English/French"@en ;
        sto:hasDBpediaResource     <https://dbpedia.org/resource/IEC_60870> , <null//dbpedia.org/resource/IEC_60870> ;
        sto:hasEdition             "1.0"^^xsd:float ;
        sto:hasFileSize            sto:FileSizeIEC_60870_P6_S502_1995 ;
        sto:hasICS                 sto:ICS_33_200 ;
        sto:hasOfficialResource    <null//webstore.iec.ch/publication/3759> , <https://webstore.iec.ch/publication/3759> ;
        sto:hasPages               "57"^^xsd:int ;
        sto:hasPublicationDate     "1995-12-339"^^xsd:date ;
        sto:hasPublisher           sto:IEC ;
        sto:hasStabilityDate       "2018"^^xsd:gYear ;
        sto:hasTag                 "IEC 60870-6-502:1995"@en ;
        sto:hasTechnicalCommittee  sto:TC_57 ;
        sto:hasTitle               "Telecontrol equipment and systems - Part 6: Telecontrol protocols compatible with ISO standards and ITU-T recommendations - Section 502: TASE.1 Protocol definitions"@en ;
        sto:hasWikipediaArticle    <null//en.wikipedia.org/wiki/IEC_60870> , <https://en.wikipedia.org/wiki/IEC_60870> .

sto:FileSizeIEC_60870_P6_S503_2014
        a                      om2:Measure , owl:NamedIndividual ;
        rdfs:comment           "Specifies the file size of the document for standard IEC 60870-6-503:2014"@en ;
        rdfs:label             "FileSize IEC 60870-6-503:2014"@en ;
        om2:hasNumericalValue  "2630.0"^^xsd:float ;
        om2:hasUnit            om2:kilobyte .

sto:DMSC  a                      owl:NamedIndividual , sto:StandardOrganization ;
        rdfs:comment             "Dimensional Metrology Standards Consortium (DMSC) is to identify urgently needed standards in the field of dimensional metrology, and to promote, foster, and encourage the development and interoperability of these standards, along with related and supporting standards that will benefit the industry as a whole."@en ;
        rdfs:label               "Dimensional Metrology Standards Consortium"@en ;
        sto:hasHeadquaterIn      dbr:_Texas ;
        sto:hasOfficialResource  <http://www.dmis.org/> .

sto:IEC_61158  a                 owl:NamedIndividual , sto:Standard ;
        rdfs:comment             "Fieldbus is the name of a family of industrial computer network protocols used for real-time distributed control, standardized as IEC 61158. A complex automated industrial system such as manufacturing assembly line usually needs a distributed control system an organized hierarchy of controller systems to function. In this hierarchy, there is usually a Human Machine Interface (HMI) at the top, where an operator can monitor or operate the system. This is typically linked to a middle layer of programmable logic controllers (PLC) via a non-time-critical communications system (e.g. Ethernet). At the bottom of the control chain is the fieldbus that links the PLCs to the components that actually do the work, such as sensors, actuators, electric motors, console lights, switches, valves and contactors"@en ;
        rdfs:label               "IEC 61158"@en ;
        sto:hasDBpediaResource   "http://dbpedia.org/page/Fieldbus" ;
        sto:hasOfficialResource  "http://www.fieldbus.org/" ;
        sto:hasPublisher         sto:IEC ;
        sto:hasTag               "Fieldbus"@en ;
        sto:hasWikipediaArticle  "https://en.wikipedia.org/wiki/Fieldbus" ;
        sto:relatedTo            sto:IEC_61784 .

dbr:Höhenkirchen-Siegertsbrunn
        a       owl:NamedIndividual .

rami:RAMIHierarchyLevel
        a                    owl:Class ;
        rdfs:label           "RAMI Hierarchy Level"@en ;
        rdfs:subClassOf      sto:StandardClassification ;
        owl:equivalentClass  [ a          owl:Class ;
                               owl:oneOf  ( rami:ConnectedWorld rami:ControlDevice rami:Enterprise rami:FieldDevice rami:Product rami:Station rami:WorkCenter )
                             ] .

sto:ISO_16792  a                 sto:Standard , owl:NamedIndividual ;
        rdfs:comment             "ISO 16792 Technical product documentation -- Digital product definition data practices-It supports two methods of application: model-only and model and drawing in digital format."@en ;
        rdfs:label               "ISO 16792"@en ;
        sto:hasClassification    sto:ModelingPractice , rami:Product , rami:Asset ;
        sto:hasDomain            sto:CAD ;
        sto:hasOfficialResource  "https://www.iso.org/standard/56865.html" ;
        sto:hasPublicationDate   "2015-12-01"^^xsd:date ;
        sto:hasPublisher         sto:ISO .

sto:ISO_10303  a                 owl:NamedIndividual , sto:Standard ;
        rdfs:comment             "Standard for the Exchange of Product model data. ISO 10303 can represent 3D objects in Computer-aided design (CAD) and related information."@en ;
        rdfs:label               "ISO 10303"@en ;
        skos:note                "TODO - Split properly and classify it - check the NIST paper" ;
        sto:hasClassification    sto:ProductLifeCycleManagement ;
        sto:hasDBpediaResource   "http://dbpedia.org/page/ISO_10303" ;
        sto:hasOfficialResource  "https://www.steptools.com/stds/step/" ;
        sto:hasPublisher         sto:ISO ;
        sto:hasTag               "STEP"@en ;
        sto:hasWikipediaArticle  "https://en.wikipedia.org/wiki/ISO_10303" .

sto:ISO_PAS_17506  a             owl:NamedIndividual , sto:Standard ;
        rdfs:comment             "SO/PAS 17506:2012 describes the COLLADA schema. COLLADA is a COLLAborative Design Activity that defines an XML-based schema to enable 3D authoring applications to freely exchange digital assets without loss of information, enabling multiple software packages to be combined into extremely powerful tool chains. The purpose of ISO/PAS 17506:2012 is to provide a specification for the COLLADA schema in sufficient detail to enable software developers to create tools to process COLLADA resources. In particular, it is relevant to those who import to or export from digital content creation (DCC) applications, 3D interactive applications and tool chains, prototyping tools, real-time visualization applications such as those used in the video game and movie industries, and CAD tools. ISO/PAS 17506:2012 covers the initial design and specifications of the COLLADA schema, as well as a minimal set of requirements for COLLADA exporters. "@en , "ISO-PAS 17506-2012 describes the COLLADA schema. COLLADA is a COLLAborative Design Activity that defines an XML-based schema to enable 3D authoring applications to freely exchange digital assets without loss of information, enabling multiple software packages to be combined into extremely powerful tool chains."@en ;
        rdfs:label               "ISO PAS 17506"@en ;
        dul:isComponentOf        sto:IEC_62714 ;
        sto:hasDBpediaResource   "http://dbpedia.org/resource/COLLADA" ;
        sto:hasDeveloper         sto:ISO ;
        sto:hasOfficialResource  "https://www.iso.org/standard/59902.html" ;
        sto:hasPublisher         sto:ISO ;
        sto:hasTag               "COLLADA"@en ;
        sto:hasWikipediaArticle  "https://en.wikipedia.org/wiki/COLLADA" .

dbr:Geneva  a   owl:NamedIndividual .

sto:IEC_29161  a                 sto:Standard , owl:NamedIndividual ;
        rdfs:comment             "ISO/IEC 29161:2016 establishes a unique identification scheme for the Internet of Things (IoT), based on existing and evolving data structures. This International Standard specifies the common rules applicable for unique identification that are required to ensure full compatibility across different identities. The unique identification is a universal construct for any physical object, virtual object, or person. It is used in IoT information systems that need to track or otherwise refer to entities. It is intended for use with any IoT media."@en ;
        rdfs:label               "IEC 29161"@en ;
        owl:sameAs               sto:ISO_29161 ;
        sto:hasDomain            "Automatic identification and data capture techniques"@en ;
        sto:hasOfficialResource  "https://www.iso.org/standard/45240.html" ;
        sto:hasPublicationDate   "2016-08-01"^^xsd:date ;
        sto:hasPublisher         sto:ISO , sto:IEC ;
        sto:hasTag               "Information technology -- Data structure -- Unique identification for the Internet of Things"@en .

sto:EnterpriseIntegration
        a       owl:NamedIndividual .

sto:TC_94  a          sto:TechnicalCommittee , owl:NamedIndividual ;
        rdfs:comment  "To prepare international standards applicable to all-or-nothing electrical relays used in the various fields of Electrical Engineering covered by the IEC, normally produced in very large\nnumbers as components of electromechanical or electronic\nequipment and eventually submitted to Quality Assurance requirements based on sampling techniques."@en , "To prepare international standards applicable to all-or-nothing\n\nelectrical relays used in the various fields of Electrical\nEngineering covered by the IEC, normally produced in very large\nnumbers as components of electromechanical or electronic\nequipment and eventually submitted to Quality Assurance\nrequirements based on sampling techniques."@en ;
        rdfs:label    "TC 94"@en ;
        sto:hasTitle  "All-or-nothing electrical relays"@en , "All-or-nothing electrical relays\n"@en .

sto:FileSizeIEC_61334_2001_P5_S1
        a                      om2:Measure , owl:NamedIndividual ;
        rdfs:comment           "Specifies the file size of the document for standard IEC 61334-5-1:2001"@en ;
        rdfs:label             "FileSize IEC 61334-5-1:2001"@en ;
        om2:hasNumericalValue  "723.0"^^xsd:float ;
        om2:hasUnit            om2:kilobyte .

dbr:Germany  a  owl:NamedIndividual .

sto:hasTask  a        owl:DatatypeProperty ;
        rdfs:comment  "Specifies the tasks for the different ISA 95 levels."@en ;
        rdfs:domain   sto:ISA95Level ;
        rdfs:label    "has Task"@en ;
        rdfs:range    xsd:string .

sto:hasTitle  a       owl:ObjectProperty , owl:DatatypeProperty ;
        rdfs:comment  "Gives Title of the Thing"@en ;
        rdfs:domain   sto:Publication ;
        rdfs:label    "has Title"@en ;
        rdfs:range    rdfs:literal .

sto:OMG_DDS  a                   owl:NamedIndividual , sto:Standard ;
        rdfs:comment             "The Data Distribution Service for real-time systems (DDS) is an Object Management Group (OMG) machine-to-machine (sometimes called middleware) standard that aims to enable scalable, real-time, dependable, high-performance and interoperable data exchanges using a publish–subscribe pattern. DDS addresses the needs of applications like financial trading, air-traffic control, smart grid management, and other big data applications. The standard is used in applications such as smartphone operating systems, transportation systems and vehicles, software-defined radio, and by healthcare providers. DDS was promoted for use in the Internet of things."@en ;
        rdfs:label               "OMG DDS"@en ;
        sto:hasDBpediaResource   "http://dbpedia.org/page/Data_Distribution_Service" ;
        sto:hasOfficialResource  "http://portals.omg.org/dds/" ;
        sto:hasPublisher         sto:OMG ;
        sto:hasTag               "Data Distribution Service for real-time systems"@en ;
        sto:hasWikipediaArticle  "https://en.wikipedia.org/wiki/Data_Distribution_Service" ;
        sto:relatedTo            sto:IEC_61158 .

sto:orgName  a        owl:DatatypeProperty ;
        rdfs:comment  "Name of the Organization"@en ;
        rdfs:domain   sto:StandardOrganization ;
        rdfs:label    "Org Name"@en ;
        rdfs:range    rdf:PlainLiteral .

sto:TC_1  a           owl:NamedIndividual , sto:TechnicalCommittee ;
        rdfs:comment  "To sanction the terms and definitions used in the different electrotechnical fields and to determine the equivalence of the terms used in the different languages. As a consequence, to prepare an International Electrotechnical Vocabulary aiming at the standardization and coordination of the terms relating to electrical sciences and techniques for use in the technical language and literature, in teaching, in technical specifications and in commercial exchanges, and at giving their equivalents in the different languages."@en ;
        rdfs:label    "TC 1"@en ;
        sto:hasTitle  "Terminology" .

sto:ICS_01_040_35  a  owl:NamedIndividual , sto:InternationalClassificationForStandards ;
        rdfs:comment  "This is ICS for  Information technology. Office machines (Vocabularies)"@en ;
        rdfs:label    "ICS 01.040.35"@en ;
        sto:hasTitle  " Information technology. Office machines (Vocabularies)"@en .

sto:ICS_33_040_40  a  owl:NamedIndividual , sto:InternationalClassificationForStandards ;
        rdfs:comment  "This is ICS for “Data communication networks”"@en ;
        rdfs:label    "ICS 33.040.40"@en ;
        sto:hasTitle  "Data communication networks "@en .

rami:LifeCycle_Status
        a       owl:NamedIndividual .

dbr:Switzerland  a  owl:NamedIndividual .

xsd:date  a     rdfs:Datatype .

rami:Asset  a              owl:NamedIndividual , rami:RAMIITLayer ;
        sto:isDescribedin  sto:RAMI40 .

sto:FileSizeIEC_60870_P5_S104_2016
        a                      om2:Measure , owl:NamedIndividual ;
        rdfs:comment           "Specifies the file size of the document for standard IEC 60870-5-104:2006"@en ;
        rdfs:label             "FileSize IEC 60870-5-104:2006"@en ;
        om2:hasNumericalValue  "2994.0"^^xsd:float ;
        om2:hasUnit            om2:kilobyte .

sto:ISO_19439  a                 owl:NamedIndividual , sto:Standard ;
        rdfs:comment             "Provides a unified conceptual basis for model-based enterprise engineering that enables consistency, convergence and interoperability of the various modelling methodologies and supporting tools."@en ;
        rdfs:label               "ISO 19439"@en ;
        sto:hasClassification    rami:Business ;
        sto:hasDBpediaResource   "http://dbpedia.org/page/ISO_19439" ;
        sto:hasOfficialResource  "https://www.iso.org/standard/33833.html" ;
        sto:hasPublisher         sto:ISO ;
        sto:hasTag               "19439"@en ;
        sto:hasWikipediaArticle  "https://en.wikipedia.org/wiki/ISO_19439" .

sto:ICS_31_240  a     owl:NamedIndividual , sto:InternationalClassificationForStandards ;
        rdfs:comment  "This is ICS for  Mechanical structures for electronic equipment"@en ;
        rdfs:label    "ICS 31.240"@en ;
        sto:hasTitle  "Mechanical structures for electronic equipment"@en .

rami:CommunicationSubModel
        a       owl:NamedIndividual .

om2:hasNumericalValue
        a       owl:AnnotationProperty .

sto:FileSizeIEC_60870_P6_S802_2014
        a                      om2:Measure , owl:NamedIndividual ;
        rdfs:comment           "Specifies the file size of the document for standard IEC 60870-6-802:2014"@en ;
        rdfs:label             "FileSize IEC 60870-6-802:2014"@en ;
        om2:hasNumericalValue  "1678.0"^^xsd:float ;
        om2:hasUnit            om2:kilobyte .

sto:StandardizationFramework
        a              owl:Class ;
        rdfs:comment   "Describes existings Standardizations Initiatives, e.g, RAMI, NIST."@en ;
        rdfs:label     "Standarization Framework"@en ;
        skos:altLabel  "Reference Architecture"@en .

sto:ProductModelDataExchange
        a                  owl:NamedIndividual , sto:ProductDevelopmentLifeCycle ;
        rdfs:comment       "These standards capture the representation of product and engineering information to enable data exchange between CAD software from different vendors."@en ;
        rdfs:label         "Product Model Data Exchange"@en ;
        sto:isDescribedin  sto:NISTInitiative .

sto:IEC_62890  a                 sto:Standard , owl:NamedIndividual ;
        rdfs:comment             "MES KPIs"@en , "Defines standards for lifecycle management for systems and products used in industrial process measurement, control and automation"@en ;
        rdfs:label               "IEC 62890"@en ;
        dcterms:hasLicense       "Private"@en ;
        sto:hasClassification    sto:ProductionLifeCycleDataManagement , rami:WorkCenter , rami:LifecycleStatus , rami:Station ;
        sto:hasMotivation        "Stations need to describe their operational state and performance parameters towards superior I4.0-Components"@en ;
        sto:hasOfficialResource  "http://www.iec.ch/dyn/www/f?p=103:38:16824039984463::::FSP_ORG_ID,FSP_APEX_PAGE,FSP_PROJECT_ID:1250,23,20929" ;
        sto:hasPublisher         sto:IEC ;
        sto:hasTag               "IEC 62890"@en .

sto:Standard  a             owl:Class , owl:NamedIndividual ;
        rdfs:comment        "Specifies that a given Publicaion is an International Standard"@en , "A document, established by consensus and approved by a recognized body, that provides, for common and repeated use, rules, guidelines or characteristics for activities or their results, aimed at the achievement of the optimum degree of order in a given context."@en ;
        rdfs:isDefinedBy    sto:IEC ;
        rdfs:label          "Standard"@en , "Standard" ;
        rdfs:seeAlso        <http://www.iec.ch/standardsdev/publications/is.htm> ;
        rdfs:subClassOf     sto:Publication ;
        cc:attributionName  "Copyright © 2016 IEC Geneva, Switzerland." ;
        cc:attributionURL   "http://www.iec.ch" ;
        owl:disjointWith    sto:StandardOrganization ;
        sto:abbreviation    "IS" .

sto:FileSizeIEC_60073_2002
        a                      owl:NamedIndividual , om2:Measure ;
        rdfs:comment           "Specifies the file size of the document for standard IEC 60073:2002"@en ;
        rdfs:label             "FileSize IEC 60073:2002"@en ;
        om2:hasNumericalValue  "525.0"^^xsd:float ;
        om2:hasUnit            om2:kilobyte .

sto:IEC_60870_P6_S702_2014
        a                          owl:NamedIndividual , sto:Standard ;
        rdfs:comment               "IEC 60870-6-702:2014 is a functional profile (FP) and defines the provision of the TASE.2 communications services between two control centre end systems. It is supported by the transport services implemented in accordance with transport-profiles defined for the type of network that interconnects the control centre end systems. The main changes with respect to the previous edition are listed below:\n- certain objects were moved from being normative to informative;\n- certain TASE.2 conformance blocks have been made out-of-scope. These changes were made in order to remove TASE.2 blocks that were seldom used and whose capabilities are typically implemented by some other means besides TASE.2. This was done to promote interoperability of implementations from an application perspective."@en ;
        rdfs:label                 "IEC 60870-6-702:2014"@en ;
        sto:hasAvailableLanguage   "English/French"@en ;
        sto:hasDBpediaResource     <null//dbpedia.org/resource/IEC_60870> , <https://dbpedia.org/resource/IEC_60870> ;
        sto:hasEdition             "2.0"^^xsd:float ;
        sto:hasFileSize            sto:FileSizeIEC_60870_P6_S702_2014 ;
        sto:hasICS                 sto:ICS_33_200 ;
        sto:hasOfficialResource    <null//webstore.iec.ch/publication/3768> , <https://webstore.iec.ch/publication/3768> ;
        sto:hasPages               "71"^^xsd:int ;
        sto:hasPublicationDate     "2014-07-196"^^xsd:date ;
        sto:hasPublisher           sto:IEC ;
        sto:hasStabilityDate       "2018"^^xsd:gYear ;
        sto:hasTag                 "IEC 60870-6-702:2014"@en ;
        sto:hasTechnicalCommittee  sto:TC_57 ;
        sto:hasTitle               "Telecontrol equipment and systems - Part 6-702: Telecontrol protocols compatible with ISO standards and ITU-T recommendations - Functional profile for providing the TASE.2 application service in end systems"@en ;
        sto:hasWikipediaArticle    <null//en.wikipedia.org/wiki/IEC_60870> , <https://en.wikipedia.org/wiki/IEC_60870> .

sto:hasOntology  a    owl:DatatypeProperty ;
        rdfs:comment  "Point to the URL of a recognized Ontology representation of the Standard"@en ;
        rdfs:domain   sto:Publication ;
        rdfs:label    "has Ontology"@en ;
        rdfs:range    xsd:anyURI .

sto:ISO_19440  a                 owl:NamedIndividual , sto:Standard ;
        rdfs:comment             "Enterprise integration -- Constructs for enterprise modelling-specifies the characteristics of the core constructs necessary for computer-supported modelling of enterprises conforming to ISO 19439.."@en ;
        rdfs:label               "ISO 19440"@en ;
        sto:hasClassification    sto:Product , sto:EnterpriseLevel , rami:Engineering , rami:Enterprise , rami:Integration ;
        sto:hasDomain            sto:EnterpriseIntegration ;
        sto:hasOfficialResource  "https://www.iso.org/standard/33834.html" ;
        sto:hasPublicationDate   "2007-12-01"^^xsd:date ;
        sto:hasPublisher         sto:ISO ;
        sto:relatedTo            sto:BPMN .

sto:TechnicalSpecification
        a                  owl:NamedIndividual , owl:Class ;
        rdfs:comment       "Specifies that a given Publication is a Technical Specification"@en , "Technical Specifications are often published when the subject under question is still under development or when insufficient consensus for approval of an International Standard is available.Technical Specifications approach International Standards in terms of detail and completeness, but have not yet passed through all approval stages either because consensus has not been reached or because standardization is seen to be premature."@en ;
        rdfs:isDefinedBy   sto:IEC ;
        rdfs:label         "Technical Specification"@en , "Technical Specification" ;
        rdfs:seeAlso       <http://www.iec.ch/standardsdev/publications/ts.htm> ;
        rdfs:subClassOf    sto:Publication ;
        cc:attributionURL  "http://www.iec.ch" ;
        sto:abbreviation   "TS" .

<http://dbpedia.org/resource#Washington,_D.C.>
        a       owl:NamedIndividual .

sto:DeviceLevel  a    owl:NamedIndividual , sto:ISA95Level ;
        rdfs:comment  "Describes the device level according to the ISA95 level classification."@en ;
        rdfs:label    "Device Level"@en .

sto:IEC_60839_P7_6  a              sto:Standard , owl:NamedIndividual ;
        rdfs:comment               "Specifies the requirements for standard interfaces employing ITU-T V.24/V.28 signalling for communications between the control and indicating equipment of an alarm system and transmission equipment used for remote communications, where the transmission equipment is general purpose equipment. Is intended to be used as interfacing to standard modems, packet switching networks, X.25 PADs, etc."@en ;
        rdfs:label                 "IEC 60839-7-6:2001"@en ;
        sto:hasAvailableLanguage   "English"@en , " English/French"@en ;
        sto:hasEdition             "1.0"^^xsd:float ;
        sto:hasFileSize            sto:FileSizeIEC_60839_P7_6 ;
        sto:hasICS                 sto:ICS_13_320 ;
        sto:hasOfficialResource    <null//webstore.iec.ch/publication/3674> ;
        sto:hasPages               "9"^^xsd:int ;
        sto:hasPublicationDate     "68/03/01"^^xsd:date ;
        sto:hasPublisher           sto:IEC ;
        sto:hasStabilityDate       "2018"^^xsd:gYear ;
        sto:hasTag                 "IEC 60839-7-6:2001"@en ;
        sto:hasTechnicalCommittee  sto:TC_79 ;
        sto:hasTitle               "Alarm systems - Part 7-6: Message formats and protocols for serial data interfaces in alarm transmission systems - Alarm system interfaces employing ITU-T Recommendation V.24/V.28 signalling"@en .

sto:ICS_29_240_20  a  owl:NamedIndividual , sto:InternationalClassificationForStandards ;
        rdfs:comment  "This is ICS for “Power transmission and distribution lines”"@en ;
        rdfs:label    "ICS 29.240.20"@en ;
        sto:hasTitle  "Power transmission and distribution lines"@en .

sto:FileSizeIEC_60839_P7_2
        a                      om2:Measure , owl:NamedIndividual ;
        rdfs:comment           "Specifies the file size of the document for standard IEC 60839-7-2:2001"@en ;
        rdfs:label             "FileSize IEC 60839-7-2:2001"@en ;
        om2:hasNumericalValue  "1047.0"^^xsd:float ;
        om2:hasUnit            om2:kilobyte .

sto:IEC_60870  a                 owl:NamedIndividual , sto:Standard ;
        rdfs:comment             "In electrical engineering and power system automation, the IEC 60870 series define systems used for telecontrol (supervisory control and data acquisition)"@en ;
        rdfs:label               "IEC 60870"@en ;
        sto:hasDBpediaResource   "http://dbpedia.org/page/IEC_60870" ;
        sto:hasPublisher         sto:IEC ;
        sto:hasWikipediaArticle  "https://en.wikipedia.org/wiki/IEC_60870" .

sto:FileSizeIEC_61334_2000_P4_S511
        a                      om2:Measure , owl:NamedIndividual ;
        rdfs:comment           "Specifies the file size of the document for standard IEC 61334-4-511:2000"@en ;
        rdfs:label             "FileSize IEC 61334-4-511:2000"@en ;
        om2:hasNumericalValue  "203.0"^^xsd:float ;
        om2:hasUnit            om2:kilobyte .

sto:IEC_61010_P2_S201_2017
        a                          sto:Standard , owl:NamedIndividual ;
        rdfs:comment               "\nIEC 61010-2-201:2017 RLV contains the International Standard and its Redline version. The Redline version is available in English only. The Redline version provides you with a quick and easy way to compare all the changes between this standard and its previous edition. The Redline version is not an official IEC Standard, only the current version of the standard is to be considered the official document.\n\nIEC 61010-2-201:2017 specifies safety requirements and related verification tests for any product performing the function of control equipment and/or their associated peripherals. In addition, these products have as their intended use the command and control of machines, automated manufacturing and industrial processes, e.g. discrete and continuous control.\nThis second edition cancels and replaces the first edition published in 2013. This edition constitutes a technical revision. This second edition includes the following significant technical changes with respect to the previous edition;\na) clarify, change, delete definitions which were causing confusion,\nb) change and clarify the temperature testing methodology,\nc) change documentation methodologies allowed,\nd) change some terminal markings,\ne) add clarity to some of the informative annexes,\nf) add Annex E with changes,\ng) add Annexes AA – FF."@en ;
        rdfs:label                 "IEC 61010-2-201:2017"@en ;
        sto:hasAvailableLanguage   "English"@en ;
        sto:hasEdition             "2.0"^^xsd:float ;
        sto:hasFileSize            sto:FileSizeIEC_61010_P2_S201_2017 ;
        sto:hasICS                 sto:19_020 , sto:ICS_17_020 , sto:ICS_25_040_40 ;
        sto:hasOfficialResource    <https://webstore.iec.ch/publication/60204> , <null//webstore.iec.ch/publication/60204> ;
        sto:hasPages               "235"^^xsd:int ;
        sto:hasPublicationDate     "2017-03-83"^^xsd:date ;
        sto:hasPublisher           sto:IEC ;
        sto:hasStabilityDate       "2020"^^xsd:gYear ;
        sto:hasTag                 "IEC 61010-2-201:2017"@en ;
        sto:hasTechnicalCommittee  sto:TC_65 ;
        sto:hasTitle               "Safety requirements for electrical equipment for measurement, control, and laboratory use - Part 2-201: Particular requirements for control equipment"@en .

sto:TC_88  a          sto:TechnicalCommittee , owl:NamedIndividual ;
        rdfs:comment  "TC 88 standardization in the field of wind energy generation systems including wind turbines, wind power plants onshore and offshore and interaction with the electrical system(s) to which energy is supplied.\n\nThese standards address site suitability and resource assessment, design\nrequirements, engineering integrity, modeling requirements, measurement techniques, test procedures, operation and maintenance. Their purpose is to provide a basis for design, quality assurance and technical aspects for certification. The standards address site-specific conditions, all systems and subsystems of wind turbines and wind power plants, such as mechanical, and electrical systems, support structures, control and protection as well as communication systems for monitoring, centralized and distributed control and evaluation, implementation of grid connection requirements for wind power plants, and environmental aspects of wind power development. The TC 88 standards will be developed based on and in agreement with appropriate IEC/ISO standards."@en , "TC 88\nStandardization in the field of wind energy generation systems including wind turbines, wind power plants onshore and offshore and interaction with the electrical system(s) to which energy is supplied.\n\nThese standards address site suitability and resource assessment, design\nrequirements, engineering integrity, modeling requirements, measurement techniques, test procedures, operation and maintenance. Their purpose is to provide a basis for design, quality assurance and technical aspects for certification. The standards address site-specific conditions, all systems and subsystems of wind turbines and wind power plants, such as mechanical, and electrical systems, support structures, control and protection as well as\ncommunication systems for monitoring, centralized and distributed control and evaluation, implementation of grid connection requirements for wind power plants, and environmental aspects of wind power development. The TC 88 standards will be developed based on and in agreement with appropriate IEC/ISO standards."@en ;
        rdfs:label    "TC 88"@en ;
        sto:hasTitle  "Wind energy generation systems"@en , "Wind energy generation systems\n"@en .

sto:OAGi  a                      owl:NamedIndividual , sto:StandardOrganization ;
        rdfs:comment             "The Open Applications Group is a not-for-profit standards development organization. Founded in 1994, is focused on building enterprise ready process-based data exchange standards for both B2B and A2A integration."@en ;
        rdfs:label               "OAGi"@en ;
        sto:abbreviation         "OAGi" ;
        sto:formationDate        "1994-01-01"^^xsd:date ;
        sto:hasHeadquaterIn      dbr:_Georgia ;
        sto:hasOfficialResource  "http://www.oagi.org/dnn2/Home.aspx" ;
        sto:orgName              "Open Applications Group"@en .

sto:W3C_RIF  a                   owl:NamedIndividual , sto:Standard ;
        rdfs:comment             "The Rule Interchange Format (RIF) is a W3C Recommendation. RIF is part of the infrastructure for the semantic web, along with (principally) SPARQL, RDF and OWL. Although originally envisioned by many as a rules layer for the semantic web, in reality the design of RIF is based on the observation that there are many rules languages in existence, and what is needed is to exchange rules between them."@en ;
        rdfs:label               "Rule Interchange Format"@en ;
        dcterms:hasLicense       "Public"@en ;
        sto:hasDBpediaResource   "http://dbpedia.org/resource/Rule_Interchange_Format" ;
        sto:hasOfficialResource  "https://www.w3.org/TR/rif-overview/" ;
        sto:hasPublisher         sto:W3C ;
        sto:hasTag               "RIF"@en ;
        sto:hasWikipediaArticle  "https://en.wikipedia.org/wiki/Rule_Interchange_Format" ;
        sto:relatedTo            sto:W3C_OWL .

sto:ICS_19_08  a      sto:InternationalClassificationForStandards , owl:NamedIndividual ;
        rdfs:comment  "This is ICS for “Electrical and electronic testing”"@en ;
        rdfs:label    "ICS 19.08"@en ;
        sto:hasTitle  "Electrical and electronic testing"@en .

sto:ISO_13849  a                 owl:NamedIndividual , sto:Standard ;
        rdfs:comment             "Provides safety requirements and guidance on the principles for the design and integration of safety-related parts of control systems (SRP/CS), including the design of software."@en ;
        rdfs:label               "ISO 13849"@en ;
        sto:hasClassification    rami:Safety ;
        sto:hasDBpediaResource   "http://dbpedia.org/resource/ISO_13849" ;
        sto:hasDomain            "Safety of machinery"@en ;
        sto:hasOfficialResource  "http://www.iso.org/iso/home/store/catalogue_tc/catalogue_detail.htm?csnumber=69883" ;
        sto:hasPublisher         sto:ISO ;
        sto:hasWikipediaArticle  "https://en.wikipedia.org/wiki/ISO_13849" .

sto:ISO_15459  a  owl:NamedIndividual .

sto:DIN  a                       owl:NamedIndividual , sto:StandardOrganization ;
        rdfs:comment             "Deutsches Institut für Normung e.V. (DIN; in English, the German Institute for Standardization) is the German national organization for standardization and is the German ISO member body. DIN is a German Registered Association (e.V.) headquartered in Berlin. There are currently around thirty thousand DIN Standards, covering nearly every field of technology"@en ;
        rdfs:label               "Deutsches Institut für Normung"@de , "German Institute for Standardization"@en ;
        sto:abbreviation         "DIN"@de ;
        sto:belongsTo            dbr:Germany ;
        sto:formationDate        "1918-01-01"^^xsd:date ;
        sto:hasDBpediaResource   <http://dbpedia.org/page/Deutsches_Institut_f%C3%BCr_Normung> ;
        sto:hasHeadquaterIn      dbr:Berlin ;
        sto:hasOfficialResource  <http://www.din.de/en/about-standards/din-standards> ;
        sto:hasWikipediaArticle  <https://en.wikipedia.org/wiki/Deutsches_Institut_f%C3%BCr_Normung> ;
        sto:orgName              "Deutsches Institut für Normung"@en .

sto:ISO_50001  a                 owl:NamedIndividual , sto:Standard ;
        rdfs:comment             "Energy management systems – Requirements with guidance for use is a specification created by the International Organization for Standardization (ISO) for an energy management system."@en ;
        rdfs:label               "ISO 50001"@en ;
        sto:hasClassification    sto:CrossLevel ;
        sto:hasDBpediaResource   "http://dbpedia.org/page/ISO_50001" ;
        sto:hasOfficialResource  "https://www.iso.org/iso-50001-energy-management.html" ;
        sto:hasPublisher         sto:ISO .

sto:IEC_60286_5_2018  a              owl:NamedIndividual , sto:Standard ;
        rdfs:comment                 "IEC 60286-5:2018 RLV contains the International Standard and its Redline version. The Redline version is available in English only. The Redline version provides you with a quick and easy way to compare all the changes between this standard and its previous edition. The Redline version is not an official IEC Standard, only the current version of the standard is to be considered the official document.IEC 60286-5:2018 describes the common dimensions, tolerances and characteristics of the tray. It includes only those dimensions that are essential for the handling of the trays for the stated purpose and for placing or removing components from the trays. This edition includes the following significant technical changes with respect to the previous edition: - The generic rules for the design of matrix trays are given in this document. Newly developed trays which follow these rules will not be listed individually. Only those trays which conform to the design rules set forth herein are classified as 'standard trays' and are thus preferred for use.- An update of the matrix trays, which do not conform to the design rules set forth herein, are considered as 'non-standard trays' and are not preferred for use, is listed in Annex A."@en ;
        rdfs:label                   "IEC 60286-5:2018"@en ;
        sto:hasAvailableLanguage     "English"@en ;
        sto:hasEdition               "3.0"^^xsd:float ;
        sto:hasFileSize              sto:FileSizeIEC_60286_5_2018 ;
        sto:hasICS                   sto:ICS_31_020 ;
        sto:hasImplementationFormat  "Document"@en ;
        sto:hasOfficialResource      <https://webstore.iec.ch/publication/63037> ;
        sto:hasPages                 71 ;
        sto:hasPublicationDate       "2018-04-25"^^xsd:date ;
        sto:hasPublisher             sto:IEC ;
        sto:hasStabilityDate         "2024"^^xsd:gYear ;
        sto:hasStatus                "RLV-Redline version"@en ;
        sto:hasTag                   "IEC 60286-5:2018"@en ;
        sto:hasTechnicalCommittee    sto:TC_40 ;
        sto:hasTitle                 "Packaging of components for automatic handling - Part 5: Matrix trays"@en .

sto:ISO_15531-4x  a        owl:NamedIndividual , sto:StandardPart ;
        rdfs:comment       "Manufacturing flow management data : refering to the material flow control and aiming at the representation of data and elements supporting the control and monitoring of the flow of materials in manufacturing processes."@en ;
        rdfs:isDefinedBy   "https://www.researchgate.net/publication/220171079_ISO_15531_MANDATE_a_standardised_data_model_for_manufacturing_management" ;
        rdfs:label         "ISO 15531 4x series"@en ;
        dul:isComponentOf  sto:ISO_15531 .

rami:Product  a            owl:NamedIndividual , rami:RAMIHierarchyLevel ;
        sto:isDescribedin  sto:RAMI40 .

sto:MTConnect  a                 sto:Standard , owl:NamedIndividual ;
        rdfs:comment             "MTConnect is a protocol designed for the exchange of data between shop floor equipment and software applications used for monitoring and data analysis. MTConnect is referred to as a read-only standard, meaning that it only defines the extraction (reading) of data from control devices, not the writing of data to a control device. Freely available, open standards are used for all aspects of MTConnect. Data from shop floor devices is presented in XML format, and is retrieved from information providers, called Agents, using Hypertext Transfer Protocol (HTTP) as the underlying transport protocol. MTConnect provides a RESTful interface, which means the interface is stateless. No session must be established to retrieve data from an MTConnect Agent, and no logon or logoff sequence is required (unless overlying security protocols are added which do). Lightweight Directory Access Protocol (LDAP) is recommended for discovery services."@en ;
        rdfs:label               "MTConnect"@en ;
        sto:hasClassification    sto:DeviceLevel ;
        sto:hasDBpediaResource   "http://dbpedia.org/resource/MTConnect" ;
        sto:hasDeveloper         sto:MTConnect_Institute ;
        sto:hasOfficialResource  "http://www.mtconnect.org/standard-documents" ;
        sto:hasPublisher         sto:MTConnect_Institute ;
        sto:hasTag               "MTConnect"@en ;
        sto:hasWikipediaArticle  "https://en.wikipedia.org/wiki/MTConnect" .

sto:QIF  a                       owl:NamedIndividual , sto:Standard ;
        rdfs:comment             " Quality Information Framework (QIF) standard defines an integrated set of information models which enable the effective exchange of metrology data throughout the entire manufacturing quality measurement process"@en ;
        rdfs:isDefinedBy         "http://qifstandards.org/about-qif/" ;
        rdfs:label               "Quality Information Framework"@en ;
        skos:note                "Is implemented in XML" ;
        sto:hasOfficialResource  "http://qifstandards.org/" ;
        sto:hasPublisher         sto:DMSC .

sto:IEC_61334  a                 owl:NamedIndividual , sto:Standard ;
        rdfs:comment             "IEC 61334 , known as Distribution automation using distribution line carrier systems, is a standard for low-speed reliable power line communications by electricity meters, water meters and SCADA."@en ;
        rdfs:label               "IEC 61334"@en ;
        sto:hasDBpediaResource   "http://dbpedia.org/page/IEC_61334" ;
        sto:hasOfficialResource  "https://webstore.iec.ch/publication/5308" ;
        sto:hasPublisher         sto:IEC .

sto:ISO_13584  a                 sto:Standard , owl:NamedIndividual ;
        rdfs:comment             "ISO 13584 is a series of International Standards for the computer-sensible representation and exchange of parts library data. The objective is to provide a mechanism capable of transferring parts library data, independent from any particular system. The nature of this description makes it suitable not only for the exchange of files containing parts libraries, but also as a basis for implementing and sharing databases of parts library data, and archiving"@en ;
        rdfs:label               "ISO 13584"@en ;
        dcterms:hasLicense       "Private"@en ;
        sto:hasClassification    sto:ProductCatalogData ;
        sto:hasDBpediaResource   "http://dbpedia.org/resource/ISO_13584" ;
        sto:hasMotivation        "Standard data elements (properties) are used as elements in administration shell"@en ;
        sto:hasOfficialResource  "https://webstore.iec.ch/publication/5380%0Ahttp://www.iso.org/iso/catalogue_detail.htm?csnumber=43423" ;
        sto:hasPublisher         sto:ISO ;
        sto:hasTag               "Industrial automation systems and integration"@en ;
        sto:hasWikipediaArticle  "https://en.wikipedia.org/wiki/ISO_13584" ;
        sto:relatedTo            sto:IEC_61360 , sto:eClass .

sto:Configuration  a       owl:NamedIndividual , rami:AdminShellSubmodel ;
        sto:isDescribedin  sto:AdministrationShell .

rami:Safety  a             owl:NamedIndividual , rami:AdminShellSubmodel ;
        sto:isDescribedin  sto:AdministrationShell .

sto:FileSizeIEC_61334_2000_P6
        a                      om2:Measure , owl:NamedIndividual ;
        rdfs:comment           "Specifies the file size of the document for standard IEC 61334-6:2000"@en ;
        rdfs:label             "FileSize IEC 61334-6:2000"@en ;
        om2:hasNumericalValue  "294.0"^^xsd:float ;
        om2:hasUnit            om2:kilobyte .

dul:isMemberOf  a  owl:AnnotationProperty .

skos:prefLabel  a  owl:AnnotationProperty .

sto:hasAvailableLanguage
        a                   owl:ObjectProperty ;
        rdfs:comment        "Languages in which the document of the Standard is available, e.g., English, French, Spanish"@en ;
        rdfs:domain         foaf:Document ;
        rdfs:label          "has Available Language"@en ;
        rdfs:subPropertyOf  dcterms:language ;
        skos:note           "dcterms:language  rdfs:range dcterms:LinguisticSystem.\n                         " .

sto:IEC_60381_1978  a                sto:Standard , owl:NamedIndividual ;
        rdfs:comment                 "Applicable to analogue direct voltage signals used in industrial process measurement and control systems. lt specifies ranges of analogue direct voltage signals and the signal common; it also deals with ripple content. The analogue direct voltage signal, unlike the analogue direct current signal specified in IEC 60381-1, is not intended for transmission over long distances. This standard does not apply to signals used entirely within an element."@en ;
        rdfs:label                   "IEC 60381-2:1978"@en ;
        sto:hasAvailableLanguage     "English/French, Russian"@en ;
        sto:hasEdition               "1.0"^^xsd:float ;
        sto:hasFileSize              sto:FileSizeIEC_60381_1978 ;
        sto:hasICS                   sto:ICS_33_200 , sto:ICS_35_240_50 ;
        sto:hasImplementationFormat  "Document"@en ;
        sto:hasOfficialResource      <https://webstore.iec.ch/publication/1949> ;
        sto:hasPages                 9 ;
        sto:hasPublicationDate       "1978-01-01"^^xsd:date ;
        sto:hasPublisher             sto:IEC ;
        sto:hasStabilityDate         "2018"^^xsd:gYear ;
        sto:hasStatus                "Valid"@en ;
        sto:hasTag                   "IEC 60381-2:1978"@en ;
        sto:hasTechnicalCommittee    sto:TC_65 ;
        sto:hasTitle                 "Analogue signals for process control systems. Part 2: Direct voltage signals"@en .

sto:IEC_60870_P5_S2_1992
        a                          sto:Standard , owl:NamedIndividual ;
        rdfs:comment               "Applies to telecontrol equipment and systems with coded bit serial data transmission for monitoring and controlling geographically widespread processes. \nThis publication is of high relevance for Smart Grid."@en ;
        rdfs:label                 "IEC 60870-5-2:1992"@en ;
        sto:hasAvailableLanguage   "English"@en , " English/French"@en ;
        sto:hasDBpediaResource     <null//dbpedia.org/resource/IEC_60870> , <https://dbpedia.org/resource/IEC_60870> ;
        sto:hasEdition             "1.0"^^xsd:float ;
        sto:hasFileSize            sto:FileSizeIEC_60870_1992_P5_S2 ;
        sto:hasICS                 sto:ICS_33_200 ;
        sto:hasOfficialResource    <null//webstore.iec.ch/publication/3747> , <https://webstore.iec.ch/publication/3747> ;
        sto:hasPages               "99"^^xsd:int ;
        sto:hasPublicationDate     "1992-04-121"^^xsd:date ;
        sto:hasPublisher           sto:IEC ;
        sto:hasStabilityDate       "2018"^^xsd:gYear ;
        sto:hasTag                 "IEC 60870-5-2:1992"@en ;
        sto:hasTechnicalCommittee  sto:TC_57 ;
        sto:hasTitle               "Telecontrol equipment and systems - Part 5: Transmission protocols - Section 2: Link transmission procedures"@en ;
        sto:hasWikipediaArticle    <null//en.wikipedia.org/wiki/IEC_60870> , <https://en.wikipedia.org/wiki/IEC_60870> .

sto:InternationalClassificationForStandards
        a                 owl:Class , owl:NamedIndividual ;
        rdfs:comment      "Serves as a structure for catalogues of international, regional and national standards and other normative documents, and as a basis for standing-order systems."@en ;
        rdfs:label        "International Classification For Standards"@en ;
        rdfs:seeAlso      <https://www.iso.org/publication/PUB100033.html> ;
        sto:abbreviation  "ICS"@en .

sto:FileSizeIEC_60255_2009
        a                      owl:NamedIndividual , om2:Measure ;
        rdfs:comment           "Specifies the file size of the document for standard 60255-1:2009"@en ;
        rdfs:label             "FileSize IEC 60255-1:2009"@en ;
        om2:hasNumericalValue  "1411.0"^^xsd:float ;
        om2:hasUnit            om2:kilobyte .

sto:ISA-95  a                    sto:Standard , owl:NamedIndividual ;
        rdfs:comment             "ANSI/ISA-95, or ISA-95 as it is more commonly referred, is an international standard from the International Society of Automation for developing an automated interface between enterprise and control systems. This standard has been developed for global manufacturers. It was developed to be applied in all industries, and in all sorts of processes, like batch processes, continuous and repetitive processes.There are 5 parts of the ISA-95 standard.ISA-95 Models"@en ;
        rdfs:label               "ISA 95"@en ;
        sto:hasDBpediaResource   "http://dbpedia.org/resource/ANSI/ISA-95" ;
        sto:hasDeveloper         sto:ISA , sto:ANSI ;
        sto:hasOfficialResource  "https://www.isa.org/isa95/" ;
        sto:hasPublisher         sto:ANSI , sto:ISA ;
        sto:hasTag               "Enterprise-Control System Integration"@en ;
        sto:hasWikipediaArticle  "https://en.wikipedia.org/wiki/ANSI/ISA-95" .

rami:RAMILifeCycleLayer
        a                owl:Class ;
        rdfs:label       "RAMI Life Cycle Layer"@en ;
        rdfs:seeAlso     "http://www.zvei.org/en/subjects/Industry-40/Pages/The-Reference-Architectural-Model-RAMI-40-and-the-Industrie-40-Component.aspx" ;
        rdfs:subClassOf  sto:StandardClassification ;
        skos:definition  "It describes the different Life Cycle and Value Stream layers for the RAMI model according to the IEC 62890 Standard."@en ;
        skos:prefLabel   "RAMI Life Cycle Layer"@en .

sto:FileSizeIEC_61690_P1_2000
        a                      om2:Measure , owl:NamedIndividual ;
        rdfs:comment           "Specifies the file size of the document for standard IEC 61690-1:2000 ."@en ;
        rdfs:label             "FileSize IEC 61690-1:2000 "@en ;
        om2:hasNumericalValue  "1676.0"^^xsd:float ;
        om2:hasUnit            om2:kilobyte .

dbo:Place  a    owl:Class .

sto:IIRC  a               owl:NamedIndividual , sto:StandardizationFramework ;
        rdfs:comment      "Industrial Internet Connectivity Framework"@en ;
        rdfs:isDefinedBy  "https://www.iiconsortium.org/IICF.htm"@en ;
        rdfs:label        "IICF"@en ;
        rdfs:seeAlso      "https://www.iiconsortium.org/pdf/IIC_PUB_G5_V1.01_PB_20180228.pdf" .

sto:ASME  a                      sto:StandardOrganization , owl:NamedIndividual ;
        rdfs:comment             "The American Society of Mechanical Engineers (ASME) is a professional association that, promotes the art, science, and practice of multidisciplinary engineering and allied sciences around the globe via continuing education, training and professional development, codes and standards, research, conferences and publications, government relations, and other forms of outreach."@en ;
        sto:abbreviation         "ASME" ;
        sto:formationDate        "1880-01-01"^^xsd:date ;
        sto:hasDBpediaResource   <http://dbpedia.org/resource/ASME> ;
        sto:hasHeadquaterIn      dbr:New_York_City ;
        sto:hasOfficialResource  <https://www.asme.org/> ;
        sto:hasWikipediaArticle  <https://en.wikipedia.org/wiki/ASME> ;
        sto:orgName              "American Society of Mechanical Engineers"@en .

sto:IBM  a                       owl:NamedIndividual , sto:StandardOrganization ;
        rdfs:comment             "International Business Machines Corporation (commonly referred to as IBM) is an American multinational technology and consulting corporation, with corporate headquarters in Armonk, New York. IBM manufactures and markets computer hardware, middleware and software, and offers infrastructure, hosting and consulting services in areas ranging from mainframe computers to nanotechnology.On August 6, 2015, IBM announced that it will buy Merge Healthcare Inc for $1 billion." ;
        sto:abbreviation         "IBM" ;
        sto:formationDate        "1911-06-16"^^xsd:date ;
        sto:hasDBpediaResource   <http://dbpedia.org/resource/IBM> ;
        sto:hasHeadquaterIn      dbr:_New_York ;
        sto:hasOfficialResource  <http://www.ibm.com> ;
        sto:hasWikipediaArticle  <https://en.wikipedia.org/wiki/IBM> ;
        sto:orgName              "International Business Machines Corporation"@en .

dbo:Country  a  owl:Class .

rami:Enterprise  a         owl:NamedIndividual , rami:RAMIHierarchyLevel ;
        sto:isDescribedin  sto:RAMI40 .

sto:VDMA_24582  a                owl:NamedIndividual , sto:Standard ;
        rdfs:comment             "Fieldbus neutral reference architecture for Condition Monitoring in production automation"@en ;
        rdfs:label               "VDMA 24582"@en ;
        sto:hasClassification    rami:ConditionMonitoring ;
        sto:hasOfficialResource  "https://www.vdma.org/documents/105628/2244593/Inhalt+VDMA+24582_en.pdf/" ;
        sto:hasPublisher         sto:VDMA ;
        sto:hasTag               "Condition Monitoring"@en .

owl:thing  a    owl:Class .

rdfs:literal  a  owl:Class .

sto:uses  a                 owl:ObjectProperty ;
        rdfs:comment        "Defines that Standard A uses Standard B. For example, IEC_62714(AML) uses MathML."@en ;
        rdfs:label          "uses"@en ;
        rdfs:subPropertyOf  sto:relatedTo .

sto:IEC_60864_P2  a                sto:Standard , owl:NamedIndividual ;
        rdfs:comment               "Deals with the itnerface between a transmitter (or system of transmitters) and the supervisory equipment which is entended to remotely monitor and/or control the transmitter(s). It details the interconnections and facilities to be provided with a view to achieving compatibility between different types and makes of transmitters and supervisory equipement."@en ;
        rdfs:label                 "IEC 60864-2:1997"@en ;
        sto:hasAvailableLanguage   "English/French"@en ;
        sto:hasEdition             "1.0"^^xsd:float ;
        sto:hasFileSize            <https://w3id.org/i40/sto#FileSizeIEC_60864_P2 > ;
        sto:hasICS                 sto:ICS_33_060_20 , sto:ICS_33_200 ;
        sto:hasOfficialResource    <null//webstore.iec.ch/publication/3728> ;
        sto:hasPages               "79"^^xsd:int ;
        sto:hasPublicationDate     "1997-06-168"^^xsd:date ;
        sto:hasPublisher           sto:IEC ;
        sto:hasStabilityDate       "2020"^^xsd:gYear ;
        sto:hasTag                 "IEC 60864-2:1997"@en ;
        sto:hasTechnicalCommittee  sto:TC_103 ;
        sto:hasTitle               "Standardization of interconnections between broadcasting transmitters or transmitter systems and supervisory equipment - Part 2: Interface standards for systems using data bus type interconnections"@en .

sto:FileSizeIEC_60255_2010
        a                      owl:NamedIndividual , om2:Measure ;
        rdfs:comment           "Specifies the file size of the document for standard IEC 60255-127:2010 "@en ;
        rdfs:label             "FileSize 60255-127:2010"@en ;
        om2:hasNumericalValue  "1215.0"^^xsd:float ;
        om2:hasUnit            om2:kilobyte .

sto:IEC_60839_P7_1  a              owl:NamedIndividual , sto:Standard ;
        rdfs:comment               "Describes the requirements for standard serial data interfaces in alarm transmission systems. Gives an outline of how alarm transmission systems are connected and the various types of serial data interfaces that might be employed."@en ;
        rdfs:label                 "IEC 60839-7-1:2001"@en ;
        sto:hasAvailableLanguage   " English/French"@en , "English"@en ;
        sto:hasEdition             "1.0"^^xsd:float ;
        sto:hasFileSize            sto:FileSizeIEC_60839_P7_1 ;
        sto:hasICS                 sto:ICS_13_320 ;
        sto:hasOfficialResource    <null//webstore.iec.ch/publication/3666> ;
        sto:hasPages               "39"^^xsd:int ;
        sto:hasPublicationDate     "68/03/01"^^xsd:date ;
        sto:hasPublisher           sto:IEC ;
        sto:hasStabilityDate       "2018"^^xsd:gYear ;
        sto:hasTag                 "IEC 60839-7-1:2001"@en ;
        sto:hasTechnicalCommittee  sto:TC_79 ;
        sto:hasTitle               "Alarm systems - Part 7-1: Message formats and protocols for serial data interfaces in alarm transmission systems – General"@en .

sto:ISO_11898-1  a               owl:NamedIndividual , sto:Standard ;
        rdfs:comment             "Used mainly for Road vehicles Controller area network (CAN) Data link layer and physical signalling."@en ;
        rdfs:label               "ISO 11898-1"@en ;
        sto:hasClassification    rami:Safety , rami:Communication , rami:Engineering ;
        sto:hasDBpediaResource   "http://dbpedia.org/page/CAN_bus" ;
        sto:hasDomain            sto:IndustrialAutomation ;
        sto:hasOfficialResource  "https://www.iso.org/standard/63648.html" ;
        sto:hasPublicationDate   "2015-12-01"^^xsd:date ;
        sto:hasPublisher         sto:ISO ;
        sto:hasTag               "CAN Bus"@en ;
        sto:relatedTo            sto:ISO_11783 .

sto:FileSizeIEC_60870_1995_P2_S1
        a                      om2:Measure , owl:NamedIndividual ;
        rdfs:comment           "Specifies the file size of the document for standard IEC 60870-2-1:1995"@en ;
        rdfs:label             "FileSize IEC 60870-2-1:1995"@en ;
        om2:hasNumericalValue  "1674.0"^^xsd:float ;
        om2:hasUnit            om2:kilobyte .

sto:ICS_33_060_20  a  owl:NamedIndividual , sto:InternationalClassificationForStandards ;
        rdfs:comment  "This is ICS for Receiving and transmitting equipment"@en ;
        rdfs:label    "ICS 33.060.20"@en ;
        sto:hasTitle  "Receiving and transmitting equipment"@en .

sto:IEC_61334_P4_S512_2001
        a                          owl:NamedIndividual , sto:Standard ;
        rdfs:comment               "Specifies the Management Information Base (MIB), which is used for the management of the communication profile defined by the following standards: IEC 61334-5-1, IEC 61334-4-32, IEC 61334-4-42, and IEC 61334-4-41.\nThis publication is of high relevance for Smart Grid."@en ;
        rdfs:label                 "IEC 61334-4-512:2001"@en ;
        sto:hasAvailableLanguage   "English/French"@en ;
        sto:hasDBpediaResource     <https://dbpedia.org/resource/IEC_61334> , <null//dbpedia.org/resource/IEC_61334> ;
        sto:hasEdition             "1.0"^^xsd:float ;
        sto:hasFileSize            sto:FileSizeIEC_61334_2001_P4_S512 ;
        sto:hasICS                 sto:ICS_33_200 ;
        sto:hasOfficialResource    <null//webstore.iec.ch/publication/5306> , <https://webstore.iec.ch/publication/5306> ;
        sto:hasPages               "47"^^xsd:int ;
        sto:hasPublicationDate     "2001-10-303"^^xsd:date ;
        sto:hasPublisher           sto:IEC ;
        sto:hasStabilityDate       "2018"^^xsd:gYear ;
        sto:hasTag                 "IEC 61334-4-512:2001"@en ;
        sto:hasTechnicalCommittee  sto:TC_57 ;
        sto:hasTitle               "Distribution automation using distribution line carrier systems - Part 4-512: Data communication protocols - System management using profile 61334-5-1 - Management Information Base (MIB)"@en ;
        sto:hasWikipediaArticle    <null//en.wikipedia.org/wiki/IEC_61334> , <https://en.wikipedia.org/wiki/IEC_61334> .

dbr:United_States  a  owl:NamedIndividual .

sto:IEC_60050_1984  a                sto:Standard , owl:NamedIndividual ;
        rdfs:comment                 "Terms on telecontrol, teleprotection and associated telecommunications for electric power systems. It has the status of a horizontal standard in accordance with IEC Guide 108."@en ;
        rdfs:label                   "IEC 60050-371:1984"@en ;
        sto:hasAvailableLanguage     "EN-FR-RU"@en ;
        sto:hasEdition               "1.0"^^xsd:float ;
        sto:hasFileSize              sto:FileSizeIEC_60050_1984 ;
        sto:hasICS                   sto:ICS_01_040_35 , sto:ICS_35_240_50 ;
        sto:hasImplementationFormat  "Document"@en ;
        sto:hasOfficialResource      <https://webstore.iec.ch/publication/196> ;
        sto:hasPages                 44 ;
        sto:hasPublicationDate       "1984-11-30"^^xsd:date ;
        sto:hasPublisher             sto:IEC ;
        sto:hasStatus                "Valid"@en ;
        sto:hasTag                   "IEC 60050-371:1984"@en ;
        sto:hasTechnicalCommittee    sto:TC_1 ;
        sto:hasTitle                 "International Electrotechnical Vocabulary. Chapter 371: Telecontrol"@en .

sto:ICS_33_100_10  a  owl:NamedIndividual , sto:InternationalClassificationForStandards ;
        rdfs:comment  "This is ICS for “Emission”"@en ;
        rdfs:label    "ICS 33.100.10"@en ;
        sto:hasTitle  "Emission"@en .

dbr:South_Korea  a  owl:NamedIndividual .

prov:wasGeneratedBy  a      owl:ObjectProperty ;
        rdfs:comment        "Standard A has influences in Standard B. For example, IEC_61499 hasInfluenceIn IEC_61804-2(EDDL)"@en ;
        rdfs:isDefinedBy    "https://www.w3.org/TR/prov-o/#wasGeneratedBy"@en ;
        rdfs:label          "was Generated By"@en ;
        rdfs:subPropertyOf  sto:relatedTo .

sto:IEC_62541  a                 owl:NamedIndividual , sto:Standard ;
        rdfs:comment             "OPC Unified Architecture (OPC UA) is an industrial M2M communication protocol for interoperability developed by the OPC Foundation. It is the successor to Open Platform Communications (OPC). Although developed by the same organization, OPC UA differs significantly from its predecessor. The Foundation's goal for this project was to provide a path forward from the original OPC communications model (namely the Microsoft Windows only process exchange COM/DCOM) to a cross-platform service-oriented architecture (SOA) for process control, while enhancing security and providing an information model."@en ;
        rdfs:label               "IEC 62541"@en ;
        dcterms:hasLicense       "Open"@en ;
        dcterms:hasLicense       sto:GPLv2 ;
        sto:hasClassification    rami:ControlDevice , rami:Station , rami:Enterprise , sto:SCADALevel , rami:WorkCenter , sto:Communication , rami:ConnectedWorld , rami:FieldDevice , rami:Communication ;
        sto:hasDBpediaResource   "http://dbpedia.org/resource/OPC_Unified_Architecture" ;
        sto:hasDeveloper         sto:OPC_Foundation ;
        sto:hasDomain            sto:IndustrialAutomation ;
        sto:hasOfficialResource  "https://opcfoundation.org/about/opc-technologies/opc-ua/" ;
        sto:hasPublisher         sto:IEC ;
        sto:hasTag               "OPC UA"@en ;
        sto:hasWikipediaArticle  "https://en.wikipedia.org/wiki/OPC_Unified_Architecture" ;
        sto:relatedTo            sto:IEC_62714 , sto:IEC_61499 , sto:IEC_61850 ;
        sto:useStructureOf       sto:IEC_61804 .

sto:ICS_01_070  a     owl:NamedIndividual , sto:InternationalClassificationForStandards ;
        rdfs:comment  "This is ICS for Colour coding "@en ;
        rdfs:label    "ICS 01.070"@en ;
        sto:hasTitle  "Colour coding  "@en .

sto:FileSizeIEC_60038_2009
        a                      owl:NamedIndividual , om2:Measure ;
        rdfs:comment           "Specifies the file size of the document for standard IEC 60038:2009"@en ;
        rdfs:label             "FileSize IEC 60038:2009"@en ;
        om2:hasNumericalValue  "946.0"^^xsd:float ;
        om2:hasUnit            om2:kilobyte .

sto:hasEdition  a     owl:DatatypeProperty ;
        rdfs:comment  "Indicates the current Edition/Version number of the document."@en ;
        rdfs:domain   foaf:Document ;
        rdfs:label    "has Edition"@en ;
        rdfs:range    xsd:float .

sto:FileSizeIEC_60255_151_2009
        a                      owl:NamedIndividual , om2:Measure ;
        rdfs:comment           "Specifies the file size of the document for standard IEC IEC 60255-151:2009"@en ;
        rdfs:label             "FileSize IEC 60255-151:2009 "@en ;
        om2:hasNumericalValue  "1341.0"^^xsd:float ;
        om2:hasUnit            om2:kilobyte .

sto:ITSecurity  a   owl:NamedIndividual , sto:Domain ;
        rdfs:label  "IT Security"@en .

sto:BPEL  a                      owl:NamedIndividual , sto:Standard ;
        rdfs:comment             "The Web Services Business Process Execution Language (WS-BPEL), commonly known as BPEL Business Process Execution Language, is a standard executable language for specifying actions within business processes with web services."@en ;
        rdfs:label               "Business Process Execution Language"@en ;
        sto:hasClassification    sto:BusinessProcessExecution ;
        sto:hasDBpediaResource   "http://dbpedia.org/resource/Business_Process_Execution_Language" ;
        sto:hasOfficialResource  "https://www.oasis-open.org/committees/tc_home.php?wg_abbrev=wsbpel" ;
        sto:hasPublisher         sto:OASIS ;
        sto:hasTag               "BPEL"@en ;
        sto:hasWikipediaArticle  "https://en.wikipedia.org/wiki/Business_Process_Execution_Language" .

sto:TC_95  a          owl:NamedIndividual , sto:TechnicalCommittee ;
        rdfs:comment  "Standardisation of measuring relays and protection equipment used in various fields of electrical engineering covered by IEC, taking into a ccount combinations of devices to form schemes for power system protection including the control, monitoring and process interface equipment used with those systems.Excluded are the following:All devices covered by standards prepared by other IEC Technical Committees, for example instrument transformers (TC 38)."@en ;
        rdfs:label    "TC 95"@en ;
        sto:hasTitle  "Measuring relays and protection equipment"@en .

sto:IEC_60870_P6_S601_1994
        a                          owl:NamedIndividual , sto:Standard ;
        rdfs:comment               "Defines the functional profile which provides the connection-oriented transport service in an end system connected via permanent access to a packet switched data network.\nThis publication is of high relevance for Smart Grid."@en ;
        rdfs:label                 "IEC 60870-6-601:1994"@en ;
        sto:hasAvailableLanguage   "English/French"@en ;
        sto:hasDBpediaResource     <https://dbpedia.org/resource/IEC_60870> , <null//dbpedia.org/resource/IEC_60870> ;
        sto:hasEdition             "1.0"^^xsd:float ;
        sto:hasFileSize            sto:FileSizeIEC_60870_P6_S601_1994 ;
        sto:hasICS                 sto:ICS_33_200 ;
        sto:hasOfficialResource    <https://webstore.iec.ch/publication/3765> , <null//webstore.iec.ch/publication/3765> ;
        sto:hasPages               "25"^^xsd:int ;
        sto:hasPublicationDate     "1994-12-355"^^xsd:date ;
        sto:hasPublisher           sto:IEC ;
        sto:hasStabilityDate       "2018"^^xsd:gYear ;
        sto:hasTag                 "IEC 60870-6-601:1994"@en ;
        sto:hasTechnicalCommittee  sto:TC_57 ;
        sto:hasTitle               "Telecontrol equipment and systems - Part 6: Telecontrol protocol s compatible with ISO standards and ITU-T recommendations - Sect ion 601: Functional profile for providing the connection-oriente d transport service in an end system connected via permanent acc ess to a packet switched data network"@en ;
        sto:hasWikipediaArticle    <https://en.wikipedia.org/wiki/IEC_60870> , <null//en.wikipedia.org/wiki/IEC_60870> .

rami:Identification  a     owl:NamedIndividual , rami:AdminShellSubmodel ;
        sto:isDescribedin  sto:AdministrationShell .

foaf:maker  a   owl:ObjectProperty .

sto:TC_65  a          owl:NamedIndividual , sto:TechnicalCommittee ;
        rdfs:comment  "To prepare international standards for systems and elements used for industrial-process measurement and control concerning continuous and batch processes."@en , "To prepare international standards for systems and elements used for industrial-process measurement and control concerning continuous and batch processes.To co-ordinate the standardization of those features of related elements which affect suitability for integration into such systems. The work of standardization outlined above is to be carried out in the international fields for equipment and systems operating with electrical, pneumatic, hydraulic, mechanical or other systems of measurement and/or control."@en ;
        rdfs:label    "TC 65"@en ;
        sto:hasTitle  "Industrial-process measurement, control and automation"@en .

sto:VDMA  a                      owl:NamedIndividual , sto:StandardOrganization ;
        rdfs:comment             "The Mechanical Engineering Industry Association (Verband Deutscher Maschinen- und Anlagenbau – VDMA) has its headquarters in Frankfurt am Main, Germany, and represents around 3,200 members, making it the largest industry association in Europe. The Association represents the interests of the predominantly medium-sized companies in the mechanical engineering industry towards policymakers and society, as well as towards business, the scientific community, public authorities and the media. With more than one million employees and a turnover of around EUR 218 billion (2015), mechanical and plant engineering is Germany’s largest employer in the industrial sector.In addition, VDMA sees itself as a platform that provides its member companies with various networks where they can discuss technological challenges, interdisciplinary issues and many other topics." ;
        sto:abbreviation         "VDMA" ;
        sto:formationDate        "1892-11-15"^^xsd:date ;
        sto:hasDBpediaResource   "http://dbpedia.org/resource/VDMA" ;
        sto:hasHeadquaterIn      dbr:Frankfurt ;
        sto:hasOfficialResource  "http://www.vdma.org" ;
        sto:hasWikipediaArticle  "https://en.wikipedia.org/wiki/Mechanical_Engineering_Industry_Association" ;
        sto:orgName              "Verband Deutscher Maschinen- und Anlagenbau"@de , "Mechanical Engineering Industry Association"@en .

sto:FileSizeIEC_60382_1991
        a                      owl:NamedIndividual , om2:Measure ;
        rdfs:comment           "Specifies the file size of the document for standard IEC 60382:1991"@en ;
        rdfs:label             "FileSize IEC 60382:1991"@en ;
        om2:hasNumericalValue  "557.0"^^xsd:float ;
        om2:hasUnit            om2:kilobyte .

sto:ICS_25_040_40  a  owl:NamedIndividual , sto:InternationalClassificationForStandards ;
        rdfs:comment  "This is ICS for industrial process measurement and control"@en , "This is ICS for “Industrial process measurement and control”"@en ;
        rdfs:label    "ICS 25.040.40"@en ;
        sto:hasTitle  "Industrial process measurement and control"@en .

sto:ModelingPractice  a    owl:NamedIndividual , sto:ProductDevelopmentLifeCycle ;
        rdfs:comment       "Modeling practice standards define digital product-definition data practices for both two-dimensional (2D) drawings and three-dimensional (3D) models."@en ;
        rdfs:label         "Modeling Practice"@en ;
        sto:isDescribedin  sto:NISTInitiative .

sto:IEC_TS_62237  a              owl:NamedIndividual , sto:Standard ;
        rdfs:comment             "Live working - Insulating hoses with fittings for use with hydraulic tools and equipment."@en ;
        rdfs:label               "IEC 62237"@en ;
        sto:hasClassification    sto:ProductionSystemModelData , rami:GeneralAdminShell , rami:FieldDevice , rami:WorkCenter , rami:Station , rami:ControlDevice ;
        sto:hasDomain            sto:IndustrialAutomation ;
        sto:hasOfficialResource  "https://webstore.iec.ch/publication/6626" ;
        sto:hasPublicationDate   "2003-10-26"^^xsd:date ;
        sto:hasPublisher         sto:IEC ;
        sto:relatedTo            sto:IEC_62337 .

sto:ISA  a                       sto:StandardOrganization , owl:NamedIndividual ;
        rdfs:comment             "The International Society of Automation (www.isa.org) is a nonprofit professional association that sets the standard for those who apply engineering and technology to improve the management, safety, and cybersecurity of modern automation and control systems used across industry and critical infrastructure. Founded in 1945, ISA develops widely used global standards; certifies industry professionals; provides education and training; publishes books and technical articles; hosts conferences and exhibits; and provides networking and career development programs for its 40,000 members and 400,000 customers around the world."@en ;
        sto:abbreviation         "ISA" ;
        sto:formationDate        "1945-04-28"^^xsd:date ;
        sto:hasDBpediaResource   <http://dbpedia.org/resource/International_Society_of_Automation> ;
        sto:hasHeadquaterIn      dbr:_North_Carolina ;
        sto:hasOfficialResource  <https://www.isa.org/> ;
        sto:hasWikipediaArticle  <https://en.wikipedia.org/wiki/International_Society_of_Automation> ;
        sto:orgName              "International Society of Automation"@en .

sto:hasStatus  a      owl:DatatypeProperty ;
        rdfs:comment  "Publication status of the Standard, e.g., Valid, Revised, Published, under preparation, Released"@en ;
        rdfs:domain   sto:Publication ;
        rdfs:label    "has Status"@en ;
        rdfs:range    rdfs:Literal .

sto:W3C_SPARQL  a                owl:NamedIndividual , sto:Standard ;
        rdfs:comment             "The SPARQL Protocol and RDF Query Language (SPARQL) is a query language and protocol for RDF. This document specifies the SPARQL Protocol; it describes a means for conveying SPARQL queries and updates to a SPARQL processing service and returning the results via HTTP to the entity that requested them. This protocol was developed by the W3C SPARQL Working Group, part of the Semantic Web Activity as described in the activity statement ."@en ;
        rdfs:label               "SPARQL"@en ;
        dcterms:hasLicense       "Public"@en ;
        sto:hasDBpediaResource   "http://dbpedia.org/resource/SPARQL" ;
        sto:hasOfficialResource  "https://www.w3.org/SPARQL" ;
        sto:hasPublisher         sto:W3C ;
        sto:hasTag               "SPARQL"@en ;
        sto:hasWikipediaArticle  "https://en.wikipedia.org/wiki/SPARQL" ;
        sto:relatedTo            sto:W3C_RDF .

dbr:Berlin  a   owl:NamedIndividual .

sto:IEC_61987_X  a               sto:Standard , owl:NamedIndividual ;
        rdfs:comment             "Industrial-process measurement and control - Data structures and elements in process equipment catalogs - Measuring equipment with analogue and digital output"@en ;
        rdfs:label               "IEC 61987_X"@en ;
        dcterms:hasLicense       "Private"@en ;
        sto:hasClassification    rami:FieldDevice , rami:Product , rami:Engineering , rami:WorkCenter , rami:ControlDevice , rami:Station , rami:Enterprise ;
        sto:hasMotivation        "Properties and LOPs as an informational representation of the features of measuring equipment. The referenced standards define general principles (e.g. part 11) as well as specific LOPs for specific device types. These international standards also may serve as examples for description of products."@en ;
        sto:hasOfficialResource  "https://webstore.iec.ch/publication/6225" ;
        sto:hasPublisher         sto:IEC ;
        sto:hasTag               "LOPs in PA"@en .

rami:Integration  a        owl:NamedIndividual , rami:RAMIITLayer ;
        sto:isDescribedin  sto:RAMI40 .

sto:SysML  a                     owl:NamedIndividual , sto:Standard ;
        rdfs:comment             "The OMG Systems Modeling Language (OMG SysML) is a general-purpose graphical modeling language for specifying, analyzing, designing, and verifying complex systems that may include hardware, software, information, personnel, procedures, and facilities. In particular, the language provides graphical representations with a semantic foundation for modeling system requirements, behavior, structure, and parametrics, which is used to integrate with other engineering analysis models. It represents a subset of UML 2 with extensions needed to satisfy the requirements of the UML for Systems Engineering RFP as indicated in Figure 1. SysML leverages the OMG XML Metadata Interchange (XMI®) to exchange modeling data between tools, and is also intended to be compatible with the evolving ISO 10303-233 systems engineering data interchange standard."@en ;
        rdfs:label               "Systems Modeling Language"@en ;
        sto:hasDBpediaResource   "http://dbpedia.org/resource/Systems_Modeling_Language" ;
        sto:hasDeveloper         sto:OMG ;
        sto:hasOfficialResource  "http://sysml.org/" , "http://www.omgsysml.org/what-is-sysml.htm" ;
        sto:hasPublisher         sto:OMG ;
        sto:hasTag               "SysML"@en ;
        sto:hasWikipediaArticle  "https://en.wikipedia.org/wiki/Systems_Modeling_Language" ;
        sto:relatedTo            sto:IEC_62714 .

sto:hasMotivation  a  owl:ObjectProperty ;
        rdfs:comment  "Describes the motivation of the standards"@en ;
        rdfs:domain   sto:Publication ;
        rdfs:label    "has Motivation"@en ;
        rdfs:range    deo:Motivation .

sto:TC_77  a          sto:TechnicalCommittee , owl:NamedIndividual ;
        rdfs:comment  "Standardization - to prepare standards and technical reports -\n\nin the field of electromagnetic compatibility (EMC), with\nparticular emphasis on general application and use by product\ncommittees. (Horizontal function).\nThe scope covers the following aspects of EMC:\n- Immunity and related items, over the whole frequency range: basic and generic standards,\n- emission in the low frequency range (f <= 9 kHz, e.g. harmonics and voltage fluctuations): basic, generic and product (family) standards,\n- emission in the high frequency range (f > 9 kHz): disturbances not covered by CISPR 10 (1992), in co-ordination with CISPR (e.g. mains signalling).\nProduct immunity standards are not included. However, at the request of product committees, TC 77 may also prepare such standards under the co-ordination of ACEC.\nHorizontal Safety Function:\nElectromagnetic compatibility in so far as safety aspects are involved."@en ;
        rdfs:label    "TC 77"@en ;
        sto:hasTitle  "Electromagnetic compatibility\n"@en .

dbr:_Arizona  a  owl:NamedIndividual .

sto:ISO_ASTM_52915  a            sto:Standard , owl:NamedIndividual ;
        rdfs:comment             "ISO ASTM 52915:2016 provides the specification for the Additive Manufacturing File Format (AMF), an interchange format to address the current and future needs of additive manufacturing technology."@en ;
        rdfs:label               "ISO ASTM 52915"@en ;
        sto:hasClassification    rami:Engineering , rami:Asset , sto:ProductionSystemEngineering , rami:Identification , rami:Product ;
        sto:hasDomain            sto:IndustrialAutomation ;
        sto:hasOfficialResource  "https://www.iso.org/standard/60572.html" ;
        sto:hasPublicationDate   "2016-02-01"^^xsd:date ;
        sto:hasPublisher         sto:ISO ;
        sto:relatedTo            sto:ISO_14306 , sto:IEC_62541 .

sto:hasWikipediaArticle
        a             owl:DatatypeProperty ;
        rdfs:comment  "Wikipedia Article about the Standard"@en ;
        rdfs:label    "has Wikipedia Article"@en ;
        rdfs:range    rdfs:Literal .

sto:IEC_60086  a                 owl:NamedIndividual , sto:Standard ;
        rdfs:comment             "Standard battery nomenclature describes portable dry cell batteries that have physical dimensions and electrical characteristics interchangeable between manufacturers."@en ;
        rdfs:label               "IEC 60086"@en ;
        sto:hasDBpediaResource   "http://dbpedia.org/page/Battery_nomenclature#IEC_60086" ;
        sto:hasOfficialResource  "https://webstore.iec.ch/publication/22991" ;
        sto:hasPublisher         sto:IEC ;
        sto:hasWikipediaArticle  "https://en.wikipedia.org/wiki/Battery_nomenclature#IEC_60086" .

sto:ISA95Level  a        owl:Class ;
        rdfs:comment     "Describes the ISA95 levels to classify the industry Standards according to those levels. Eg., Device, SCADA, etc. It has strong relation to the RAMI Hierarchy levels"@en ;
        rdfs:label       "ISA95 Level"@en ;
        rdfs:subClassOf  sto:StandardClassification .

sto:IEC_61334_P4_S32_1996
        a                          sto:Standard , owl:NamedIndividual ;
        rdfs:comment               "Covers the services required of, or by, the DCP Logical Link Control (LLC) sublayer entity at the logical interfaces with the application layer and the MAC sublayer.\nThis publication is of high relevance for Smart Grid."@en ;
        rdfs:label                 "IEC 61334-4-32:1996 "@en ;
        sto:hasAvailableLanguage   "English/French"@en ;
        sto:hasDBpediaResource     <https://dbpedia.org/resource/IEC_61334> , <null//dbpedia.org/resource/IEC_61334> ;
        sto:hasEdition             "1.0"^^xsd:float ;
        sto:hasFileSize            sto:FileSizeIEC_61334_1996_P4_S32 ;
        sto:hasICS                 sto:ICS_29_240_20 , sto:ICS_33_200 ;
        sto:hasOfficialResource    <https://webstore.iec.ch/publication/5301> , <null//webstore.iec.ch/publication/5301> ;
        sto:hasPages               "69"^^xsd:int ;
        sto:hasPublicationDate     "1996-09-26"^^xsd:date ;
        sto:hasPublisher           sto:IEC ;
        sto:hasStabilityDate       "2018"^^xsd:gYear ;
        sto:hasTag                 "IEC 61334-4-32:1996 "@en ;
        sto:hasTechnicalCommittee  sto:TC_57 ;
        sto:hasTitle               "Distribution automation using distribution line carrier systems - Part 4: Data communication protocols - Section 32: Data link layer - Logical link control (LLC)"@en ;
        sto:hasWikipediaArticle    <null//en.wikipedia.org/wiki/IEC_61334> , <https://en.wikipedia.org/wiki/IEC_61334> .

sto:B2MML  a                     sto:Standard , owl:NamedIndividual ;
        rdfs:comment             "B2MML or Business To Manufacturing Markup Language is an XML implementation of the ANSI/ISA-95 family of standards (ISA-95)"@en ;
        rdfs:label               "Business To Manufacturing Markup Language" ;
        skos:altLabel            "IEC 62264"@en ;
        sto:hasClassification    sto:BusinessProcessExecution , sto:EnterpriseLevel ;
        sto:hasDBpediaResource   "http://dbpedia.org/resource/B2MML" ;
        sto:hasDeveloper         sto:MESA ;
        sto:hasOfficialResource  "https://services.mesa.org/ResourceLibrary/ShowResource/0f47758b-60f0-40c6-a71b-fa7b2363fb3a" ;
        sto:hasPublisher         sto:MESA ;
        sto:hasTag               "B2MML"@en ;
        sto:hasWikipediaArticle  "https://en.wikipedia.org/wiki/B2MML" ;
        sto:isImplementationOf   sto:ISA-95 .

sto:FileSizeIEC_60870_P6_S2_1995
        a                      om2:Measure , owl:NamedIndividual ;
        rdfs:comment           "Specifies the file size of the document for standard IEC 60870-6-2:1995"@en ;
        rdfs:label             "FileSize IEC 60870-6-2:1995"@en ;
        om2:hasNumericalValue  "3524.0"^^xsd:float ;
        om2:hasUnit            om2:kilobyte .

sto:IEC_60870_P2_S1_1995
        a                          owl:NamedIndividual , sto:Standard ;
        rdfs:comment               "Specifies classes for environmental conditions under which telecontrol equipment has to operate."@en ;
        rdfs:label                 "IEC 60870-2-1:1995"@en ;
        sto:hasAvailableLanguage   "English/French"@en , " Spanish"@en ;
        sto:hasDBpediaResource     <https://dbpedia.org/resource/IEC_60870> , <null//dbpedia.org/resource/IEC_60870> ;
        sto:hasEdition             "2.0"^^xsd:float ;
        sto:hasFileSize            sto:FileSizeIEC_60870_1995_P2_S1 ;
        sto:hasICS                 sto:ICS_33_200 , sto:ICS_33_100_10 , sto:ICS_29_020 ;
        sto:hasOfficialResource    <https://webstore.iec.ch/publication/3738> , <null//webstore.iec.ch/publication/3738> ;
        sto:hasPages               "43"^^xsd:int ;
        sto:hasPublicationDate     "1995-12-342"^^xsd:date ;
        sto:hasPublisher           sto:IEC ;
        sto:hasStabilityDate       "2018"^^xsd:gYear ;
        sto:hasTag                 "IEC 60870-2-1:1995"@en ;
        sto:hasTechnicalCommittee  sto:TC_57 ;
        sto:hasTitle               "Telecontrol equipment and systems - Part 2: Operating conditions - Section 1: Power supply and electromagnetic compatibility"@en ;
        sto:hasWikipediaArticle    <https://en.wikipedia.org/wiki/IEC_60870> , <null//en.wikipedia.org/wiki/IEC_60870> .

sto:belongsTo  a      owl:ObjectProperty ;
        rdfs:comment  "A Standard Organization that belongs to the country"@en ;
        rdfs:domain   sto:StandardOrganization ;
        rdfs:label    "belongs To"@en ;
        rdfs:range    dbo:Country .

sto:IEC_60839_P7_7  a              owl:NamedIndividual , sto:Standard ;
        rdfs:comment               "Specifies the requirements for standard interfaces between the control and indicating equipment (CIE) of an alarm system and an alarm system transceiver where the alarm system transceiver is intended to plug into a standard space inside the CIE of the alarm system."@en ;
        rdfs:label                 "IEC 60839-7-7:2001"@en ;
        sto:hasAvailableLanguage   "English"@en , " English/French"@en ;
        sto:hasEdition             "1.0"^^xsd:float ;
        sto:hasFileSize            sto:FileSizeIEC_60839_P7_7 ;
        sto:hasICS                 sto:ICS_13_320 ;
        sto:hasOfficialResource    <null//webstore.iec.ch/publication/3675> ;
        sto:hasPages               "21"^^xsd:int ;
        sto:hasPublicationDate     "68/03/01"^^xsd:date ;
        sto:hasPublisher           sto:IEC ;
        sto:hasStabilityDate       "2018"^^xsd:gYear ;
        sto:hasTag                 "IEC 60839-7-7:2001"@en ;
        sto:hasTechnicalCommittee  sto:TC_79 ;
        sto:hasTitle               "Alarm systems - Part 7-7: Message formats and protocols for serial data interfaces in alarm transmission systems - Alarm system interfaces for plug-in alarm system transceivers"@en .

rami:Information  a        owl:NamedIndividual , rami:RAMIITLayer ;
        sto:isDescribedin  sto:RAMI40 .

rami:Station  a            owl:NamedIndividual , rami:RAMIHierarchyLevel ;
        sto:isDescribedin  sto:RAMI40 .

rami:Security  a           owl:NamedIndividual , rami:AdminShellSubmodel ;
        sto:isDescribedin  sto:AdministrationShell .

sto:FileSizeIEC_60839_P7_3
        a                      om2:Measure , owl:NamedIndividual ;
        rdfs:comment           "Specifies the file size of the document for standard IEC 60839-7-3:2001"@en ;
        rdfs:label             "FileSize IEC 60839-7-3:2001"@en ;
        om2:hasNumericalValue  "975.0"^^xsd:float ;
        om2:hasUnit            om2:kilobyte .

sto:ISO_1302  a                  owl:NamedIndividual , sto:Standard ;
        rdfs:comment             "Geometrical product specifications Standards"@en ;
        rdfs:label               "ISO 1302"@en ;
        sto:hasClassification    sto:ModelingPractice ;
        sto:hasOfficialResource  "https://www.iso.org/standard/28089.html" ;
        sto:hasPublicationDate   "2002-02-01"^^xsd:date .

rami:TypeDevelopment  a  owl:NamedIndividual , rami:RAMILifeCycleLayer ;
        rdfs:label  "Type Development"@en .

xsd:gYear  a    rdfs:Datatype .

rami:ControlDevice  a      owl:NamedIndividual , rami:RAMIHierarchyLevel ;
        sto:isDescribedin  sto:RAMI40 .

sto:IEC_60364  a                 owl:NamedIndividual , sto:Standard ;
        rdfs:comment             "Electrical Installations for Buildings is the International Electrotechnical Commission's international standard on electrical installations of buildings"@en ;
        rdfs:label               "IEC 60364"@en ;
        sto:hasDBpediaResource   "http://dbpedia.org/page/IEC_60364" ;
        sto:hasPublisher         sto:IEC ;
        sto:hasWikipediaArticle  "https://en.wikipedia.org/wiki/IEC_60364" .

sto:IEC_60870_P5_S103_1997
        a                          sto:Standard , owl:NamedIndividual ;
        rdfs:comment               "Applies to protection equipment with coded bit serial data transmission for exchanging information with control systems. Defines a companion standard that enables interoperability between protection equipment and devices of a control system in a substation.\nThis publication is of high relevance for Smart Grid."@en ;
        rdfs:label                 "IEC 60870-5-103:1997"@en ;
        sto:hasAvailableLanguage   " English/French"@en , "English"@en , " French"@en ;
        sto:hasDBpediaResource     <null//dbpedia.org/resource/IEC_60870> , <https://dbpedia.org/resource/IEC_60870> ;
        sto:hasEdition             "1.0"^^xsd:float ;
        sto:hasFileSize            sto:FileSizeIEC_60870_P5_S103_1997 ;
        sto:hasICS                 sto:ICS_33_200 ;
        sto:hasOfficialResource    <https://webstore.iec.ch/publication/3745> , <null//webstore.iec.ch/publication/3745> ;
        sto:hasPages               "203"^^xsd:int ;
        sto:hasPublicationDate     "1997-12-345"^^xsd:date ;
        sto:hasPublisher           sto:IEC ;
        sto:hasStabilityDate       "2018"^^xsd:gYear ;
        sto:hasTag                 "IEC 60870-5-103:1997"@en ;
        sto:hasTechnicalCommittee  sto:TC_57 ;
        sto:hasTitle               "Telecontrol equipment and systems - Part 5-103: Transmission protocols - Companion standard for the informative interface of protection equipment"@en ;
        sto:hasWikipediaArticle    <null//en.wikipedia.org/wiki/IEC_60870> , <https://en.wikipedia.org/wiki/IEC_60870> .

sto:hasFileSize  a    owl:ObjectProperty ;
        rdfs:comment  "The size of document file in some unit e.g. 104 Kilobyte."@en ;
        rdfs:domain   foaf:Document ;
        rdfs:label    "has File Size"@en ;
        rdfs:range    om2:Measure ;
        rdfs:seeAlso  <https://webstore.iec.ch/webstore/webstore.nsf/xpFAQ.xsp?Open&id=ADMN-7NALM5> ;
        skos:note     "1. Reference for om2:Measure <http://www.ontology-of-units-of-measure.org/page/om-2/Measure>\n                         2. om2:Measure om2:hasNumericalValue xsd:float;\n                         3. om2:Measure om2:hasUnit om2:Unit;\n                         4. om2:hasUnit om2:InformationCapacityUnit; is another possibility for range that could not be verified.\n                         5. rdfs:seeAlso <http://www.ontology-of-units-of-measure.org/page/om-2/kilobyte> \n                         6. Documentation on Measure <https://github.com/HajoRijgersberg/OM>" .

sto:IEC_60870_P5_S6_2006
        a                          owl:NamedIndividual , sto:Standard ;
        rdfs:comment               "IEC 60870-5-6:2006 Specifies methods for conformance testing of telecontrol equipment, amongst substation automation systems and telecontrol systems, including front-end functions of SCADA. Facilitates interoperability by providing a standard method of testing protocol implementations. Is expected to minimize the risk of non-interoperability."@en ;
        rdfs:label                 "IEC 60870-5-6:2006"@en ;
        sto:hasAvailableLanguage   " English/French"@en , "English"@en ;
        sto:hasDBpediaResource     <null//dbpedia.org/resource/IEC_60870> , <https://dbpedia.org/resource/IEC_60870> ;
        sto:hasEdition             "1.0"^^xsd:float ;
        sto:hasFileSize            sto:FileSizeIEC_60870_P5_S6_2006 ;
        sto:hasICS                 sto:ICS_33_200 ;
        sto:hasOfficialResource    <https://webstore.iec.ch/publication/3751> , <null//webstore.iec.ch/publication/3751> ;
        sto:hasPages               "46"^^xsd:int ;
        sto:hasPublicationDate     "2006-03-67"^^xsd:date ;
        sto:hasPublisher           sto:IEC ;
        sto:hasStabilityDate       "2018"^^xsd:gYear ;
        sto:hasTag                 "IEC 60870-5-6:2006"@en ;
        sto:hasTechnicalCommittee  sto:TC_57 ;
        sto:hasTitle               "Telecontrol equipment and systems - Part 5-6: Guidelines for conformance testing for the IEC 60870-5 companion standards"@en ;
        sto:hasWikipediaArticle    <null//en.wikipedia.org/wiki/IEC_60870> , <https://en.wikipedia.org/wiki/IEC_60870> .

dbr:_Georgia  a  owl:NamedIndividual .

sto:ICS_19_020  a     sto:InternationalClassificationForStandards , owl:NamedIndividual ;
        rdfs:comment  "This is ICS for “Test conditions and procedures in general"@en , "This is ICS for “Test conditions and procedures in general”"@en ;
        rdfs:label    "ICS 19.020"@en ;
        sto:hasTitle  "Test conditions and procedures in general"@en .

sto:IEC_60255_149_2013
        a                            owl:NamedIndividual , sto:Standard ;
        rdfs:comment                 "IEC 60255-149:2013 specifies minimum requirements for thermal protection relays. This standard includes specification of the protection function, measurement characteristics and test methodologies. The object is to establish a common and reproducible reference for evaluating dependent time relays which protect equipment from thermal damage by measuring a.c. current flowing through the equipment. Complementary input energizing quantities such as ambient, coolant, top oil and winding temperature may be applicable for the thermal protection specification set forth in this standard. This standard covers protection relays based on a thermal model with memory function."@en ;
        rdfs:label                   "IEC 60255-149:2013 "@en ;
        sto:hasAvailableLanguage     "English/French"@en ;
        sto:hasEdition               "1.0"^^xsd:float ;
        sto:hasFileSize              sto:FileSizeIEC_60255_149_2013 ;
        sto:hasICS                   sto:ICS_29_120_70 ;
        sto:hasImplementationFormat  "Document"@en ;
        sto:hasOfficialResource      <https://webstore.iec.ch/publication/1165> ;
        sto:hasPages                 93 ;
        sto:hasPublicationDate       "2013-07-30"^^xsd:date ;
        sto:hasPublisher             sto:IEC ;
        sto:hasStatus                "Valid"@en ;
        sto:hasTag                   "IEC 60255-149:2013 "@en ;
        sto:hasTechnicalCommittee    sto:TC_95 ;
        sto:hasTitle                 "Measuring relays and protection equipment - Part 149: Functional requirements for thermal electrical relays"@en .

sto:ISO_13374  a                 sto:Standard , owl:NamedIndividual ;
        rdfs:comment             "Condition monitoring and diagnostics of machines -- Data processing, communication and presentation"@en ;
        rdfs:label               "ISO 13374"@en ;
        sto:hasClassification    rami:Business , rami:Enterprise , sto:ProductionSystemEngineering , rami:Conditional_Monitoring ;
        sto:hasDomain            sto:IndustrialAutomation ;
        sto:hasOfficialResource  "https://www.iso.org/standard/61131.html" ;
        sto:hasPublicationDate   "2012-02-01"^^xsd:date ;
        sto:hasPublisher         sto:ISO .

sto:hasPublicationDate
        a             owl:DatatypeProperty ;
        rdfs:comment  "Publication date of the Publication"@en ;
        rdfs:domain   sto:Publication ;
        rdfs:label    "has Publication Date"@en ;
        rdfs:range    xsd:date .

sto:formationDate  a  owl:DatatypeProperty , owl:FunctionalProperty ;
        rdfs:comment  "Formation date of the Organization"@en ;
        rdfs:domain   sto:StandardOrganization ;
        rdfs:label    "has Formation Date"@en ;
        rdfs:range    xsd:date .

sto:TC_8  a           owl:NamedIndividual , sto:TechnicalCommittee ;
        rdfs:comment  "To prepare and coordinate, in co-operation with other TC/SCs, the development of international standards and other deliverables with emphasis on overall system aspects of electricity supply systems and acceptable balance between cost and quality for the users of electrical energy. Electricity supply system encompasses transmission and distribution networks, generators and loads with their network interfaces."@en ;
        rdfs:label    "TC 8"@en ;
        sto:hasTitle  "Systems aspects of electrical energy supply"@en .

sto:IEC  a                       owl:NamedIndividual , sto:StandardOrganization ;
        rdfs:comment             "Is a non-profit, non-governmental international standards organization that prepares and publishes International Standards for all electrical, electronic and related technologies – collectively known as \"electrotechnology\". IEC standards cover a vast range of technologies from power generation, transmission and distribution to home appliances and office equipment, semiconductors, fiber optics, batteries, solar energy, nanotechnology and marine energy as well as many others. The IEC also manages three global conformity assessment systems that certify whether equipment, system or components conform to its International Standards."@en ;
        sto:abbreviation         "IEC" ;
        sto:formationDate        "1906-06-26"^^xsd:date ;
        sto:hasDBpediaResource   <http://dbpedia.org/resource/International_Electrotechnical_Commission> ;
        sto:hasHeadquaterIn      dbr:Geneva ;
        sto:hasOfficialResource  <http://www.iec.ch/> ;
        sto:hasWikipediaArticle  <https://en.wikipedia.org/wiki/International_Electrotechnical_Commission> ;
        sto:orgName              "Commission électrotechnique internationale"@fr , "International Electrotechnical Commission"@en .

sto:FileSizeIEC_60050_1998
        a                      owl:NamedIndividual , om2:Measure ;
        rdfs:comment           "Specifies the file size of the document for standard IEC 60050-101:1998 "@en ;
        rdfs:label             "FileSize IEC 60050-101:1998"@en ;
        om2:hasNumericalValue  "1712.0"^^xsd:float ;
        om2:hasUnit            om2:kilobyte .

sto:Written  a        owl:NamedIndividual , dcterms:linguisticSystem ;
        rdfs:comment  "Describes a Written Linguistic System"@en ;
        rdfs:label    "Written"@en .

rami:InformationLayer
        a                  owl:NamedIndividual , rami:RAMIITLayer ;
        rdfs:label         "Information Layer"@en ;
        sto:isDescribedin  sto:RAMI40 .

sto:ProductionSystemEngineering
        a                  owl:NamedIndividual , sto:ProductionSystemLifeCycle ;
        rdfs:comment       "Standards can interconnect engineering tools from different disciplines, e.g., system engineering, mechanical plant engineering, electrical design, process engineering, process control engineering, Human Machine Interface (HMI) development, PLC programming, and robotic programming."@en ;
        rdfs:label         "Production System Engineering"@en ;
        sto:isDescribedin  sto:NISTInitiative .

sto:ISO_16739  a                 owl:NamedIndividual , sto:Standard ;
        rdfs:comment             "Industry Foundation Classes (IFC) for data sharing in the construction and facility management industries."@en ;
        rdfs:label               "ISO 16739"@en ;
        sto:hasClassification    rami:Station , rami:LifecycleStatus , sto:ProductLifeCycleManagement , rami:WorkCenter ;
        sto:hasDomain            sto:IndustrialAutomation ;
        sto:hasOfficialResource  "https://www.iso.org/standard/51622.html" ;
        sto:hasPublicationDate   "2013-04-01"^^xsd:date ;
        sto:hasPublisher         sto:ISO ;
        sto:relatedTo            sto:IEC_62890 .

sto:IEC_60073_2002  a                owl:NamedIndividual , sto:Standard ;
        rdfs:comment                 "Establishes general rules for assigning particular meanings to certain visual, acoustsic and tactile indications. It has the status of a Basic Safety Publication in accordance with IEC Guide 104."@en ;
        rdfs:label                   "IEC 60073:2002 "@en ;
        sto:hasAvailableLanguage     "English/French, Spanish"@en ;
        sto:hasEdition               "6.0"^^xsd:float ;
        sto:hasFileSize              sto:FileSizeIEC_60073_2002 ;
        sto:hasICS                   sto:ICS_01_070 , sto:ICS_29_020 ;
        sto:hasImplementationFormat  "Document"@en ;
        sto:hasOfficialResource      <https://webstore.iec.ch/publication/587> ;
        sto:hasPages                 61 ;
        sto:hasPublicationDate       "2002-05-22"^^xsd:date ;
        sto:hasPublisher             sto:IEC ;
        sto:hasStabilityDate         "2025"^^xsd:gYear ;
        sto:hasStatus                "Valid"@en ;
        sto:hasTag                   "IEC_60073:2002"@en ;
        sto:hasTechnicalCommittee    sto:TC_3 ;
        sto:hasTitle                 "Basic and safety principles for man-machine interface, marking and identification - Coding principles for indicators and actuators"@en .

sto:ISO_27000  a                 owl:NamedIndividual , sto:Standard ;
        rdfs:comment             "The ISO/IEC 27000 family of standards helps organizations keep information assets secure. Using this family of standards will help your organization manage the security of assets such as financial information, intellectual property, employee details or information entrusted to you by third parties."@en ;
        rdfs:label               "ISO/IEC 27000"@en , "ISO 27000"@en , "IEC 27000"@en ;
        sto:hasDBpediaResource   "http://dbpedia.org/resource/IEC_27000" ;
        sto:hasMotivation        "Provides best practices for information security management. A critical issue for Industry 4.0 "@en ;
        sto:hasOfficialResource  "http://www.27000.org/" ;
        sto:hasPublisher         sto:ISO ;
        sto:hasTag               "Information Security Management Systems"@en ;
        sto:hasWikipediaArticle  "https://en.wikipedia.org/wiki/ISO/IEC_27000" .

sto:FileSizeIEC_60870_P5_S4_1993
        a                      om2:Measure , owl:NamedIndividual ;
        rdfs:comment           "Specifies the file size of the document for standard IEC 60870-5-4:1993"@en ;
        rdfs:label             "FileSize IEC 60870-5-4:1993"@en ;
        om2:hasNumericalValue  "1776.0"^^xsd:float ;
        om2:hasUnit            om2:kilobyte .

om2:Measure  a  owl:Class .

sto:IEC_60839-5-2  a             owl:NamedIndividual , sto:Standard ;
        rdfs:comment             "IEC 60839-5-2:2016 specifies the general equipment requirements for the performance, reliability, resilience, security and safety characteristics of supervised premises transceiver (SPT) installed in supervised premises and used in alarm transmission systems (ATS). A supervised premises transceiver can be a stand-alone device or an integrated part of an alarm system. These requirements also apply to the SPT sharing means of interconnection, control, communication and power supplies with other applications. The alarm transmission system requirements and classifications are defined within IEC 60839-5-1. This new edition includes the following significant technical changes with respect to the previous edition: reflects the current technological state of art (IP networks) ,harmonizes with the ATS categories introduced in IEC 60839-5-1:2014; introduces test requirements."@en ;
        rdfs:label               "IEC 60839-5-2"@en ;
        sto:hasClassification    rami:Security , rami:Communication , rami:FieldDevice , rami:ControlDevice ;
        sto:hasOfficialResource  "https://webstore.iec.ch/publication/24120" ;
        sto:hasPublicationDate   "2016-02-03"^^xsd:date ;
        sto:hasPublisher         sto:IEC .

sto:FileSizeIEC_60870_P5_S102_1996
        a                      om2:Measure , owl:NamedIndividual ;
        rdfs:comment           "Specifies the file size of the document for standard IEC 60870-5-102:1996"@en ;
        rdfs:label             "FileSize IEC 60870-5-102:1996"@en ;
        om2:hasNumericalValue  "505.0"^^xsd:float ;
        om2:hasUnit            om2:kilobyte .

sto:BusinessCycleSCM  a   owl:Class ;
        rdfs:comment      "Suply Chain Management Business Cycle."@en ;
        rdfs:isDefinedBy  "http://nvlpubs.nist.gov/nistpubs/ir/2016/NIST.IR.8107.pdf" ;
        rdfs:label        "Business Cycle SCM"@en ;
        rdfs:seeAlso      "https://en.wikipedia.org/wiki/Supply_chain_management" ;
        rdfs:subClassOf   sto:StandardClassification .

sto:MTConnect_Institute
        a                        owl:NamedIndividual , sto:StandardOrganization ;
        rdfs:comment             "MTConnect Institute is a collaborative effort to develop technical standards and specifications intended to foster greater interoperability between automation/control applications, field systems/devices, and business/office applications in the manufacturing industry (\"MTConnect Specifications\"), as well as schema, prototype software examples, and related documentation in order to facilitate the implementation of the MTConnect Specifications in compliant applications, drivers, and other services"@en ;
        sto:abbreviation         "MTC" ;
        sto:formationDate        "2006-01-01"^^xsd:date ;
        sto:hasOfficialResource  "https://w3id.org/i40/www.mtconnect.org" ;
        sto:orgName              "MTConnect Institute"@en .

rami:InstanceMaintenance
        a           owl:NamedIndividual , rami:RAMILifeCycleLayer ;
        rdfs:label  "Instance Maintenance"@en .

sto:ISO_29002  a                 owl:NamedIndividual , sto:Standard ;
        rdfs:comment             "ISO 29002 is an interoperability standard, which provides a repository to be used in various ISO XML formats. It is used in ontoML."@en ;
        rdfs:label               "ISO 29002"@en ;
        sto:hasDomain            sto:IndustrialProcessMeasurementControl ;
        sto:hasOfficialResource  "https://www.iso.org/standard/53617.html" ;
        sto:hasPublicationDate   "2010-04-01"^^xsd:date ;
        sto:hasPublisher         sto:ISO ;
        sto:relatedTo            sto:eClass .

sto:ProductionSystemModelData
        a                  owl:NamedIndividual , sto:ProductionSystemLifeCycle ;
        rdfs:comment       "Provide information models for factory and production system design. They enhance information exchange among stakeholders, and enable virtual commissioning, which can improve manufacturing agility and reduce manufacturing cost."@en ;
        rdfs:label         "Production System Model Data"@en ;
        sto:isDescribedin  sto:NISTInitiative .

sto:hasDeveloper  a         owl:ObjectProperty ;
        rdfs:comment        "The organization that developed this Standard"@en ;
        rdfs:domain         sto:Publication ;
        rdfs:label          "has Developer"@en ;
        rdfs:range          sto:StandardOrganization ;
        rdfs:subPropertyOf  foaf:maker .

sto:IEC_62264  a                 sto:Standard , owl:NamedIndividual ;
        rdfs:comment             "IEC 62264 is an international standard for enterprise-control system integration. This standard is based upon ANSI/ISA-95."@en , "Enterprise-control system integration - Models and terminology"@en ;
        rdfs:label               "IEC 62264"@en ;
        rdfs:seeAlso             "https://en.wikipedia.org/wiki/B2MML" ;
        dcterms:hasLicense       "Private"@en ;
        skos:altLabel            "B2MML" ;
        sto:hasClassification    rami:Functional ;
        sto:hasDBpediaResource   "http://dbpedia.org/resource/IEC_62264" ;
        sto:hasDeveloper         sto:IEC ;
        sto:hasDomain            "Enterprise Control"@en ;
        sto:hasMotivation        "Informational representation of MES and ERP models."@en ;
        sto:hasOfficialResource  "https://webstore.iec.ch/publication/6675" , "https://www.iso.org/standard/57308.html" , "http://www.iso.org/iso/catalogue_detail.htm?csnumber=63740" ;
        sto:hasPublisher         sto:MESA , sto:IEC ;
        sto:hasTag               "Enterprise-control system integration"@en , "Enterprise control systems"@en ;
        sto:hasWikipediaArticle  "https://en.wikipedia.org/wiki/IEC_62264" ;
        sto:relatedTo            sto:ISA-95 .

dbr:_Maryland  a  owl:NamedIndividual .

sto:IEC_62656  a                 owl:NamedIndividual , sto:Standard ;
        rdfs:comment             "Specifies the logical structure for a set of spreadsheets, used as data parcels, to define, transfer and register product ontologies"@en ;
        rdfs:label               "IEC 62656"@en ;
        sto:hasOfficialResource  "https://webstore.iec.ch/publication/7326" ;
        sto:hasPublisher         sto:IEC .

rami:EnergyEfficiency
        a                  owl:NamedIndividual , rami:AdminShellSubmodel ;
        sto:isDescribedin  sto:AdministrationShell .

sto:NISTIR_8107  a         owl:NamedIndividual ;
        rdfs:comment       "Describes the NIST Initiative"@en ;
        rdfs:isDefinedBy   "http://nvlpubs.nist.gov/nistpubs/ir/2016/NIST.IR.8107.pdf" ;
        rdfs:label         "NISTIR_8107"@en ;
        skos:note          "TODO - improve this classification" ;
        sto:isDescribedin  sto:BusinessProcessExecution , sto:SCM .

sto:IEC_60839_P7_2  a              sto:Standard , owl:NamedIndividual ;
        rdfs:comment               "Specifies a common application layer protocol (message structure, formats and transmission procedures) to be used at standard interfaces in alarm transmission systems. Should be used at all such interfaces where equipment from one supplier is intended to inter-work with equipment from other suppliers."@en ;
        rdfs:label                 "IEC 60839-7-2:2001"@en ;
        sto:hasAvailableLanguage   " English/French"@en , "English"@en ;
        sto:hasEdition             "1.0"^^xsd:float ;
        sto:hasFileSize            sto:FileSizeIEC_60839_P7_2 ;
        sto:hasICS                 sto:ICS_13_320 ;
        sto:hasOfficialResource    <null//webstore.iec.ch/publication/3669> ;
        sto:hasPages               "53"^^xsd:int ;
        sto:hasPublicationDate     "68/03/01"^^xsd:date ;
        sto:hasPublisher           sto:IEC ;
        sto:hasStabilityDate       "2018"^^xsd:gYear ;
        sto:hasTag                 "IEC 60839-7-2:2001"@en ;
        sto:hasTechnicalCommittee  sto:TC_79 ;
        sto:hasTitle               "Alarm systems - Part 7-2: Message formats and protocols for serial data interfaces in alarm transmission systems - Common application layer protocol"@en .

sto:IEC_62837  a                 owl:NamedIndividual , sto:Standard ;
        rdfs:comment             "Provides to the technical committees a framework for the development and adaptation of documents in order to improve energy efficiency in manufacturing, process control and industrial facility management."@en ;
        rdfs:label               "IEC 62837"@en ;
        sto:hasOfficialResource  "https://webstore.iec.ch/publication/7446" ;
        sto:hasPublisher         sto:IEC ;
        sto:hasTag               "62837"@en .

sto:FileSizeIEC_61010_P2_S012_2016
        a                      om2:Measure , owl:NamedIndividual ;
        rdfs:comment           "Specifies the file size of the document for standard IEC 61010-2-012:2016."@en ;
        rdfs:label             "FileSize IEC 61010-2-012:2016"@en ;
        om2:hasNumericalValue  "2717.0"^^xsd:float ;
        om2:hasUnit            om2:kilobyte .

sto:eClass  a                    sto:Standard , owl:NamedIndividual ;
        rdfs:comment             "eCl@ss is the cross-industry product data standard for classification and clear description of products and services."@en ;
        rdfs:label               "eClass"@en ;
        sto:hasClassification    rami:Station , rami:WorkCenter , rami:Product , rami:Engineering , rami:ConnectedWorld , rami:Enterprise , rami:ControlDevice ;
        sto:hasDBpediaResource   "http://de.dbpedia.org/page/ECl@ss" ;
        sto:hasDeveloper         sto:eClassAssoc ;
        sto:hasMotivation        "Global identification, semantic description and automatic product classification"@en ;
        sto:hasOfficialResource  "https://www.eclass.eu/eclasscontent/standard/overview.html.en" ;
        sto:hasPublisher         sto:eClassAssoc ;
        sto:hasTag               "eClass"@en ;
        sto:hasWikipediaArticle  "https://de.wikipedia.org/wiki/ECl@ss" ;
        sto:relatedTo            sto:IEC_61360 , sto:ISO_13584 .

sto:IEC_61334_P4_S1_1996
        a                          sto:Standard , owl:NamedIndividual ;
        rdfs:comment               "Provides a basic description of the communication system based on a three layer model. Application examples are control and monitoring of the distribution network, order broadcast, control of user interfaces, public lighting, automatic meter reading, etc.\nThis publication is of high relevance for Smart Grid."@en ;
        rdfs:label                 "IEC 61334-4-1:1996 "@en ;
        sto:hasAvailableLanguage   "English/French"@en ;
        sto:hasDBpediaResource     <null//dbpedia.org/resource/IEC_61334> , <https://dbpedia.org/resource/IEC_61334> ;
        sto:hasEdition             "1.0"^^xsd:float ;
        sto:hasFileSize            sto:FileSizeIEC_61334_1996_P4_S1 ;
        sto:hasICS                 sto:ICS_29_240_20 , sto:ICS_33_200 ;
        sto:hasOfficialResource    <null//webstore.iec.ch/publication/5300> , <https://webstore.iec.ch/publication/5300> ;
        sto:hasPages               "43"^^xsd:int ;
        sto:hasPublicationDate     "1996-07-31"^^xsd:date ;
        sto:hasPublisher           sto:IEC ;
        sto:hasStabilityDate       "2018"^^xsd:gYear ;
        sto:hasTag                 "IEC 61334-4-1:1996 "@en ;
        sto:hasTechnicalCommittee  sto:TC_57 ;
        sto:hasTitle               "Distribution automation using distribution line carrier systems - Part 4: Data communication protocols - Section 1: Reference model of the communication system"@en ;
        sto:hasWikipediaArticle    <null//en.wikipedia.org/wiki/IEC_61334> , <https://en.wikipedia.org/wiki/IEC_61334> .

sto:FrameworkLayer  a     owl:NamedIndividual , sto:ConnectivityLayer ;
        rdfs:comment      "Framework Layer"@en , "Framework Layer an instance of the Connectivity Layer"@en ;
        rdfs:isDefinedBy  "https://www.iiconsortium.org/pdf/IIC_PUB_G5_V1.01_PB_20180228.pdf" .

sto:StandardClassification
        a             owl:Class ;
        rdfs:comment  "Describes categorization areas that the different Standardizations Initiatives use to category Standards."@en ;
        rdfs:label    "Standard Classification"@en .

sto:IEC_60870_P5_S5_1995
        a                          owl:NamedIndividual , sto:Standard ;
        rdfs:comment               "Applies to telecontrol equipment and systems with coded bit serial data transmission for monitoring and controlling geographically widespread processes. It defines a telecontrol companion standard that enables interoperability among compatible telecontrol equipment. \nThis publication is of high relevance for Smart Grid."@en ;
        rdfs:label                 "IEC 60870-5-5:1995"@en ;
        sto:hasAvailableLanguage   "English/French"@en ;
        sto:hasDBpediaResource     <null//dbpedia.org/resource/IEC_60870> , <https://dbpedia.org/resource/IEC_60870> ;
        sto:hasEdition             "1.0"^^xsd:float ;
        sto:hasFileSize            sto:FileSizeIEC_60870_P5_S5_1995 ;
        sto:hasICS                 sto:ICS_33_200 ;
        sto:hasOfficialResource    <null//webstore.iec.ch/publication/3750> , <https://webstore.iec.ch/publication/3750> ;
        sto:hasPages               "101"^^xsd:int ;
        sto:hasPublicationDate     "1995-06-155"^^xsd:date ;
        sto:hasPublisher           sto:IEC ;
        sto:hasStabilityDate       "2018"^^xsd:gYear ;
        sto:hasTag                 "IEC 60870-5-5:1995"@en ;
        sto:hasTechnicalCommittee  sto:TC_57 ;
        sto:hasTitle               "Telecontrol equipment and systems - Part 5: Transmission protocols - Section 5: Basic application functions"@en ;
        sto:hasWikipediaArticle    <https://en.wikipedia.org/wiki/IEC_60870> , <null//en.wikipedia.org/wiki/IEC_60870> .

sto:ETSI_LTN  a                  sto:Standard , owl:NamedIndividual ;
        rdfs:comment             "Machine-to-Machine communications and the Internet of Things (IoT) involve the connection of potentially billions of connected objects which need only low throughput connectivity. The anticipated benefits of creating new dedicated IoT Low Throughput Networks (LTN) include lower costs, the creation of new applications, a reduction in electromagnetic radiation by improving data transmission efficiency LTN are expected to be crucial to the success of IoT standardization and implementation, and to provide the basis for many new and innovative applications. "@en ;
        rdfs:label               "ETSI LTN"@en ;
        sto:hasDeveloper         sto:ETSI ;
        sto:hasDomain            sto:M2M ;
        sto:hasOfficialResource  "http://www.etsi.org/technologies-clusters/technologies/low-throughput-networks" ;
        sto:hasPublisher         sto:ETSI ;
        sto:hasTag               "Low Throughput Networks"@en ;
        sto:relatedTo            sto:ETSI_DECT .

sto:IEC_61360  a                 owl:NamedIndividual , sto:Standard ;
        rdfs:comment             "IEC Common Data Dictionary (IEC CDD) is a common repository of concepts for all electrotechnical domains based on the methodology and the information model of IEC 61360 series. Standard data elements types with associated classification scheme for electric items."@en ;
        rdfs:label               "IEC 61360"@en ;
        sto:hasClassification    rami:Engineering , sto:ManufacturingModelData , rami:Asset ;
        sto:hasDomain            "Electrotechnical"@en ;
        sto:hasMotivation        "Standard data elements (properties) are used as elements in administration shell"@en ;
        sto:hasOfficialResource  "http://cdd.iec.ch/cdd/iec61360/iec61360.nsf" , "https://webstore.iec.ch/publication/5380" ;
        sto:hasPublisher         sto:IEC ;
        sto:hasTag               "IEC Common Data Dictionary"@en ;
        sto:relatedTo            sto:eClass , sto:ISO_13584 .

dcterms:language  a  owl:ObjectProperty .

sto:FileSizeIEC_61334_1996_P4_S41
        a                      om2:Measure , owl:NamedIndividual ;
        rdfs:comment           "Specifies the file size of the document for standard IEC 61334-4-41:1996"@en ;
        rdfs:label             "FileSize IEC 61334-4-41:1996"@en ;
        om2:hasNumericalValue  "834.0"^^xsd:float ;
        om2:hasUnit            om2:kilobyte .

sto:Publication  a        owl:Class ;
        rdfs:comment      "Specifies a Publicaion. Eg: International Standards,Technical Specifications,Publicly Available Specifications,Amendments\n                Technical Corrigenda,Interpretation Sheets,Technical Reports,Guides"@en ;
        rdfs:isDefinedBy  sto:IEC ;
        rdfs:label        "Publication"@en ;
        rdfs:seeAlso      <http://www.iec.ch/standardsdev/publications/> ;
        rdfs:subClassOf   foaf:Document .

sto:ICS_13_320  a     owl:NamedIndividual , sto:InternationalClassificationForStandards ;
        rdfs:comment  "This is ICS for Alarm and warning systems"@en ;
        rdfs:label    "ICS 13.320"@en ;
        sto:hasTitle  "Alarm and warning systems"@en .

sto:Prodcut  a  owl:NamedIndividual .

sto:IEC_61511  a                 sto:Standard , owl:NamedIndividual ;
        rdfs:comment             "IEC 61511 is a technical standard which sets out practices in the engineering of systems that ensure the safety of an industrial process through the use of instrumentation."@en ;
        rdfs:label               "IEC 61511" ;
        dcterms:hasLicense       "Private"@en ;
        sto:hasDBpediaResource   "http://dbpedia.org/resource/IEC_61511" ;
        sto:hasDomain            sto:FunctionalSafety ;
        sto:hasMotivation        "Defines the functional safety requirements established by IEC 61508 in process industry sector terminology"@en ;
        sto:hasOfficialResource  "https://webstore.iec.ch/publication/24241" ;
        sto:hasPublisher         sto:IEC ;
        sto:hasTag               "Functional safety - Safety instrumented systems for the process industry sector"@en ;
        sto:hasWikipediaArticle  "https://en.wikipedia.org/wiki/IEC_61511" ;
        sto:relatedTo            sto:IEC_62061 , sto:ISO_13849 .

dbr:Paris  a    owl:NamedIndividual .

sto:FileSizeIEC_60870_P5_S101_2003
        a                      om2:Measure , owl:NamedIndividual ;
        rdfs:comment           "Specifies the file size of the document for standard IEC 60870-5-101:2003"@en ;
        rdfs:label             "FileSize IEC 60870-5-101:2003"@en ;
        om2:hasNumericalValue  "2651.0"^^xsd:float ;
        om2:hasUnit            om2:kilobyte .

sto:CAD  a                      owl:NamedIndividual , sto:Domain ;
        rdfs:comment            "Computer-Aided Design"@en ;
        rdfs:isDefinedBy        <https://en.wikipedia.org/wiki/Computer-aided_design> ;
        rdfs:label              "CAD" ;
        sto:domainName          "Computer-Aided Design"@en ;
        sto:hasDBpediaResource  <http://dbpedia.org/resource/Computer-aided_design> .

sto:IEC_60870_P6_S701_1998
        a                          owl:NamedIndividual , sto:Standard ;
        rdfs:comment               "Describes the functional profile which defines the provision of the TASE.1 communication services between two control centre end systems.\nThis publication is of high relevance for Smart Grid"@en ;
        rdfs:label                 "IEC 60870-6-701:1998"@en ;
        sto:hasAvailableLanguage   "English/French"@en ;
        sto:hasDBpediaResource     <https://dbpedia.org/resource/IEC_60870> , <null//dbpedia.org/resource/IEC_60870> ;
        sto:hasEdition             "1.0"^^xsd:float ;
        sto:hasFileSize            sto:FileSizeIEC_60870_P6_S701_1998 ;
        sto:hasICS                 sto:ICS_33_200 ;
        sto:hasOfficialResource    <https://webstore.iec.ch/publication/3767> , <null//webstore.iec.ch/publication/3767> ;
        sto:hasPages               "37"^^xsd:int ;
        sto:hasPublicationDate     "1998-08-219"^^xsd:date ;
        sto:hasPublisher           sto:IEC ;
        sto:hasStabilityDate       "2018"^^xsd:gYear ;
        sto:hasTag                 "IEC 60870-6-701:1998"@en ;
        sto:hasTechnicalCommittee  sto:TC_57 ;
        sto:hasTitle               "Telecontrol equipment and systems - Part 6-701: Telecontrol protocols compatible with ISO standards and ITU-T recommendations - Functional profile for providing the TASE.1 application service in end systems"@en ;
        sto:hasWikipediaArticle    <https://en.wikipedia.org/wiki/IEC_60870> , <null//en.wikipedia.org/wiki/IEC_60870> .

rami:FieldDevice  a        owl:NamedIndividual , rami:RAMIHierarchyLevel ;
        sto:isDescribedin  sto:RAMI40 .

sto:TC_3  a           owl:NamedIndividual , sto:TechnicalCommittee ;
        rdfs:comment  "To prepare standards for the electrotechnical and related fields regarding:1) methods and rules associated with the human interpretation of information. This refers to:- presentation of information in technical documentation,- graphical symbols for use in technical documentation,- graphical symbols for the human interaction with equipment,2) methods and rules associated with the handling of information in computer sensible form. This refers to:- information models for the purpose of technical documentation and the exchange of technical information, and the identification of further needs for such models,- definition of data element types and data sets for use in information models and technical documentation, and for exchange of technical information.It includes definition and co-ordination of the information required during the whole life cycle of a device, system, or plant.3) General and safety application concerning the man-machine interface, marking and identification in electrical installations and equipment, marking systems and general rules for:- the meanings of colours and alternative means, when used for marking and identification,- the arrangement of indicating devices and actuators,- coding principles for indicating and actuating devices,- terminal designation of electrical and electronic components, apparatus and equipment,- the termination designation of certain designated conductors,- marking of electrical and electronic equipment with ratings related to supply and to its properties,- marking of bare and insulated conductors.These standards are principally intended for use by technical committees in the preparation of standards in accordance with the principles laid down in IEC Guide 104: Guide to the drafting of Safety Standards, and the role of committees with Safety Pilot Functions and Safety Group Functions, and in ISO/IEC Guide 51: Guidelines for the inclusion of safety aspects in standards."@en ;
        rdfs:label    "TC 3"@en ;
        sto:hasTitle  "Information structures and elements, identification and marking principles, documentation and graphical symbols"@en .

sto:IEC_60255_2009  a                owl:NamedIndividual , sto:Standard ;
        rdfs:comment                 "IEC 60255-1:2009 specifies common rules and requirements applicable to measuring relays and protection equipment including any combination of devices to form schemes for power system protection such as control, monitoring and process interface equipment in order to obtain uniformity of requirements and tests. Covers all measuring relays and protection equipment used for protection within the power system environment."@en ;
        rdfs:label                   "IEC 60255-1:2009 "@en ;
        sto:hasAvailableLanguage     "English/French, Spanish"@en ;
        sto:hasEdition               "1.0"^^xsd:float ;
        sto:hasFileSize              sto:FileSizeIEC_60255_2009 ;
        sto:hasICS                   sto:ICS_29_120_70 ;
        sto:hasImplementationFormat  "Document"@en ;
        sto:hasOfficialResource      <https://webstore.iec.ch/publication/1160> ;
        sto:hasPages                 89 ;
        sto:hasPublicationDate       "2009-08-18"^^xsd:date ;
        sto:hasPublisher             sto:IEC ;
        sto:hasStabilityDate         "2018"^^xsd:gYear ;
        sto:hasStatus                "Valid"@en ;
        sto:hasTag                   "IEC 60255-1:2009 "@en ;
        sto:hasTechnicalCommittee    sto:TC_95 ;
        sto:hasTitle                 "Measuring relays and protection equipment - Part 1: Common requirements"@en .

sto:TC_66  a          sto:TechnicalCommittee , owl:NamedIndividual ;
        rdfs:comment  "To prepare safety standards for test and measurement equipment, industrial-process control equipment, and laboratory equipment wherever they are used.\n\nSuch equipment includes:\na) equipment and systems to measure, test, generate, and analyse, simple and complex electromagnetic quantities and equipment that by electromagnetic means measure physical quantities.\nNote: Aspects of this equipment other than safety are covered by other technical committees.\nb) equipment and systems for industrial-process measurement and control.\nNote: Aspects of this equipment other than safety are covered by TC 65 except that SC 65A has a Horizontal Safety Function relating to the functional safety of electrical/electronic/ programmable electronic systems and SC 65B is responsible for the functional safety of programmable controllers.\nc) laboratory equipment for analysis, handling and preparation of materials.\nNote: This equipment includes measuring instruments, systems and their accessories, for preparation, treatment and analysis of materials in the fields of research, medicine, industry and education, and for environmental monitoring.\nTC 66 has a Group Safety Function in accordance with IEC Guide 104 for the equipment in categories a) to c) above."@en ;
        rdfs:label    "TC 66"@en ;
        sto:hasTitle  " control and laboratory equipment"@en , "Safety of measuring"@en , "Safety of measuring, control and laboratory equipment"@en .

rami:Work_Centers  a  owl:NamedIndividual .

sto:ICS_01_040_07  a  owl:NamedIndividual , sto:InternationalClassificationForStandards ;
        rdfs:comment  "This is ICS for Natural and applied sciences (Vocabularies)"@en ;
        rdfs:label    "ICS 01.040.07"@en ;
        sto:hasTitle  "Natural and applied sciences (Vocabularies)"@en .

sto:W3C  a                       owl:NamedIndividual , sto:StandardOrganization ;
        rdfs:comment             "The World Wide Web Consortium (W3C) is the main international standards organization for the World Wide Web (abbreviated WWW or W3). Founded and currently led by Tim Berners-Lee, the consortium is made up of member organizations which maintain full-time staff for the purpose of working together in the development of standards for the World Wide Web. As of 4 November 2015, the World Wide Web Consortium (W3C) has 408 members. The W3C also engages in education and outreach, develops software and serves as an open forum for discussion about the Web."@en ;
        rdfs:label               "W3C"@en ;
        sto:abbreviation         "W3C" ;
        sto:formationDate        "1994-10-01"^^xsd:date ;
        sto:hasDBpediaResource   "http://dbpedia.org/resource/World_Wide_Web_Consortium" ;
        sto:hasHeadquaterIn      dbr:_Massachusetts ;
        sto:hasOfficialResource  "https://www.w3.org/" ;
        sto:hasWikipediaArticle  "https://en.wikipedia.org/wiki/World_Wide_Web_Consortium" ;
        sto:orgName              "World Wide Web Consortium"@en .

sto:MESA  a                      sto:StandardOrganization , owl:NamedIndividual ;
        rdfs:comment             "The Manufacturing Enterprise Solutions Association International is a global community of manufacturers, producers, industry leaders, and solution providers who are focused on driving business results from manufacturing information."@en ;
        sto:abbreviation         "MESA" ;
        sto:formationDate        "1992-01-01"^^xsd:date ;
        sto:hasDBpediaResource   "http://dbpedia.org/page/Manufacturing_Enterprise_Solutions_Association" ;
        sto:hasHeadquaterIn      dbr:_Arizona ;
        sto:hasOfficialResource  "http://www.mesa.org/en/index.asp" ;
        sto:hasWikipediaArticle  "https://en.wikipedia.org/wiki/Manufacturing_Enterprise_Solutions_Association" ;
        sto:orgName              "Manufacturing Enterprise Solutions Association"@en .

sto:IEC_15459  a                 owl:NamedIndividual , sto:Standard ;
        rdfs:comment             "ISO/IEC 15459-1:2014 specifies a unique string of characters for the identification of individual transport units. The character string is intended to be represented in a bar code label or other AIDC media attached to the entity to meet management needs. To address management needs, different types of entities are recognized in the various parts of ISO/IEC 15459, which allows different requirements to be met by the identities associated with each type. The rules for the unique identification for individual transport units, to identify physical logistical transfers, with the identity relevant for the duration of one or more items in the load being held or transported as part of that load, are defined and supported by example."@en ;
        rdfs:label               "IEC 15459"@en ;
        owl:sameAs               sto:ISO_15459 ;
        sto:hasOfficialResource  "https://www.iso.org/standard/54779.html" ;
        sto:hasPublisher         sto:IEC , sto:ISO ;
        sto:hasTag               "Information technology -- Automatic identification and data capture techniques -- Unique identification"@en .

sto:IEC_61131  a                 owl:NamedIndividual , sto:Standard ;
        rdfs:comment             "IEC 61131 is an IEC standard for programmable controllers. It was known as IEC 1131 before the change in numbering system by IEC. The parts of the IEC 61131 standard are prepared and maintained working group 7, programmable control systems, of subcommittee SC 65B of Technical Committee TC65 of the IEC."@en ;
        rdfs:label               "IEC 61131"@en ;
        dul:isComponentOf        sto:IEC_62714 ;
        sto:hasClassification    rami:ControlDevice , rami:Station , rami:WorkCenter ;
        sto:hasDBpediaResource   "http://dbpedia.org/page/IEC_61131" ;
        sto:hasOfficialResource  "https://webstore.iec.ch/publication/4550" ;
        sto:hasPublisher         sto:IEC ;
        sto:hasTag               "PLC Open"@en ;
        sto:hasWikipediaArticle  "https://en.wikipedia.org/wiki/IEC_61131" ;
        sto:relatedTo            sto:IEC_61499 .

sto:IEC_60255_2010  a                owl:NamedIndividual , sto:Standard ;
        rdfs:comment                 "IEC 60255-127:2010 specifies minimum requirements for over/under voltage relays. The standard includes specification of the protection function, measurement characteristics and time delay characteristics."@en ;
        rdfs:label                   "IEC 60255-127:2010"@en ;
        sto:hasAvailableLanguage     "English/French"@en ;
        sto:hasEdition               "1.0"^^xsd:float ;
        sto:hasFileSize              sto:FileSizeIEC_60255_2010 ;
        sto:hasICS                   sto:ICS_29_120_70 ;
        sto:hasImplementationFormat  "Document"@en ;
        sto:hasOfficialResource      <https://webstore.iec.ch/publication/1163> ;
        sto:hasPages                 49 ;
        sto:hasPublicationDate       "2010-04-27"^^xsd:date ;
        sto:hasPublisher             sto:IEC ;
        sto:hasStatus                "Valid"@en ;
        sto:hasTag                   "IEC 60255-127:2010"@en ;
        sto:hasTechnicalCommittee    sto:TC_95 ;
        sto:hasTitle                 "Measuring relays and protection equipment - Part 127: Functional requirements for over/under voltage protection"@en .

sto:isDescribedin  a  owl:ObjectProperty ;
        rdfs:comment  "Links the Standarization Frameworks with the Classification of Standards"@en ;
        rdfs:domain   sto:StandardClassification ;
        rdfs:label    "is Described in"@en ;
        rdfs:range    sto:StandardizationFramework .

dbr:_Massachusetts  a  owl:NamedIndividual .

sto:KATS  a                      owl:NamedIndividual , sto:StandardOrganization ;
        rdfs:comment             "Korean Agency for Technology and Standards is the government standards organization for South Korea. It is part of the Ministry of Knowledge Economy. It is authorized to regulate and manage the legal measures of South Korea by the current Measures Act."@en ;
        rdfs:label               "Korean Agency for Technology and Standards"@en ;
        dul:isMemberOf           sto:ISO , sto:IEC ;
        sto:abbreviation         "KATS"@de ;
        sto:belongsTo            dbr:South_Korea ;
        sto:hasDBpediaResource   "http://dbpedia.org/page/Korean_Agency_for_Technology_and_Standards" ;
        sto:hasHeadquaterIn      dbr:Eumseong ;
        sto:hasWikipediaArticle  "https://en.wikipedia.org/wiki/Korean_Agency_for_Technology_and_Standards" ;
        sto:orgName              "Korean Agency for Technology and Standards"@en .

rami:AdminShellGeneral
        a                  owl:NamedIndividual , rami:AdminShellSubmodel ;
        sto:isDescribedin  sto:AdministrationShell .

sto:ISO_15926  a                 sto:Standard , owl:NamedIndividual ;
        rdfs:comment             "Industrial automation systems and integration -- Integration of life-cycle data for process plants including oil and gas production facilities."@en ;
        rdfs:label               "ISO 15926"@en ;
        sto:hasClassification    rami:Engineering , rami:Integration , rami:Configuration , rami:Product , sto:ProductLifeCycleManagement ;
        sto:hasDomain            sto:IndustrialAutomation ;
        sto:hasOfficialResource  "https://www.iso.org/standard/29557.html" ;
        sto:hasPublicationDate   "2003-12-01"^^xsd:date ;
        sto:hasPublisher         sto:ISO ;
        sto:relatedTo            sto:ISO_ASTM_52915 .

sto:FileSizeIEC_60381_1982
        a                      owl:NamedIndividual , om2:Measure ;
        rdfs:comment           "Specifies the file size of the document for standard IEC 60381-1:1982 "@en ;
        rdfs:label             "FileSize IEC 60381-1:1982"@en ;
        om2:hasNumericalValue  "507.0"^^xsd:float ;
        om2:hasUnit            om2:kilobyte .

sto:SCADALevel  a          owl:NamedIndividual , sto:ISA95Level ;
        rdfs:comment       "Describes the SCADA level according to the ISA95 level classification."@en ;
        rdfs:label         "SCADA Level"@en ;
        skos:definition    "Supervisory control and data acquisition according to ISA 95"@en ;
        sto:isDescribedin  sto:ISA95 .

sto:FileSizeIEC_61334_1996_P3_S21
        a                      om2:Measure , owl:NamedIndividual ;
        rdfs:comment           "Specifies the file size of the document for standard IEC 61334-3-21:1996 "@en ;
        rdfs:label             "FileSize IEC 61334-3-21:1996 "@en ;
        om2:hasNumericalValue  "1112.0"^^xsd:float ;
        om2:hasUnit            om2:kilobyte .

sto:IEC_62832  a                   sto:TechnicalSpecification , owl:NamedIndividual ;
        rdfs:comment               "Industrial-process measurement, control and automation - Digital factory framework - Part 1: General principles"@en ;
        rdfs:label                 "IEC TS 62832-1:2016 "@en ;
        sto:hasAvailableLanguage   "English"@en ;
        sto:hasEdition             "1.0"^^xsd:float ;
        sto:hasFileSize            sto:FileSizeIEC_62832 ;
        sto:hasICS                 sto:ICS_25_040_40 ;
        sto:hasPages               47 ;
        sto:hasPublicationDate     "2016-12-16"^^xsd:date ;
        sto:hasStabilityDate       "2020"^^xsd:gYear ;
        sto:hasTechnicalCommittee  sto:TC_65 .

sto:ISO_15531-3x  a        owl:NamedIndividual , sto:StandardPart ;
        rdfs:comment       "Manufacturing resource usage management data : refering to the way of managing the use of resources, such as resource configuration and capabilities, operation management of manufacturing devices, installations and facilities."@en ;
        rdfs:isDefinedBy   "https://www.researchgate.net/publication/220171079_ISO_15531_MANDATE_a_standardised_data_model_for_manufacturing_management" ;
        rdfs:label         "ISO 15531 3x series"@en ;
        dul:isComponentOf  sto:ISO_15531 .

sto:IEC_60870_P5_S3_1992
        a                          sto:Standard , owl:NamedIndividual ;
        rdfs:comment               "Applies to telecontrol equipment and systems with coded bit serial data transmission for monitoring and controlling geographically widespread processes; specifies rules for structuring application data units in transmission frames of telecontrol systems.\nThis publication is of high relevance for Smart Grid."@en ;
        rdfs:label                 "IEC 60870-5-3:1992"@en ;
        sto:hasAvailableLanguage   "English/French"@en ;
        sto:hasDBpediaResource     <https://dbpedia.org/resource/IEC_60870> , <null//dbpedia.org/resource/IEC_60870> ;
        sto:hasEdition             "1.0"^^xsd:float ;
        sto:hasFileSize            sto:FileSizeIEC_60870_1992_P5_S3 ;
        sto:hasICS                 sto:ICS_33_200 ;
        sto:hasOfficialResource    <null//webstore.iec.ch/publication/3748> , <https://webstore.iec.ch/publication/3748> ;
        sto:hasPages               "43"^^xsd:int ;
        sto:hasPublicationDate     "1992-09-273"^^xsd:date ;
        sto:hasPublisher           sto:IEC ;
        sto:hasStabilityDate       "2018"^^xsd:gYear ;
        sto:hasTag                 "IEC 60870-5-3:1992"@en ;
        sto:hasTechnicalCommittee  sto:TC_57 ;
        sto:hasTitle               "Telecontrol equipment and systems - Part 5: Transmission protocols - Section 3: General structure of application data"@en ;
        sto:hasWikipediaArticle    <null//en.wikipedia.org/wiki/IEC_60870> , <https://en.wikipedia.org/wiki/IEC_60870> .

dbr:_North_Carolina  a  owl:NamedIndividual .

sto:ISO_11783  a                 owl:NamedIndividual , sto:Standard ;
        rdfs:comment             "ISO 11783, known as Tractors and machinery for agriculture and forestry—Serial control and communications data network is a communication protocol for the agriculture industry based on the SAE J1939 protocol (which includes CANbus)."@en ;
        rdfs:label               "ISO 11783"@en ;
        sto:hasDBpediaResource   "http://dbpedia.org/resource/ISO_11783" ;
        sto:hasOfficialResource  "https://www.iso.org/standard/61646.html" ;
        sto:hasPublisher         sto:ISO ;
        sto:hasTag               "ISOBUS"@en ;
        sto:hasWikipediaArticle  "https://en.wikipedia.org/wiki/ISO_11783" .

rami:Functional  a         owl:NamedIndividual , rami:RAMIITLayer ;
        sto:isDescribedin  sto:RAMI40 .

sto:FileSizeIEC_61690_P2_2000
        a                      om2:Measure , owl:NamedIndividual ;
        rdfs:comment           "Specifies the file size of the document for standard IEC 61690-2:2000 ."@en ;
        rdfs:label             "FileSize IEC 61690-2:2000 "@en ;
        om2:hasNumericalValue  "6700.0"^^xsd:float ;
        om2:hasUnit            om2:kilobyte .

sto:FileSizeIEC_60839_P7_4
        a                      om2:Measure , owl:NamedIndividual ;
        rdfs:comment           "Specifies the file size of the document for standard IEC 60839-7-4:2001"@en ;
        rdfs:label             "FileSize IEC 60839-7-4:2001"@en ;
        om2:hasNumericalValue  "967.0"^^xsd:float ;
        om2:hasUnit            om2:kilobyte .

sto:hasOfficialResource
        a             owl:DatatypeProperty ;
        rdfs:comment  "Standard Official Website"@en ;
        rdfs:label    "has Official Resource"@en ;
        rdfs:range    xsd:string .

dbr:Boston  a   owl:NamedIndividual .

sto:IEC_60038_2009  a                sto:Standard , owl:NamedIndividual ;
        rdfs:comment                 "IEC 60038:2009 specifies standard voltage values which are intended to serve as preferential values for the nominal voltage of electrical supply systems, and as reference values for equipment and system design. This seventh edition supersedes the sixth edition (1993), its Amendment 1 (1994) and its Amendment 2 (1997). It constitutes a technical revision. The significant technical changes are: -the addition of the values of 230 V (50 Hz) and 230/400 V (60 Hz) to Table 1;-the replacement of the utilization voltage range at LV by a reference to the relevant standard and an informative annex;- the addition of the value of 30 kV to Table 3;- the replacement of the value of 1 050 kV by 1 100 kV in Table 5. It has the status of a horizontal standard in accordance with IEC Guide 108."@en ;
        rdfs:label                   "IEC 60038:2009"@en ;
        sto:hasAvailableLanguage     "English/French, Spanish"@en ;
        sto:hasDBpediaResource       <http://dbpedia.org/page/IEC_60038> ;
        sto:hasEdition               "7.0"^^xsd:float ;
        sto:hasFileSize              sto:FileSizeIEC_60038_2009 ;
        sto:hasICS                   sto:ICS_29_020 ;
        sto:hasImplementationFormat  "Document"@en ;
        sto:hasOfficialResource      <https://webstore.iec.ch/publication/153> ;
        sto:hasPages                 26 ;
        sto:hasPublicationDate       "2009-06-17"^^xsd:date ;
        sto:hasPublisher             sto:IEC ;
        sto:hasStabilityDate         "2020"^^xsd:gYear ;
        sto:hasStatus                "Valid"@en ;
        sto:hasTag                   "IEC 60038:2009"@en ;
        sto:hasTechnicalCommittee    sto:TC_8 ;
        sto:hasTitle                 "IEC standard voltages"@en ;
        sto:hasWikipediaArticle      <https://en.wikipedia.org/wiki/IEC_60038> .

sto:FileSizeIEC_61000_P6_S2_2016
        a                      om2:Measure , owl:NamedIndividual ;
        rdfs:comment           "Specifies the file size of the document for standard IEC 61000-6-2:2016."@en ;
        rdfs:label             "FileSize IEC 61000-6-2:2016"@en ;
        om2:hasNumericalValue  "2028.0"^^xsd:float ;
        om2:hasUnit            om2:kilobyte .

sto:FileSizeIEC_60382
        a                      om2:Measure , owl:NamedIndividual ;
        rdfs:comment           "Specifies the file size of the document for standard  IEC 60382:1991."@en ;
        rdfs:label             "FileSize IEC 60382:1991"@en ;
        om2:hasNumericalValue  "557.0"^^xsd:float ;
        om2:hasUnit            om2:kilobyte .

sto:ODVA  a                      owl:NamedIndividual , sto:StandardOrganization ;
        rdfs:comment             "Founded in 1995, ODVA is a global association whose members comprise the world’s leading automation companies. ODVA’s mission is to advance open, interoperable information and communication technologies in industrial automation. ODVA recognizes its media independent network protocol, the Common Industrial Protocol or “CIP” — and the network adaptations of CIP — EtherNet/IP, DeviceNet, CompoNet and ControlNet — as its core technology and the primary common interest of its membership. For future interoperability of production systems and the integration of the production systems with other systems, ODVA embraces the adoption of commercial-off-the-shelf (COTS) and standard, unmodified Internet and Ethernet technologies as a guiding principle wherever possible. This principle is exemplified by EtherNet/IP — the world’s number one industrial Ethernet network."@en ;
        sto:abbreviation         "ODVA" ;
        sto:formationDate        "1995-01-01"^^xsd:date ;
        sto:hasDBpediaResource   "http://dbpedia.org/resource/ODVA_(company)" ;
        sto:hasHeadquaterIn      dbr:_Michigan ;
        sto:hasOfficialResource  "https://www.odva.org" ;
        sto:hasWikipediaArticle  "https://en.wikipedia.org/wiki/ODVA_(company)" ;
        sto:orgName              "ODVA, Inc"@en .

sto:ISO_20922  a                 sto:Standard , owl:NamedIndividual ;
        rdfs:comment             "ISO/IEC 20922:2016 is a Client Server publish/subscribe messaging transport protocol. It is light weight, open, simple, and designed so as to be easy to implement. These characteristics make it ideal for use in many situations, including constrained environments such as for communication in Machine to Machine (M2M) and Internet of Things (IoT) contexts where a small code footprint is required and/or network bandwidth is at a premium."@en ;
        rdfs:label               "ISO 20922"@en ;
        sto:hasDBpediaResource   "http://dbpedia.org/resource/MQTT" ;
        sto:hasDeveloper         sto:IBM , sto:OASIS ;
        sto:hasDomain            sto:M2M ;
        sto:hasOfficialResource  "https://www.iso.org/standard/69466.html" , "http://mqtt.org/" ;
        sto:hasPublisher         sto:IEC , sto:ISO ;
        sto:hasTag               "MQTT"@en , "Message Queue Telemetry Transport"@en ;
        sto:hasWikipediaArticle  "https://en.wikipedia.org/wiki/MQTT" ;
        sto:relatedTo            sto:IEC_62541 .

sto:IEC_60870_P6_S503_2014
        a                          sto:Standard , owl:NamedIndividual ;
        rdfs:comment               "IEC 60870-6-503:2014 specifies a method of exchanging time-critical control centre data through wide-area and local-area networks using a full ISO compliant protocol stack. It contains provisions for supporting both centralized and distributed architectures. This standard includes the exchange of real-time data indications, control operations, time-series data, scheduling and accounting information, remote program control and event notification. This new edition includes the following significant technical changes with respect to the previous edition:\n- certain objects were made informative;\n- services associated with the informative objects were made informative;\n- certain TASE.2 conformance blocks were made out-of-scope."@en ;
        rdfs:label                 "IEC 60870-6-503:2014"@en ;
        sto:hasAvailableLanguage   "English/French"@en ;
        sto:hasDBpediaResource     <https://dbpedia.org/resource/IEC_60870> , <null//dbpedia.org/resource/IEC_60870> ;
        sto:hasEdition             "3.0"^^xsd:float ;
        sto:hasFileSize            sto:FileSizeIEC_60870_P6_S503_2014 ;
        sto:hasICS                 sto:ICS_33_200 ;
        sto:hasOfficialResource    <null//webstore.iec.ch/publication/3760> , <https://webstore.iec.ch/publication/3760> ;
        sto:hasPages               "310"^^xsd:int ;
        sto:hasPublicationDate     "2014-07-196"^^xsd:date ;
        sto:hasPublisher           sto:IEC ;
        sto:hasStabilityDate       "2018"^^xsd:gYear ;
        sto:hasTag                 "IEC 60870-6-503:2014"@en ;
        sto:hasTechnicalCommittee  sto:TC_57 ;
        sto:hasTitle               "Telecontrol equipment and systems - Part 6-503: Telecontrol protocols compatible with ISO standards and ITU-T recommendations - TASE.2 Services and protocol"@en ;
        sto:hasWikipediaArticle    <null//en.wikipedia.org/wiki/IEC_60870> , <https://en.wikipedia.org/wiki/IEC_60870> .

sto:FileSizeIEC_61334_1998_P3_S1
        a                      om2:Measure , owl:NamedIndividual ;
        rdfs:comment           "Specifies the file size of the document for standard IEC 61334-3-1:1998 "@en ;
        rdfs:label             "FileSize IEC 61334-3-1:1998 "@en ;
        om2:hasNumericalValue  "147.0"^^xsd:float ;
        om2:hasUnit            om2:kilobyte .

sto:FileSizeIEC_60204_2000
        a                      owl:NamedIndividual , om2:Measure ;
        rdfs:comment           "Specifies the file size of the document for standard IEC 60204:2000"@en ;
        rdfs:label             "FileSize IEC 60204:2000"@en ;
        om2:hasNumericalValue  "494.0"^^xsd:float ;
        om2:hasUnit            om2:kilobyte .

sto:TC_91  a          sto:TechnicalCommittee , owl:NamedIndividual ;
        rdfs:comment  "To prepare international standards on design, manufacturing and testing of electronic assemblies including the requirements and tests for materials and components used to manufacture circuit boards and electronic assemblies, as well as the formats of electronic data and libraries for describing these products and processes."@en ;
        rdfs:label    "TC 91"@en ;
        sto:hasTitle  "Electronics assembly technology"@en , "Electronics assembly technology\n"@en .

sto:IEC_62337  a                 sto:Standard , owl:NamedIndividual ;
        rdfs:comment             "Commissioning of electrical, instrumentation and control systems in the process industry - Specific phases and milestones."@en ;
        rdfs:label               "IEC 62337"@en ;
        sto:hasClassification    rami:Lifecycle_Status , rami:Enterprise , rami:Work_Centers , rami:Functional , sto:ProductionSystemModelData , rami:Conditional_Monitoring ;
        sto:hasDomain            sto:IndustrialAutomation ;
        sto:hasOfficialResource  "https://webstore.iec.ch/publication/6871" ;
        sto:hasPublicationDate   "2012-02-22"^^xsd:date ;
        sto:hasPublisher         sto:IEC .

sto:FileSizeIEC_60870_P6_S501_1995
        a                      om2:Measure , owl:NamedIndividual ;
        rdfs:comment           "Specifies the file size of the document for standard IEC 60870-6-501:1995"@en ;
        rdfs:label             "FileSize IEC 60870-6-501:1995"@en ;
        om2:hasNumericalValue  "578.0"^^xsd:float ;
        om2:hasUnit            om2:kilobyte .

deo:Motivation  a  owl:Class .

sto:AdministrationShell
        a             owl:NamedIndividual , sto:StandardizationFramework ;
        rdfs:comment  "Represents the classifications of the standards according to the submodels of the administration shell."@en ;
        rdfs:label    "Administration Shell"@en .

sto:IEC_60382_1991  a                owl:NamedIndividual , sto:Standard ;
        rdfs:comment                 "Applies to analogue pneumatic signals used in process control systems to transmit information between the elements of systems and gives definitions, units and the recommended value of the range of the analogue pneumatic signal."@en ;
        rdfs:label                   "IEC 60382:1991"@en ;
        sto:hasAvailableLanguage     "English/French"@en ;
        sto:hasEdition               "2.0"^^xsd:float ;
        sto:hasFileSize              sto:FileSizeIEC_60382_1991 ;
        sto:hasICS                   sto:ICS_25_040_40 ;
        sto:hasImplementationFormat  "Document"@en ;
        sto:hasOfficialResource      <https://webstore.iec.ch/publication/1950> ;
        sto:hasPages                 9 ;
        sto:hasPublicationDate       "1991-11-01"^^xsd:date ;
        sto:hasPublisher             sto:IEC ;
        sto:hasStabilityDate         "2018"^^xsd:gYear ;
        sto:hasStatus                "Valid"@en ;
        sto:hasTag                   "IEC 60382:1991"@en ;
        sto:hasTechnicalCommittee    sto:TC_65 ;
        sto:hasTitle                 "Analogue pneumatic signal for process control systems"@en .

dbr:Cologne  a  owl:NamedIndividual .

sto:ProductCatalogData
        a                  owl:NamedIndividual , sto:ProductDevelopmentLifeCycle ;
        rdfs:comment       "Product catalog data standards support the description of particular instances of products or parts in a uniform, vendor-neutral way."@en ;
        rdfs:label         "Product Catalog Data"@en ;
        sto:isDescribedin  sto:NISTInitiative .

sto:IEC_60870_P5_S104_2016
        a                          owl:NamedIndividual , sto:Standard ;
        rdfs:comment               "IEC 60870-5-104:2006+A1:2016 Defines a telecontrol companion standard that enables interoperability among compatible telecontrol equipment. Applies to telecontrol equipment and systems with coded bit serial data transmission for monitoring and controlling geographically widespread processes. \nThis publication is of high relevance for Smart Grid. This consolidated version consists of the second edition (2006) and its amendment 1 (2012). Therefore, no need to order amendment in addition to this publication."@en ;
        rdfs:label                 "IEC 60870-5-104:2006"@en ;
        sto:hasAvailableLanguage   "English/French"@en ;
        sto:hasDBpediaResource     <https://dbpedia.org/resource/IEC_60870> , <null//dbpedia.org/resource/IEC_60870> ;
        sto:hasEdition             "2.1"^^xsd:float ;
        sto:hasFileSize            sto:FileSizeIEC_60870_P5_S104_2016 ;
        sto:hasICS                 sto:ICS_33_200 ;
        sto:hasOfficialResource    <null//webstore.iec.ch/publication/25035> , <https://webstore.iec.ch/publication/25035> ;
        sto:hasPages               "281"^^xsd:int ;
        sto:hasPublicationDate     "2016-06-159"^^xsd:date ;
        sto:hasPublisher           sto:IEC ;
        sto:hasStabilityDate       "2018"^^xsd:gYear ;
        sto:hasTag                 "IEC 60870-5-104:2006"@en ;
        sto:hasTechnicalCommittee  sto:TC_57 ;
        sto:hasTitle               "Telecontrol equipment and systems - Part 5-104: Transmission protocols - Network access for IEC 60870-5-101 using standardtransport profiles"@en ;
        sto:hasWikipediaArticle    <https://en.wikipedia.org/wiki/IEC_60870> , <null//en.wikipedia.org/wiki/IEC_60870> .

sto:IEC_29182-1  a               sto:Standard , owl:NamedIndividual ;
        rdfs:comment             "ISO/IEC 29182-1: provides a general overview of the characteristics of a sensor network and the organization of the entities that comprise such a network. It also describes the general requirements that are identified for sensor networks."@en ;
        rdfs:label               "IEC 29182-1"@en ;
        sto:hasClassification    rami:FieldDevice , rami:ControlDevice , rami:Communications , sto:ProductionSystemModelData ;
        sto:hasDomain            sto:M2M ;
        sto:hasOfficialResource  "https://www.iso.org/standard/45261.html" ;
        sto:hasPublicationDate   "2013-06-01"^^xsd:date ;
        sto:hasPublisher         sto:ISO , sto:IEC ;
        sto:relatedTo            sto:IEC_61158 .

dcterms:issued  a  owl:AnnotationProperty .

sto:hasDBpediaResource
        a             owl:DatatypeProperty ;
        rdfs:comment  "Instance's DBpedia Resource"@en ;
        rdfs:label    "has DBpedia Resource"@en ;
        rdfs:range    xsd:string .

sto:IEC_60870_P2_S2_1996
        a                          sto:Standard , owl:NamedIndividual ;
        rdfs:comment               "Applies to telecontrol equipment and systems with coded bit serial data transmission for monitoring and control of geographically wides pread processes. Specifies classes for environmental conditions under which the various components of the systems have to operate."@en ;
        rdfs:label                 "IEC 60870-2-2:1996"@en ;
        sto:hasAvailableLanguage   " Spanish"@en , "English/French"@en ;
        sto:hasDBpediaResource     <https://dbpedia.org/resource/IEC_60870> , <null//dbpedia.org/resource/IEC_60870> ;
        sto:hasEdition             "1.0"^^xsd:float ;
        sto:hasFileSize            sto:FileSizeIEC_60870_1996_P2_S2 ;
        sto:hasICS                 sto:ICS_33_200 , sto:ICS_29_020 ;
        sto:hasOfficialResource    <null//webstore.iec.ch/publication/3739> , <https://webstore.iec.ch/publication/3739> ;
        sto:hasPages               "33"^^xsd:int ;
        sto:hasPublicationDate     "1996-08-232"^^xsd:date ;
        sto:hasPublisher           sto:IEC ;
        sto:hasStabilityDate       "2018"^^xsd:gYear ;
        sto:hasTag                 "IEC 60870-2-2:1996"@en ;
        sto:hasTechnicalCommittee  sto:TC_57 ;
        sto:hasTitle               "Telecontrol equipment and systems - Part 2: Operating conditions -Section 2: Environmental conditions (climatic, mechanical and othernon electrical influences)"@en ;
        sto:hasWikipediaArticle    <null//en.wikipedia.org/wiki/IEC_60870> , <https://en.wikipedia.org/wiki/IEC_60870> .

sto:hasClassification
        a             owl:ObjectProperty ;
        rdfs:comment  "An Standard is isCategorizedBy a given Categorization Area which is connected to a specific Standarization Initiative"@en ;
        rdfs:domain   sto:Standard ;
        rdfs:label    "has Classification"@en ;
        rdfs:range    sto:StandardClassification .

sto:FileSizeIEC_61010_P2_S202_2016
        a                      om2:Measure , owl:NamedIndividual ;
        rdfs:comment           "Specifies the file size of the document for standard IEC 61010-2-202:2016."@en ;
        rdfs:label             "FileSize IEC 61010-2-202:2016"@en ;
        om2:hasNumericalValue  "1027.0"^^xsd:float ;
        om2:hasUnit            om2:kilobyte .

sto:IEC_62591  a                 owl:NamedIndividual , sto:Standard ;
        rdfs:comment             "Industrial networks - Wireless communication network and communication profiles."@en ;
        rdfs:label               "IEC 62591"@en ;
        sto:hasDBpediaResource   "http://dbpedia.org/page/WirelessHART" ;
        sto:hasOfficialResource  "https://webstore.iec.ch/publication/24433" ;
        sto:hasPublisher         sto:IEC ;
        sto:hasWikipediaArticle  "https://en.wikipedia.org/wiki/WirelessHART" .

sto:MOMLevel  a          owl:NamedIndividual , sto:ISA95Level ;
        rdfs:comment     "Describes the MOM level according to the ISA95 level classification."@en ;
        rdfs:label       "MOM Level"@en ;
        skos:definition  "Manufacturing Operation Management Level according to ISA 95"@en .

sto:ISO_14443  a      owl:NamedIndividual , sto:Standard ;
        rdfs:comment  "ISO 14443 Identification cards -- Contactless integrated circuit cards -- Proximity cards is an international standard that defines proximity cards used for identification, and the transmission protocols for communicating with it"@en ;
        rdfs:label    "ISO 14443"@en .

dcterms:hasLicense  a       owl:ObjectProperty ;
        rdfs:comment        "A legal document giving official permission to do something with the resource."@en , "A legal document giving official permission to do something with the resource. In this ontology denotes the license of a Standard."@en , "Represent the license document for a given Standard"@en ;
        rdfs:domain         sto:Standard ;
        rdfs:isDefinedBy    dcterms: ;
        rdfs:label          "has License"@en ;
        rdfs:range          dcterms:LicenseDocument ;
        dcterms:hasVersion  <http://dublincore.org/usage/terms/history/#license-002> ;
        dcterms:issued      "2004-06-14"^^xsd:date ;
        dcterms:modified    "2017-12-19"^^xsd:date .

sto:ASME_Y1441  a                owl:NamedIndividual , sto:Standard ;
        rdfs:comment             "ASME Y14.41 establishs requirements for model-based definition upon CAD software and those who use CAD software to create product definition within the 3D model."@en ;
        rdfs:label               "ASME Y14.41"@en ;
        sto:hasClassification    sto:ModelingPractice ;
        sto:hasDBpediaResource   "http://dbpedia.org/resource/ASME_Y14.41" ;
        sto:hasOfficialResource  "https://www.asme.org/products/codes-standards/y1441-2012-digital-product-definition-data" ;
        sto:hasPublisher         sto:ASME ;
        sto:hasWikipediaArticle  "https://en.wikipedia.org/wiki/ASME_Y14.41" .

sto:ICS_01_060  a     owl:NamedIndividual , sto:InternationalClassificationForStandards ;
        rdfs:comment  "This is ICS for Quantities and units"@en ;
        rdfs:label    "ICS 01.060"@en ;
        sto:hasTitle  "Quantities and units "@en .

sto:IEC_60839_P7_3  a              sto:Standard , owl:NamedIndividual ;
        rdfs:comment               "Specifies the data link layer message structure, formats and transmission procedures which should be used at standard serial data interfaces in alarm transmission systems where the transmission network employed does not offer a standard protocol. Is necessary in order to ensure compatibility of equipment from different suppliers."@en ;
        rdfs:label                 "IEC 60839-7-3:2001"@en ;
        sto:hasAvailableLanguage   " English/French"@en , "English"@en ;
        sto:hasEdition             "1.0"^^xsd:float ;
        sto:hasFileSize            sto:FileSizeIEC_60839_P7_3 ;
        sto:hasICS                 sto:ICS_13_320 ;
        sto:hasOfficialResource    <null//webstore.iec.ch/publication/3671> ;
        sto:hasPages               "29"^^xsd:int ;
        sto:hasPublicationDate     "68/03/01"^^xsd:date ;
        sto:hasPublisher           sto:IEC ;
        sto:hasStabilityDate       "2018"^^xsd:gYear ;
        sto:hasTag                 "IEC 60839-7-3:2001"@en ;
        sto:hasTechnicalCommittee  sto:TC_79 ;
        sto:hasTitle               "Alarm systems - Part 7-3: Message formats and protocols for serial data interfaces in alarm transmission systems - Common data link layer protocol"@en .

sto:ISO_22400  a                 owl:NamedIndividual , sto:Standard ;
        rdfs:comment             "Automation systems and integration -- Key performance indicators (KPIs) for manufacturing operations management."@en ;
        rdfs:label               "ISO 22400"@en ;
        sto:hasClassification    rami:ConnectedWorld , rami:FieldDevice , rami:Enterprise , rami:WorkCenter , rami:LifeCycle_Status , rami:Conditional_Monitoring , rami:Station , rami:ControlDevice , rami:Business ;
        sto:hasDomain            sto:IndustrialAutomation ;
        sto:hasOfficialResource  "https://www.iso.org/standard/54497.html" ;
        sto:hasPublicationDate   "2014-01-01"^^xsd:date ;
        sto:hasPublisher         sto:ISO ;
        sto:relatedTo            sto:IEC_62541 .

sto:FileSizeIEC_60870_P6_S502_1995
        a                      om2:Measure , owl:NamedIndividual ;
        rdfs:comment           "Specifies the file size of the document for standard IEC 60870-6-502:1995"@en ;
        rdfs:label             "FileSize IEC 60870-6-502:1995"@en ;
        om2:hasNumericalValue  "1963.0"^^xsd:float ;
        om2:hasUnit            om2:kilobyte .

sto:MIIT  a                      owl:NamedIndividual , sto:StandardOrganization ;
        rdfs:comment             "Ministry of Industry and Information Technology (MIIT) of the Chinese government, established in March 2008, is the state agency of the People's Republic of China responsible for regulation and development of the postal service, Internet, wireless, broadcasting, communications, production of electronic and information goods, software industry and the promotion of the national knowledge economy."@en ;
        sto:abbreviation         "MIIT" ;
        sto:belongsTo            dbr:China ;
        sto:formationDate        "2008-03-01"^^xsd:date ;
        sto:hasDBpediaResource   "http://dbpedia.org/page/Ministry_of_Industry_and_Information_Technology" ;
        sto:hasHeadquaterIn      dbr:Beijing ;
        sto:hasOfficialResource  "http://www.miit.gov.cn/" ;
        sto:hasWikipediaArticle  "https://en.wikipedia.org/wiki/Ministry_of_Industry_and_Information_Technology" ;
        sto:orgName              "Ministry of Industry and Information Technology"@en .

sto:FileSizeIEC_60255_149_2013
        a                      owl:NamedIndividual , om2:Measure ;
        rdfs:comment           "Specifies the file size of the document for standard IEC 60255-149:2013 "@en ;
        rdfs:label             "FileSize 60255-149:2013"@en ;
        om2:hasNumericalValue  "1722.0"^^xsd:float ;
        om2:hasUnit            om2:kilobyte .

sto:IEC_81714  a                 owl:NamedIndividual , sto:Standard ;
        rdfs:comment             "ISO/IEC 81714 Design of graphical symbols for use in the technical documentation of products -- Part 3: Classification of connect nodes, networks and their encoding-- specifies requirements concerning the classification of connect nodes assigned to graphical symbols, being a representation of functional and product concepts."@en ;
        rdfs:label               "IEC 81714"@en ;
        sto:hasClassification    sto:ModelingPractice , rami:Product , rami:Identification , rami:Engineering , rami:Asset ;
        sto:hasDomain            sto:CAD ;
        sto:hasOfficialResource  "https://www.iso.org/standard/40134.html" ;
        sto:hasPublicationDate   "2004-10-01"^^xsd:date ;
        sto:hasPublisher         sto:IEC , sto:ISO .

rami:AdminShellSubmodel
        a                 owl:Class ;
        rdfs:comment      "Describes the Administration Shell concept to organize/classify standards into submodels"@en ;
        rdfs:isDefinedBy  <https://www.plattform-i40.de/I40/Redaktion/EN/Downloads/Publikation/structure-of-the-administration-shell.pdf?__blob=publicationFile&v=7> ;
        rdfs:label        "Admin Shell Sub Model"@en ;
        rdfs:subClassOf   sto:StandardClassification .

sto:FileSizeIEC_61334_1996_P4_S42
        a                      om2:Measure , owl:NamedIndividual ;
        rdfs:comment           "Specifies the file size of the document for standard IEC 61334-4-42:1996"@en ;
        rdfs:label             "FileSize IEC 61334-4-42:1996"@en ;
        om2:hasNumericalValue  "305.0"^^xsd:float ;
        om2:hasUnit            om2:kilobyte .

sto:SCM  a                 owl:NamedIndividual , sto:BusinessCycleSCM ;
        rdfs:comment       "Describes Plan-Source-Make-Deliver-Return cycle for managing the manufacturing supply chain."@en ;
        rdfs:label         "Supply Chain Management"@en ;
        sto:isDescribedin  sto:NISTInitiative .

sto:EnterpriseLevel  a  owl:NamedIndividual , sto:ISA95Level ;
        rdfs:comment  "Describes the Enterprise level according to the ISA95 level classification."@en ;
        rdfs:label    "Enterprise Level"@en .

sto:IEC_60848  a                   sto:Standard , owl:NamedIndividual ;
        rdfs:comment               "IEC 60848:2013 defines the GRAFCET specification language for the functional description of the behaviour of the sequential part of a control system. It specifies the symbols and rules for the graphical representation of this language, as well as for its interpretation and has been prepared for automated production systems of industrial applications. This third edition cancels and replaces the second edition published in 2002 and constitutes a global technical revision with the extended definition of the concept of variables introducing: internal variable, input variable and output variable."@en ;
        rdfs:label                 "IEC 60848:2013"@en ;
        sto:hasAvailableLanguage   "English/French"@en ;
        sto:hasEdition             "3.0"^^xsd:float ;
        sto:hasFileSize            sto:FileSizeIEC_60848 ;
        sto:hasICS                 sto:ICS_29_020 ;
        sto:hasOfficialResource    <null//webstore.iec.ch/publication/3684> ;
        sto:hasPages               "109"^^xsd:int ;
        sto:hasPublicationDate     "58/02/13"^^xsd:date ;
        sto:hasPublisher           sto:IEC ;
        sto:hasStabilityDate       "2020"^^xsd:gYear ;
        sto:hasTag                 "IEC 60848:2013"@en ;
        sto:hasTechnicalCommittee  sto:TC_3 ;
        sto:hasTitle               "GRAFCET specification language for sequential function charts"@en .

sto:TC_25  a          owl:NamedIndividual , sto:TechnicalCommittee ;
        rdfs:comment  "To prepare international standards on quantities and units to be used in electrical technology. Such standards may relate to their definitions, names, letter symbols and use; to the relations in which they appear; and to the signs and symbols used with them."@en ;
        rdfs:label    "TC 25"@en ;
        sto:hasTitle  "Quantities and units"@en .

sto:IEC_61334_P6_2000
        a                          owl:NamedIndividual , sto:Standard ;
        rdfs:comment               "Defines a set of encoding rules that may be used to derive the specification of a transfer syntax for values of types defined in the DLMS core standard using the ASN.1 notation (see IEC 61334-4-41).\nThis publication is of high relevance for Smart Grid."@en ;
        rdfs:label                 "IEC 61334-6:2000"@en ;
        sto:hasAvailableLanguage   "English/French"@en ;
        sto:hasDBpediaResource     <null//dbpedia.org/resource/IEC_61334> , <https://dbpedia.org/resource/IEC_61334> ;
        sto:hasEdition             "1.0"^^xsd:float ;
        sto:hasFileSize            sto:FileSizeIEC_61334_2000_P6 ;
        sto:hasICS                 sto:ICS_29_240_20 , sto:ICS_33_200 ;
        sto:hasOfficialResource    <https://webstore.iec.ch/publication/5313> , <null//webstore.iec.ch/publication/5313> ;
        sto:hasPages               "75"^^xsd:int ;
        sto:hasPublicationDate     "2000-06-168"^^xsd:date ;
        sto:hasPublisher           sto:IEC ;
        sto:hasStabilityDate       "2018"^^xsd:gYear ;
        sto:hasTag                 "IEC 61334-6:2000"@en ;
        sto:hasTechnicalCommittee  sto:TC_57 ;
        sto:hasTitle               "Distribution automation using distribution line carrier systems - Part 6: A-XDR encoding rule"@en ;
        sto:hasWikipediaArticle    <null//en.wikipedia.org/wiki/IEC_61334> , <https://en.wikipedia.org/wiki/IEC_61334> .

skos:altLabel  a  owl:AnnotationProperty .

sto:ICS_13_110  a     sto:InternationalClassificationForStandards , owl:NamedIndividual ;
        rdfs:comment  "This is ICS for Safety of machinery "@en , "This is ICS for “Safety of machinery  ”"@en ;
        rdfs:label    "ICS 13.110"@en ;
        sto:hasTitle  "Safety of machinery"@en , "Safety of machinery "@en .

sto:hasObjective  a   owl:DatatypeProperty ;
        rdfs:comment  "Specifies the objectives for the different ISA 95 levels."@en ;
        rdfs:domain   sto:ISA95Level ;
        rdfs:label    "has Objective"@en ;
        rdfs:range    xsd:string .

sto:ICS_31_020  a     owl:NamedIndividual , sto:InternationalClassificationForStandards ;
        rdfs:comment  "This is ICS for Electronic components in general "@en ;
        rdfs:label    "ICS 31.020"@en ;
        sto:hasTitle  "Electronic components in general "@en .

sto:IEC_61512  a                 owl:NamedIndividual , sto:Standard ;
        rdfs:comment             "Batch control - Models and terminology"@en ;
        rdfs:label               "IEC 61512"@en ;
        sto:hasClassification    rami:WorkCenter , rami:Product , rami:Station , rami:ControlDevice ;
        sto:hasDBpediaResource   "http://dbpedia.org/resource/ISA-88" ;
        sto:hasMotivation        "The standard sought to address the following problems: lack of a universal model for batch control, difficulty in communicating user requirement, integration among batch automation suppliers, difficulty in batch control configuration."@en ;
        sto:hasOfficialResource  "https://webstore.iec.ch/publication/5528" ;
        sto:hasPublisher         sto:IEC ;
        sto:hasTag               "ISA-88"@en ;
        sto:hasWikipediaArticle  "https://en.wikipedia.org/wiki/ISA-88" .

sto:ISO_20140_5  a               owl:NamedIndividual , sto:Standard ;
        rdfs:comment             "Automation systems and integration -- Evaluating energy efficiency and other factors of manufacturing systems that influence the environment"@en ;
        rdfs:label               "ISO 20140-5"@en ;
        sto:hasClassification    rami:EnergyEfficiency ;
        sto:hasOfficialResource  "http://www.iso.org/iso/catalogue_detail.htm?csnumber=54809" ;
        sto:hasPublisher         sto:ISO ;
        sto:hasTag               "Energy Efficiency"@en .

sto:FileSizeIEC_60286_3_2013
        a                      owl:NamedIndividual , om2:Measure ;
        rdfs:comment           "Specifies the file size of the document for standard IEC IEC 60286-3:2013 "@en ;
        rdfs:label             "FileSize IEC 60286-3:2013  "@en ;
        om2:hasNumericalValue  "1764.0"^^xsd:float ;
        om2:hasUnit            om2:kilobyte .

sto:abbreviation  a   owl:DatatypeProperty ;
        rdfs:comment  "Abbreviated  name of the thing."@en ;
        rdfs:domain   owl:thing ;
        rdfs:label    "has Abbreviated Name"@en ;
        rdfs:range    rdf:PlainLiteral .

dc11:rights  a  owl:AnnotationProperty .

sto:IEC_60050_1998  a                owl:NamedIndividual , sto:Standard ;
        rdfs:comment                 "It has the status of a horizontal standard in accordance with IEC Guide 108."@en ;
        rdfs:label                   "IEC 60050-101:1998"@en ;
        sto:hasAvailableLanguage     "English/French, Spanish"@en ;
        sto:hasDBpediaResource       <http://dbpedia.org/page/International_Electrotechnical_Vocabulary> ;
        sto:hasEdition               "2.0"^^xsd:float ;
        sto:hasFileSize              sto:FileSizeIEC_60050_1998 ;
        sto:hasICS                   sto:ICS_01_040_07 ;
        sto:hasImplementationFormat  "Document"@en ;
        sto:hasOfficialResource      <https://webstore.iec.ch/publication/159> ;
        sto:hasPages                 129 ;
        sto:hasPublicationDate       "1998-04-30"^^xsd:date ;
        sto:hasPublisher             sto:IEC ;
        sto:hasStatus                "Replaced"@en ;
        sto:hasTag                   "IEC 60050-101:1998"@en ;
        sto:hasTechnicalCommittee    sto:TC_1 ;
        sto:hasTitle                 "International Electrotechnical Vocabulary - Part 101: Mathematics"@en ;
        sto:hasWikipediaArticle      <https://en.wikipedia.org/wiki/International_Electrotechnical_Vocabulary> .

cc:attributionURL  a  owl:AnnotationProperty .

sto:FileSizeIEC_60870_P5_S103_1997
        a                      om2:Measure , owl:NamedIndividual ;
        rdfs:comment           "Specifies the file size of the document for standard IEC 60870-5-103:1997"@en ;
        rdfs:label             "FileSize IEC 60870-5-103:1997"@en ;
        om2:hasNumericalValue  "964.0"^^xsd:float ;
        om2:hasUnit            om2:kilobyte .

sto:IEC_61499  a                 owl:NamedIndividual , sto:Standard ;
        rdfs:comment             "Function Blocks - Architecture Related Applications http://www.eclipse.org/4diac/ (sourceforge.net/projects/oooneida-fbench/) http://timeme.io/  not accepted by the Industry yet. http://www.holobloc.com/Proposed for IEC to overcome the restricctions of IEC 61131"@en ;
        rdfs:label               "IEC 61499"@en ;
        sto:hasClassification    rami:FieldDevice , rami:ControlDevice ;
        sto:hasDBpediaResource   "http://dbpedia.org/resource/IEC_61499" ;
        sto:hasMotivation        "Functional description, informational representation and communication mapping of application functionality. This standard describes how a distributed control application is composed of functional units (FB), which are executed in different context. It may help to describe how functions are distributed between different I40-Components and how the execution of the functions between the different I40-Components is controled."@en ;
        sto:hasOfficialResource  "https://webstore.iec.ch/publication/5506" ;
        sto:hasPublisher         sto:IEC ;
        sto:hasTag               "FBs distributed systems"@en ;
        sto:hasWikipediaArticle  "https://en.wikipedia.org/wiki/IEC_61499" ;
        sto:relatedTo            sto:IEC_62541 , sto:IEC_61131 .

sto:IEC_61000_P6_S2_2016
        a                          sto:Standard , owl:NamedIndividual ;
        rdfs:comment               "IEC 61000-6-2:2016 RLV contains the International Standard and its Redline version. The Redline version is available in English only. The Redline version provides you with a quick and easy way to compare all the changes between this standard and its previous edition. The Redline version is not an official IEC Standard, only the current version of the standard is to be considered the official document.\nIEC 61000-6-2:2016 for EMC immunity requirements applies to electrical and electronic equipment intended for use in industrial locations, as described below. Immunity requirements in the frequency range 0 Hz to 400 GHz are covered. No tests need to be performed at frequencies where no requirements are specified. This generic EMC immunity standard is applicable if no relevant dedicated product or product-family EMC immunity standard exists. This third edition cancels and replaces the second edition published in 2005. This edition constitutes a technical revision."@en ;
        rdfs:label                 "IEC 61000-6-2:2016"@en ;
        sto:hasAvailableLanguage   "English"@en ;
        sto:hasEdition             "3.0"^^xsd:float ;
        sto:hasFileSize            sto:FileSizeIEC_61000_P6_S2_2016 ;
        sto:hasICS                 sto:ICS_33_100_20 ;
        sto:hasOfficialResource    <https://webstore.iec.ch/publication/25629> , <null//webstore.iec.ch/publication/25629> ;
        sto:hasPages               "57"^^xsd:int ;
        sto:hasPublicationDate     "2016-08-223"^^xsd:date ;
        sto:hasPublisher           sto:IEC ;
        sto:hasStabilityDate       "2020"^^xsd:gYear ;
        sto:hasTag                 "IEC 61000-6-2:2016"@en ;
        sto:hasTechnicalCommittee  sto:TC_77 ;
        sto:hasTitle               "Electromagnetic compatibility (EMC) - Part 6-2: Generic standards - Immunity standard for industrial environments"@en .

sto:IEC_61850  a                 owl:NamedIndividual , sto:Standard ;
        rdfs:comment             "IEC 61850 is a standard for vendor-agnostic engineering of the configuration of Intelligent Electronic Devices for electrical substation automation systems to be able to communicate with each other.."@en ;
        rdfs:label               "IEC 61850"@en ;
        sto:hasDBpediaResource   "http://dbpedia.org/page/IEC_61850" ;
        sto:hasOfficialResource  "https://webstore.iec.ch/publication/4550" ;
        sto:hasPublisher         sto:IEC ;
        sto:hasWikipediaArticle  "https://en.wikipedia.org/wiki/IEC_61850" .

sto:useStructureOf  a       owl:ObjectProperty ;
        rdfs:comment        "Standard A uses the structure of Standard B. For example, OPC UA uses Structure Of IEC_61804 (EDDL)"@en ;
        rdfs:label          "use Structure Of"@en ;
        rdfs:subPropertyOf  sto:relatedTo .

sto:FileSizeIEC_60870_1992_P5_S2
        a                      om2:Measure , owl:NamedIndividual ;
        rdfs:comment           "Specifies the file size of the document for standard IEC 60870-5-2:1992"@en ;
        rdfs:label             "FileSize IEC 60870-5-2:1992"@en ;
        om2:hasNumericalValue  "3658.0"^^xsd:float ;
        om2:hasUnit            om2:kilobyte .

sto:ISO_15704  a                 sto:Standard , owl:NamedIndividual ;
        rdfs:comment             "Identifies requirements for enterprise-reference architectures and methodologies"@en ;
        rdfs:label               "ISO 15704"@en ;
        sto:hasClassification    rami:Business , rami:Other , rami:Enterprise ;
        sto:hasDomain            sto:IndustrialAutomation ;
        sto:hasOfficialResource  "https://www.iso.org/standard/28777.html" ;
        sto:hasPublicationDate   "2000-06-01"^^xsd:date ;
        sto:hasPublisher         sto:ISO ;
        sto:relatedTo            sto:ISO_19439 , sto:ISO_13374 .

rami:LifecycleStatus  a    owl:NamedIndividual , rami:AdminShellSubmodel ;
        sto:isDescribedin  sto:AdministrationShell .

sto:ETSI_ULE  a                  sto:Standard , owl:NamedIndividual ;
        rdfs:comment             "DECT Ultra Low Energy (DECT ULE) is a technology based on DECT, and intended for Machine-to-Machine communications such as Home and Industrial automation. The main characteristics of the technology are ultra-low power consumption (much lower than IEEE 802.11) and wider coverage (much wider than IEEE 802.15 and Bluetooth Low Energy)."@en ;
        rdfs:label               "Ultra Low Energy"@en ;
        sto:hasDBpediaResource   "http://dbpedia.org/resource/ULE_-_Ultra_Low_Energy" ;
        sto:hasDeveloper         sto:ETSI ;
        sto:hasOfficialResource  "http://www.etsi.org/technologies-clusters/technologies/dect/dect-ule" ;
        sto:hasPublisher         sto:ETSI ;
        sto:hasTag               "ETSI ULE"@en ;
        sto:hasWikipediaArticle  "https://en.wikipedia.org/wiki/DECT_Ultra_Low_Energy" ;
        sto:relatedTo            sto:ETSI_DECT .

sto:edition  a  owl:AnnotationProperty .

sto:FileSizeIEC_60027_2006
        a                      owl:NamedIndividual , om2:Measure ;
        rdfs:comment           "Specifies the file size of the document for standard IEC 60027:2006"@en ;
        rdfs:label             "FileSize IEC 60027:2006"@en ;
        om2:hasNumericalValue  "661.0"^^xsd:float ;
        om2:hasUnit            om2:kilobyte .

sto:isImplementationOf
        a                   owl:ObjectProperty ;
        rdfs:comment        "Represent the relation that connects two standards when standard A is the implementation of standard B, e.g., B2MML isImplementationOf ISA-95."@en ;
        rdfs:label          "is Implementation Of"@en ;
        rdfs:subPropertyOf  sto:relatedTo .

sto:ProcessPlanning  a  owl:NamedIndividual .

sto:FileSizeIEC_60870_P6_S702_2014
        a                      om2:Measure , owl:NamedIndividual ;
        rdfs:comment           "Specifies the file size of the document for standard IEC 60870-6-702:2014"@en ;
        rdfs:label             "FileSize IEC 60870-6-702:2014"@en ;
        om2:hasNumericalValue  "1374.0"^^xsd:float ;
        om2:hasUnit            om2:kilobyte .

sto:FileSizeIEC_61334_1998_P4_S61
        a                      om2:Measure , owl:NamedIndividual ;
        rdfs:comment           "Specifies the file size of the document for standard IEC 61334-4-61:1998"@en ;
        rdfs:label             "FileSize IEC 61334-4-61:1998"@en ;
        om2:hasNumericalValue  "753.0"^^xsd:float ;
        om2:hasUnit            om2:kilobyte .

sto:OPC_Foundation  a            owl:NamedIndividual , sto:StandardOrganization ;
        rdfs:comment             "Is an industry consortium that creates and maintains standards for open connectivity of industrial automation devices and systems, such as industrial control systems and process control generally"@en ;
        rdfs:label               "OPC Foundation"@en ;
        sto:abbreviation         "OPC" ;
        sto:formationDate        "1994-01-01"^^xsd:date ;
        sto:hasDBpediaResource   "http://dbpedia.org/page/OPC_Foundation" ;
        sto:hasHeadquaterIn      dbr:_Arizona ;
        sto:hasOfficialResource  "https://opcfoundation.org/" ;
        sto:hasWikipediaArticle  "https://en.wikipedia.org/wiki/OPC_Foundation" ;
        sto:orgName              "OPC Foundation"@en .

foaf:Organization  a  owl:Class .

sto:TechnicalCommittee
        a                 owl:Class , owl:NamedIndividual ;
        rdfs:comment      "Specifies the representitive code name of the Technical Committee that covers a Standard for e.g, TC 1, SC 3C. Many thousand experts carry out standardization work in the IEC in TCs (technical committees) and SCs (subcommittees), in hundreds of working groups, project and maintenance teams. They represent the national electrotechnical needs of IEC Member countries and of many Affiliates at the global level in the IEC. These technical experts are sent by industry, governments, test and research laboratories, academia and even consumer groups to work on the global, neutral and independent platform of the IEC. That's where they develop globally relevant, voluntary, consensus based IEC International Standards."@en ;
        rdfs:isDefinedBy  sto:IEC ;
        rdfs:label        "Technical Committe"@en ;
        rdfs:seeAlso      <http://www.iec.ch/dyn/www/f?p=103:62:9979528650478:::62:FSP_ORG_ID,FSP_LANG_ID:,25> ;
        skos:note         "1.sto:       a property explaining that TC and SC are managed by SMB (Standardization Management Board) needs to be added" ;
        sto:abbreviation  "TC" ;
        sto:hasTitle      xsd:string .

sto:ICS_29_020  a     sto:InternationalClassificationForStandards , owl:NamedIndividual ;
        rdfs:comment  "This is ICS for Electrical engineering in general"@en , "This is ICS for “Electrical engineering in general”"@en ;
        rdfs:label    "ICS 29.020"@en ;
        sto:hasTitle  "Electrical engineering in general "@en .

sto:ISO_15746  a                 sto:Standard , owl:NamedIndividual ;
        rdfs:comment             "Automation systems and integration -- Integration of advanced process control and optimization capabilities for manufacturing systems."@en ;
        rdfs:label               "ISO 15746"@en ;
        sto:hasClassification    rami:FieldDevice , rami:Information , rami:Integration , sto:ProductLifeCycleManagement , rami:Engineering , rami:Product , rami:Communication , rami:Functional , rami:ControlDevice ;
        sto:hasDomain            sto:IndustrialAutomation ;
        sto:hasOfficialResource  "https://www.iso.org/standard/61131.html" ;
        sto:hasPublicationDate   "2015-04-01"^^xsd:date ;
        sto:hasPublisher         sto:ISO ;
        sto:relatedTo            sto:ISO_15926 .

sto:TC_79  a          owl:NamedIndividual , sto:TechnicalCommittee ;
        rdfs:comment  "To prepare international standards for the protection of buildings, persons, areas and properties against fraudulent actions having the purpose to enter in a place or to take or to use something without permission and other threat related to persons.The scope includes, but is not limited to equipment and systems, either used by ordinary persons or by trained people in the following residential and non residential applications:- Access control systems- Alarm transmission systems- Video surveillance systems- Combined and/or integrated systems even including fire alarm systems*- Fire detection and fire alarm systems*- Intruder and hold-up alarm systems- Remote receiving and/or surveillance centres- Social alarm systems.These systems can be used for providing a local or remote alarm; they can be used for calling private guards, social assistance, fire brigade or police force. They can be used for recording and transmission of dated or undated information, sounds, pictures of places and people for surveillance purposes. The standards cover:- terminology;- technical characteristics regarding performance criteria, reliable operation, installation, maintenance;- testing for detection, monitoring, recording, triggering an alarm and transmission to a remote centre including procedures and protocols for communication.Electrical safety, environmental conditions and behaviour of alarm systems regarding electromagnetic compatibility are also considered with reference to the appropriate standards (e.g. Guide ISO/IEC 51).* ISO/TC21/SC3 is in charge of the production of standards for \"Fire detection and alarm systems\"."@en ;
        rdfs:label    "TC 79"@en ;
        sto:hasTitle  "Alarm and electronic security systems"@en .

sto:FileSizeIEC_60286_5_2018
        a                      owl:NamedIndividual , om2:Measure ;
        rdfs:comment           "Specifies the file size of the document for standard IEC IEC 60286-5:2018 "@en ;
        rdfs:label             "FileSize IEC 60286-5:2018  "@en ;
        om2:hasNumericalValue  "3481.0"^^xsd:float ;
        om2:hasUnit            om2:kilobyte .

muto:Tag  a     owl:Class .

sto:hasTag  a         owl:ObjectProperty , owl:DatatypeProperty ;
        rdfs:comment  "Points to the identification of the standards"@en ;
        rdfs:domain   sto:Publication ;
        rdfs:label    "has Tag"@en ;
        rdfs:range    muto:Tag , rdfs:Literal .

sto:FileSizeIEC_61334_1996_P3_S22
        a                      om2:Measure , owl:NamedIndividual ;
        rdfs:comment           "Specifies the file size of the document for standard IEC 61334-3-22:2001"@en ;
        rdfs:label             "FileSize IEC 61334-4-1:1996"@en ;
        om2:hasNumericalValue  "165.0"^^xsd:float ;
        om2:hasUnit            om2:kilobyte .

rami:WorkCenter  a         owl:NamedIndividual , rami:RAMIHierarchyLevel ;
        sto:isDescribedin  sto:RAMI40 .

sto:ASAM_ODS  a                  owl:NamedIndividual , sto:Standard ;
        rdfs:comment             "Set up a test data management system on top of test systems that produce measured or calculated data from testing activities"@en ;
        rdfs:label               "ASAM ODS"@en ;
        sto:hasOfficialResource  "https://wiki.asam.net/display/STANDARDS/ASAM+ODS" ;
        sto:hasPublisher         sto:ASAM .

sto:SCOR  a                      owl:NamedIndividual , sto:Standard ;
        rdfs:comment             "APICS Supply Chain Operations Reference."@en ;
        rdfs:label               "SCOR"@en ;
        sto:hasClassification    sto:SCM ;
        sto:hasDBpediaResource   "http://dbpedia.org/page/Supply-chain_operations_reference" ;
        sto:hasDeveloper         sto:APICS ;
        sto:hasOfficialResource  "http://www.apics.org/apics-for-business/products-and-services/apics-scc-frameworks/scor" ;
        sto:hasTag               "SCOR"@en ;
        sto:hasWikipediaArticle  "https://en.wikipedia.org/wiki/Supply-chain_operations_reference" .

sto:IEC_60870_P6_S2_1995
        a                          sto:Standard , owl:NamedIndividual ;
        rdfs:comment               "Considers the standards related to layers 1-4 of the OSI reference model and describes the role and the functions carried out by each layer.\nThis publication is of high relevance for Smart Grid."@en ;
        rdfs:label                 "IEC 60870-6-2:1995"@en ;
        sto:hasAvailableLanguage   "English/French"@en ;
        sto:hasDBpediaResource     <https://dbpedia.org/resource/IEC_60870> , <null//dbpedia.org/resource/IEC_60870> ;
        sto:hasEdition             "1.0"^^xsd:float ;
        sto:hasFileSize            sto:FileSizeIEC_60870_P6_S2_1995 ;
        sto:hasICS                 sto:ICS_33_200 ;
        sto:hasOfficialResource    <null//webstore.iec.ch/publication/3757> , <https://webstore.iec.ch/publication/3757> ;
        sto:hasPages               "83"^^xsd:int ;
        sto:hasPublicationDate     "1995-10-304"^^xsd:date ;
        sto:hasPublisher           sto:IEC ;
        sto:hasStabilityDate       "2018"^^xsd:gYear ;
        sto:hasTag                 "IEC 60870-6-2:1995"@en ;
        sto:hasTechnicalCommittee  sto:TC_57 ;
        sto:hasTitle               "Telecontrol equipment and systems - Part 6: Telecontrol protocols compatible with ISO standards and ITU-T recommendations - Section 2: Use of basic standards (OSI layers 1-4)"@en ;
        sto:hasWikipediaArticle    <null//en.wikipedia.org/wiki/IEC_60870> , <https://en.wikipedia.org/wiki/IEC_60870> .

sto:ISA95  a          owl:NamedIndividual , sto:StandardizationFramework ;
        rdfs:comment  "Describes the ISA95 as a Standarization Initiative that classifies Standards"@en ;
        rdfs:label    "ISA 95"@en .

sto:ICS_29_120_70  a  owl:NamedIndividual , sto:InternationalClassificationForStandards ;
        rdfs:comment  "This is ICS for Relays"@en ;
        rdfs:label    "ICS 29.120.70"@en ;
        sto:hasTitle  "Relays"@en .

rami:Business  a           owl:NamedIndividual , rami:RAMIITLayer ;
        sto:isDescribedin  sto:RAMI40 .

sto:FileSizeIEC_61010_P2_S201_2017
        a                      om2:Measure , owl:NamedIndividual ;
        rdfs:comment           "Specifies the file size of the document for standard IEC 61010-2-201:2017."@en ;
        rdfs:label             "FileSize IEC 61010-2-201:2017"@en ;
        om2:hasNumericalValue  "5743.0"^^xsd:float ;
        om2:hasUnit            om2:kilobyte .

sto:TC_103  a         owl:NamedIndividual , sto:TechnicalCommittee ;
        rdfs:comment  "Standardization of transmitting equipment for radiocom-\n\nmunications purposes and electronic devices employing similar\ntechniques. The standardization work deals with methods of\nmeasurement, safety requirements and transmitter control and\nInterconnection"@en ;
        rdfs:label    "TC 103"@en ;
        sto:hasTitle  "Transmitting equipment for radiocommunication"@en .

sto:FileSizeIEC_60286_4_2013
        a                      owl:NamedIndividual , om2:Measure ;
        rdfs:comment           "Specifies the file size of the document for standard IEC IEC 60286-4:2013 "@en ;
        rdfs:label             "FileSize IEC 60286-4:2013  "@en ;
        om2:hasNumericalValue  "1129.0"^^xsd:float ;
        om2:hasUnit            om2:kilobyte .

sto:FileSizeIEC_60839_P7_5
        a                      om2:Measure , owl:NamedIndividual ;
        rdfs:comment           "Specifies the file size of the document for standard IEC 60839-7-5:2001"@en ;
        rdfs:label             "FileSize IEC 60839-7-5:2001"@en ;
        om2:hasNumericalValue  "939.0"^^xsd:float ;
        om2:hasUnit            om2:kilobyte .

rami:ConnectedWorld  a     owl:NamedIndividual , rami:RAMIHierarchyLevel ;
        sto:isDescribedin  sto:RAMI40 .

sto:CrossLevel  a          owl:NamedIndividual , sto:ISA95Level ;
        rdfs:comment       "Describes the cross-level according to the ISA95 level classification. It means standards that are used at more than one level, e.g., manufacturing system security, etc"@en ;
        rdfs:label         "Cross Level"@en ;
        sto:isDescribedin  sto:ISA95 .

sto:ASAM  a                      owl:NamedIndividual , sto:StandardOrganization ;
        rdfs:comment             "Association for Standardization of Automation and Measuring Systems or ASAM is an incorporated association under German law. Its members are primarily international car manufacturers, suppliers and engineering service providers from the automotive industry. The association coordinates the development of technical standards, which are developed by working groups composed of experts from its member companies. ASAM pursues the vision that the tools of a development process chain can be freely interconnected and allow a seamless exchange of data. The standards define protocols, data models, file formats and application programming interfaces (APIs) for the use in the development and testing of automotive electronic control units. A large amount of popular tools in the areas of simulation, measurement, calibration and test automation are compliant to ASAM standards. Compliance shall guarantee interoperability of tools from different vendors, allow data exchange without the need for converters, and facilitate the exchange of unambiguous specification between customers and suppliers."@en ;
        rdfs:label               "ASAM" ;
        sto:abbreviation         "ASAM" ;
        sto:belongsTo            dbr:Germany ;
        sto:formationDate        "1998-12-01"^^xsd:date ;
        sto:hasDBpediaResource   "http://dbpedia.org/page/Association_for_Standardisation_of_Automation_and_Measuring_Systems" ;
        sto:hasDBpediaResource   <http://dbpedia.org/resource/Association_for_Standardisation_of_Automation_and_Measuring_Systems> ;
        sto:hasHeadquaterIn      dbr:Höhenkirchen-Siegertsbrunn ;
        sto:hasOfficialResource  <https://www.asam.net/> ;
        sto:hasWikipediaArticle  "https://en.wikipedia.org/wiki/Association_for_Standardisation_of_Automation_and_Measuring_Systems" ;
        sto:hasWikipediaArticle  <https://en.wikipedia.org/wiki/Association_for_Standardisation_of_Automation_and_Measuring_Systems> ;
        sto:orgName              "Association for Standardization of Automation and Measuring Systems"@en .

dbr:Chicago  a  owl:NamedIndividual .

skos:note  a    owl:AnnotationProperty .

sto:IEC_62061  a                 owl:NamedIndividual , sto:Standard ;
        rdfs:comment             "provides requirements that are applicable to the system level design of all types of machinery safety-related electrical control systems and also for the design of non-complex subsystems or devices."@en ;
        rdfs:label               "IEC 60061"@en ;
        sto:hasClassification    rami:Safety ;
        sto:hasDBpediaResource   "http://dbpedia.org/resource/IEC_62061" ;
        sto:hasOfficialResource  "https://webstore.iec.ch/publication/22797" ;
        sto:hasPublisher         sto:IEC ;
        sto:hasTag               "Safety of machinery"@en ;
        sto:hasWikipediaArticle  "https://en.wikipedia.org/wiki/IEC_62061" .

sto:IEC_62453  a                 owl:NamedIndividual , sto:Standard ;
        rdfs:comment             "Field device tool (FDT) interface specification - Overview and guidance"@en ;
        rdfs:label               "IEC 62453"@en ;
        sto:hasClassification    rami:ControlDevice , rami:Configuration , rami:Station , rami:FieldDevice ;
        sto:hasMotivation        "FDT is an interface for integration of devices into a system (e.g. control system or engineering system). The standard supports factory automation as well as process automation with a wide range of fieldbus protocols. The interface defines fieldbus-independent mechanisms for accessing data and functions of the devices."@en ;
        sto:hasOfficialResource  "https://webstore.iec.ch/publication/7040" ;
        sto:hasPublisher         sto:IEC ;
        sto:hasTag               "FDT"@en .

sto:FileSizeIEC_62832
        a                      owl:NamedIndividual , om2:Measure ;
        om2:hasNumericalValue  "2722.0"^^xsd:float ;
        om2:hasUnit            om2:kilobyte .

dbr:New_York_City  a  owl:NamedIndividual .

xsd:string  a   owl:NamedIndividual .

sto:ProductionSystemMaintenance
        a                  owl:NamedIndividual , sto:ProductionSystemLifeCycle ;
        rdfs:comment       "Classifies standards define data processing, communication, and presentation standards for condition monitoring and diagnostics of machines, for maintaining the adequate performance of the system, and for searching ways to improve performance"@en ;
        rdfs:label         "Production System Maintenance"@en ;
        sto:isDescribedin  sto:NISTInitiative .

sto:FileSizeIEC_61334_1998_P4_S3
        a                      om2:Measure , owl:NamedIndividual ;
        rdfs:comment           "Specifies the file size of the document for standard IEC 61334-4-33:1998 "@en ;
        rdfs:label             "FileSize IEC 61334-4-33:1998"@en ;
        om2:hasNumericalValue  "135.0"^^xsd:float ;
        om2:hasUnit            om2:kilobyte .

dbr:Frankfurt  a  owl:NamedIndividual .

rami:InstanceProduction
        a           owl:NamedIndividual , rami:RAMILifeCycleLayer ;
        rdfs:label  "Instance Production"@en .

dbr:Valbonne  a  owl:NamedIndividual .

sto:IEC_61690_P1_2000
        a                          sto:Standard , owl:NamedIndividual ;
        rdfs:comment               "IEC 61690-1:2000 defines the syntax and semantics for EDIF Version 3 0 0. EDIF Version 3 0 0 addresses EDIF Level 0 and Level 1. EDIF Version 3 0 0 completely addresses the Connectivity and Schematic views, including at Level 1 the ability to represent frames. It includes capabilities formerly found in the Document and Graphics views. A series of releases is planned in the near future to address those views not completely addressed in this version."@en ;
        rdfs:label                 "IEC 61690-1:2000"@en ;
        sto:hasAvailableLanguage   "English"@en , " French"@en ;
        sto:hasEdition             "1.0"^^xsd:float ;
        sto:hasFileSize            sto:FileSizeIEC_61690_P1_2000 ;
        sto:hasICS                 sto:ICS_35_240_50 ;
        sto:hasOfficialResource    <https://webstore.iec.ch/publication/5723> , <null//webstore.iec.ch/publication/5723> ;
        sto:hasPublicationDate     "2000-01-31"^^xsd:date ;
        sto:hasPublisher           sto:IEC ;
        sto:hasStabilityDate       "2018"^^xsd:gYear ;
        sto:hasTag                 "IEC 61690-1:2000"@en ;
        sto:hasTechnicalCommittee  sto:TC_91 ;
        sto:hasTitle               "Electronic design interchange format (EDIF) - Part 1: Version 3 0 0. (This publication is available in electronic HTML format only)"@en .

sto:ISO_14739-1  a               owl:NamedIndividual , sto:Standard ;
        rdfs:comment             "Document management -- 3D use of Product Representation Compact (PRC) format-ISO 14739-1:2014 describes PRC 10001 of a product representation compact (PRC) file format for three dimensional (3D) content data. This format is designed to be included in PDF (ISO 32000) and other similar document formats for the purpose of 3D visualization and exchange. "@en ;
        rdfs:label               "ISO 14739-1"@en ;
        skos:altLabel            "STEP"@en ;
        sto:hasClassification    sto:ProductModelDataExchange ;
        sto:hasDomain            sto:CAD ;
        sto:hasOfficialResource  "https://www.iso.org/standard/54948.html" ;
        sto:hasPublicationDate   "2014-12-01"^^xsd:date ;
        sto:hasPublisher         sto:ISO .

rami:Lifecycle_Status
        a       owl:NamedIndividual .

sto:FileSizeIEC_60870_1990_P5_S1
        a                      om2:Measure , owl:NamedIndividual ;
        rdfs:comment           "Specifies the file size of the document for standard IEC 60870-5-1:1990"@en ;
        rdfs:label             "FileSize IEC 60870-5-1:1990"@en ;
        om2:hasNumericalValue  "2954.0"^^xsd:float ;
        om2:hasUnit            om2:kilobyte .

sto:    a                              owl:Ontology , owl:NamedIndividual , sto:Standard , om2:Measure ;
        rdfs:comment                   "IEC 60038:2009 specifies standard voltage values which are intended to serve as preferential values for the nominal voltage of electrical supply systems, and as reference values for equipment and system design. This seventh edition supersedes the sixth edition (1993), its Amendment 1 (1994) and its Amendment 2 (1997). It constitutes a technical revision. The significant technical changes are: -the addition of the values of 230 V (50 Hz) and 230/400 V (60 Hz) to Table 1;-the replacement of the utilization voltage range at LV by a reference to the relevant standard and an informative annex;- the addition of the value of 30 kV to Table 3;- the replacement of the value of 1 050 kV by 1 100 kV in Table 5. It has the status of a horizontal standard in accordance with IEC Guide 108."@en , "It has the status of a horizontal standard in accordance with IEC Guide 108."@en , "Specifies the file sice of the document for standard IEC_60050-101:1998 "@en ;
        rdfs:label                     "IEC 60050-101:1998"@en , "FileSize IEC_60050-101:1998"@en , "IEC 60038:2009"@en ;
        dc11:description               "An ontology to describe industry standards related to Smart Manufacturing" ;
        dc11:title                     "Standards Ontology"@en ;
        dcterms:created                "2017-01-25"^^xsd:date ;
        dcterms:creator                <http://http://sda.cs.uni-bonn.de/people/irlan-grangel-gonzalez/> , <https://www.linkedin.com/in/paul-baptista-601177b2> , <http://data.semanticweb.org/person/steffen-lohmann> ;
        dcterms:modified               "2017-09-08"^^xsd:date ;
        dcterms:publisher              <http://de.dbpedia.org/resource/Fraunhofer-Gesellschaft> ;
        dcterms:rights                 "This work is distributed under a Creative Commons Attribution License (http://creativecommons.org/licenses/by/3.0/)."@en ;
        vann:preferredNamespacePrefix  "sto" ;
        vann:preferredNamespaceUri     "https://w3id.org/i40/sto#" ;
        doap:repository                <https://github.com/i40-Tools/StandardsOntology> ;
        om2:hasNumericalValue          "1712.0"^^xsd:float , "946.0"^^xsd:float ;
        om2:hasUnit                    om2:kilobyte ;
        owl:imports                    sto: ;
        owl:versionInfo                "0.2" ;
        sto:hasAvailableLanguage       "English/French, Spanish"@en ;
        sto:hasDBpediaResource         <http://dbpedia.org/page/International_Electrotechnical_Vocabulary> , <http://dbpedia.org/page/IEC_60038> ;
        sto:hasEdition                 "7.0"^^xsd:float , "2.0"^^xsd:float ;
        sto:hasFileSize                sto: ;
        sto:hasICS                     sto:ICS_01_040_07 ;
        sto:hasImplementationFormat    "Document"@en ;
        sto:hasOfficialResource        <https://webstore.iec.ch/publication/159> , <https://webstore.iec.ch/publication/153> ;
        sto:hasPages                   129 , 26 ;
        sto:hasPublicationDate         "2009-06-17"^^xsd:date , "1998-04-30"^^xsd:date ;
        sto:hasPublisher               sto:IEC ;
        sto:hasStabilityDate           "2020"^^xsd:gYear ;
        sto:hasStatus                  "Valid"@en ;
        sto:hasTag                     "IEC 60050-101:1998"@en , "IEC 60038:2009"@en ;
        sto:hasTechnicalCommittee      sto:TC_1 , sto:TC_8 ;
        sto:hasTitle                   "IEC standard voltages"@en , "International Electrotechnical Vocabulary - Part 101: Mathematics"@en ;
        sto:hasWikipediaArticle        <https://en.wikipedia.org/wiki/IEC_60038> , <https://en.wikipedia.org/wiki/International_Electrotechnical_Vocabulary> .

sto:hasTechnicalCommittee
        a             owl:ObjectProperty ;
        rdfs:comment  "Specifies the Technical Committe or a Sub-Committee that is responsible for creation and maintenance of a standard"@en ;
        rdfs:domain   sto:Publication ;
        rdfs:label    "has Technical Committee"@en ;
        rdfs:range    sto:TechnicalCommittee .

dbr:_Michigan  a  owl:NamedIndividual .

sto:IEC_42010  a                 owl:NamedIndividual , sto:Standard ;
        rdfs:comment             "ISO/IEC/IEEE 42010:2011 defines requirements on the description of system, software and enterprise architectures. It aims to standardise the practice of architecture description by defining standard terms, presenting a conceptual foundation for expressing, communicating and reviewing architectures and specifying requirements that apply to architecture descriptions, architecture frameworks and architecture description languages."@en ;
        rdfs:label               "IEC 60038:1983+AMD1:1994+AMD2:1997"@en ;
        skos:note                "The IIRA is based in this standards" ;
        sto:hasDBpediaResource   "http://dbpedia.org/page/ISO/IEC_42010" ;
        sto:hasOfficialResource  "http://www.iso-architecture.org/ieee-1471/" ;
        sto:hasPublisher         sto:ISO , sto:IEC ;
        sto:hasTag               "ISO/IEC/IEEE 42010"@en ;
        sto:hasWikipediaArticle  "https://en.wikipedia.org/wiki/ISO/IEC_42010" .

sto:RAMI  a                owl:NamedIndividual ;
        rdfs:comment       "Describes the RAMI model"@en ;
        rdfs:isDefinedBy   "https://www.plattform-i40.de/I40/Redaktion/EN/Downloads/Publikation/structure-of-the-administration-shell.html" ;
        rdfs:label         "RAMI"@en ;
        sto:isDescribedin  rami:InformationLayer .

sto:BBF_TR-069  a                owl:NamedIndividual , sto:Standard ;
        rdfs:comment             "Digital Enhanced Cordless Telecommunications (DECT™) is the ETSI standard for short-range cordless communications, which can be adapted for many applications and can be used over unlicensed frequency allocations world-wide."@en ;
        rdfs:label               "BBF TR-069"@en ;
        sto:hasDBpediaResource   "http://dbpedia.org/resource/TR-069" ;
        sto:hasDeveloper         sto:BBF ;
        sto:hasOfficialResource  "https://www.broadband-forum.org/standards-and-software/technical-specifications/tr-069-files-tools" ;
        sto:hasPublisher         sto:BBF ;
        sto:hasTag               "CPE WAN Management Protocol"@en ;
        sto:hasWikipediaArticle  "https://en.wikipedia.org/wiki/TR-069" .

sto:IEC_60870_P5_S4_1993
        a                          owl:NamedIndividual , sto:Standard ;
        rdfs:comment               "Gives rules for defining information elements and presents a set of information elements, in particular of digital and analog process variables frequently used in telecontrol applications. \nThis publication is of high relevance for Smart Grid."@en ;
        rdfs:label                 "IEC 60870-5-4:1993"@en ;
        sto:hasAvailableLanguage   "English/French"@en ;
        sto:hasDBpediaResource     <null//dbpedia.org/resource/IEC_60870> , <https://dbpedia.org/resource/IEC_60870> ;
        sto:hasEdition             "1.0"^^xsd:float ;
        sto:hasFileSize            sto:FileSizeIEC_60870_P5_S4_1993 ;
        sto:hasICS                 sto:ICS_33_200 ;
        sto:hasOfficialResource    <https://webstore.iec.ch/publication/3749> , <null//webstore.iec.ch/publication/3749> ;
        sto:hasPages               "45"^^xsd:int ;
        sto:hasPublicationDate     "1993-08-218"^^xsd:date ;
        sto:hasPublisher           sto:IEC ;
        sto:hasStabilityDate       "2018"^^xsd:gYear ;
        sto:hasTag                 "IEC 60870-5-4:1993"@en ;
        sto:hasTechnicalCommittee  sto:TC_57 ;
        sto:hasTitle               "Telecontrol equipment and systems - Part 5: Transmission protocols - Section 4: Definition and coding of application information elements"@en ;
        sto:hasWikipediaArticle    <null//en.wikipedia.org/wiki/IEC_60870> , <https://en.wikipedia.org/wiki/IEC_60870> .

sto:ISO_TS_14649-201  a          sto:Standard , owl:NamedIndividual ;
        rdfs:comment             "SO/TS 14649-201:2011 specifies the technology-specific machine tool description data elements needed as process data for manufacturing and machine characteristics. The machine tool descriptions covered in this schema are, initially, milling machines, machining centres, turning machines and multi-tasking machines.ISO/TS 14649-201:2011 is not intended to replace existing machine tool description standards, but to cover the specific needs of manufacturing resource description for manufacturing needs in the technologies described in ISO 14649."@en ;
        rdfs:label               "ISO TS 14649-201"@en ;
        sto:hasClassification    rami:Safety , rami:Engineering , rami:Product , rami:Configuration , rami:Integration , sto:ProductionSystemModelData , rami:Assest ;
        sto:hasDomain            sto:IndustrialAutomation ;
        sto:hasOfficialResource  "https://www.iso.org/standard/60042.html" ;
        sto:hasPublicationDate   "2011-12-01"^^xsd:date ;
        sto:hasPublisher         sto:ISO .

sto:IEC_60870_P5_S1_1990
        a                          owl:NamedIndividual , sto:Standard ;
        rdfs:comment               "Covers asynchronous data transmission with half duplex and duplex link protocols operating with window size one for message transfers. Specifies the basic requirements for services to be provided by the link plus physical layers, for telecontrol applications. In particular it specifies standards on coding, formatting and synchronizing data frames of variable and filed lengths which meet specified data integrity requirements."@en ;
        rdfs:label                 "IEC 60870-5-1:1990"@en ;
        sto:hasAvailableLanguage   "English/French"@en ;
        sto:hasDBpediaResource     <null//dbpedia.org/resource/IEC_60870> , <https://dbpedia.org/resource/IEC_60870> ;
        sto:hasEdition             "1.0"^^xsd:float ;
        sto:hasFileSize            sto:FileSizeIEC_60870_1990_P5_S1 ;
        sto:hasICS                 sto:ICS_33_200 ;
        sto:hasOfficialResource    <https://webstore.iec.ch/publication/3742> , <null//webstore.iec.ch/publication/3742> ;
        sto:hasPages               "79"^^xsd:int ;
        sto:hasPublicationDate     "1990-02-32"^^xsd:date ;
        sto:hasPublisher           sto:IEC ;
        sto:hasStabilityDate       "2018"^^xsd:gYear ;
        sto:hasTag                 "IEC 60870-5-1:1990"@en ;
        sto:hasTechnicalCommittee  sto:TC_57 ;
        sto:hasTitle               "Telecontrol equipment and systems. Part 5: Transmission protocols - Section One: Transmission frame formats"@en ;
        sto:hasWikipediaArticle    <https://en.wikipedia.org/wiki/IEC_60870> , <null//en.wikipedia.org/wiki/IEC_60870> .

sto:IEC_60381_1982  a                sto:Standard , owl:NamedIndividual ;
        rdfs:comment                 "Applicable to analogue direct current signals used in industrial-process measurement and control systems to transmit information between elements of systems. Does not apply to signals used entirely within an element."@en ;
        rdfs:label                   "IEC 60381-1:1982"@en ;
        sto:hasAvailableLanguage     "English/French"@en ;
        sto:hasEdition               "2.0"^^xsd:float ;
        sto:hasFileSize              sto:FileSizeIEC_60381_1982 ;
        sto:hasICS                   sto:ICS_33_200 ;
        sto:hasImplementationFormat  "Document"@en ;
        sto:hasOfficialResource      <https://webstore.iec.ch/publication/1948> ;
        sto:hasPages                 9 ;
        sto:hasPublicationDate       "1982-01-01"^^xsd:date ;
        sto:hasPublisher             sto:IEC ;
        sto:hasStabilityDate         "2018"^^xsd:gYear ;
        sto:hasStatus                "Valid"@en ;
        sto:hasTag                   "IEC 60381-1:1982"@en ;
        sto:hasTechnicalCommittee    sto:TC_40 ;
        sto:hasTitle                 "Analogue signals for process control systems. Part 1: Direct current signals"@en .

sto:FunctionalSafety  a  owl:NamedIndividual , sto:Domain ;
        rdfs:comment  "Functional Safety"@en ;
        rdfs:label    "Functional Safety"@en .

sto:FileSizeIEC_60255_2013
        a                      owl:NamedIndividual , om2:Measure ;
        rdfs:comment           "Specifies the file size of the document for standard IEC 60255-27:2013"@en ;
        rdfs:label             "FileSize IEC 60255-27:2013"@en ;
        om2:hasNumericalValue  "2520.0"^^xsd:float ;
        om2:hasUnit            om2:kilobyte .

sto:ISO_29161  a                 owl:NamedIndividual , sto:Standard ;
        rdfs:comment             "ISO/IEC 29161:2016 establishes a unique identification scheme for the Internet of Things (IoT), based on existing and evolving data structures."@en ;
        rdfs:label               "ISO 29161" ;
        sto:hasOfficialResource  "https://www.iso.org/standard/45240.html" .

sto:TC_44  a          owl:NamedIndividual , sto:TechnicalCommittee ;
        rdfs:comment  "Standardization in the field of the application of electro-technical equipment and systems to machinery (including a group of machines working together in a coordinated manner, excluding higher-level systems aspects) not portable by hand while working, but which may include mobile equipment. The equipment covered commences at the point of connection of the electrical supply to the machinery.Standardization of interfaces (excluding local area networks and fieldbus) between control equipment and the electro-technical equipment of machinery.Standardization of electrotechnical equipment and systems relating to the safeguarding of persons from hazards of the machinery, its associated equipment and the environment.To coordinate with ISO all matters concerning the safety of machinery.."@en , "Standardization in the field of the application of electro-technical equipment and systems to machinery (including a group of machines working together in a coordinated manner, excluding higher-level systems aspects) not portable by hand while working, but which may include mobile equipment. The equipment covered commences at the point of connection of the electrical supply to the machinery.\n\nStandardization of interfaces (excluding local area networks\nand fieldbus) between control equipment and the electro-\ntechnical equipment of machinery.\nStandardization of electrotechnical equipment and systems\nrelating to the safeguarding of persons from hazards of the\nmachinery, its associated equipment and the environment.\nTo coordinate with ISO all matters concerning the safety of\nMachinery."@en ;
        rdfs:label    "TC 44"@en ;
        sto:hasTitle  "Safety of machinery - Electrotechnical aspects"@en .

sto:ISO_18629  a                 owl:NamedIndividual , sto:Standard ;
        rdfs:comment             "ISO 18629-1:2004 provides a general overview of the different series of parts of ISO 18629, which defines a process specification language aimed at identifying, formally defining and structuring the semantic concepts intrinsic to the capture and exchange of process information related to discrete manufacturing."@en ;
        rdfs:label               "ISO 19629"@en ;
        sto:hasClassification    rami:Integration , rami:FieldDevice , rami:Engineering , rami:Functional , rami:Communication , rami:Information , rami:Product , sto:ProductModelDataExchange , rami:ControlDevice , rami:Configuration ;
        sto:hasDomain            sto:IndustrialAutomation ;
        sto:hasOfficialResource  "https://www.iso.org/standard/35431.html" ;
        sto:hasPublicationDate   "2004-11-01"^^xsd:date ;
        sto:hasPublisher         sto:ISO ;
        sto:hasTag               "PSL"@en ;
        sto:hasWikipediaArticle  "https://en.wikipedia.org/wiki/Process_Specification_Language" ;
        sto:relatedTo            sto:ISO_15926 , sto:ISO_ASTM_52915 .

dbr:Eumseong  a  owl:NamedIndividual .

sto:RAMI40  a         owl:NamedIndividual , sto:StandardizationFramework ;
        rdfs:comment  "Describes the Reference Architecture Model for Industry 4.0, i.e., the RAMI Initiative."@en ;
        rdfs:label    "RAMI 4.0"@en .

sto:IEC_60839_P7_4  a              sto:Standard , owl:NamedIndividual ;
        rdfs:comment               "Specifies the transport layer message structure, formats and transmission procedures to be used at standard interfaces in alarm transmission systems. Should be used at all such interfaces where equipment from one supplier is intended to inter-work with equipment from other suppliers, and where the underlying system architecture does not provide the necessary facilities to support the common application layer."@en ;
        rdfs:label                 "IEC 60839-7-4:2001"@en ;
        sto:hasAvailableLanguage   " English/French"@en , "English"@en ;
        sto:hasEdition             "1.0"^^xsd:float ;
        sto:hasFileSize            sto:FileSizeIEC_60839_P7_4 ;
        sto:hasICS                 sto:ICS_13_320 ;
        sto:hasOfficialResource    <null//webstore.iec.ch/publication/3672> ;
        sto:hasPages               "23"^^xsd:int ;
        sto:hasPublicationDate     "68/03/01"^^xsd:date ;
        sto:hasPublisher           sto:IEC ;
        sto:hasStabilityDate       "2018"^^xsd:gYear ;
        sto:hasTag                 "IEC 60839-7-4:2001"@en ;
        sto:hasTechnicalCommittee  sto:TC_79 ;
        sto:hasTitle               "Alarm systems - Part 7-4: Message formats and protocols for serial data interfaces in alarm transmission systems - Common transport layer protocol"@en .

dbr:_California  a  owl:NamedIndividual .

sto:ISO_13485  a                 owl:NamedIndividual , sto:Standard ;
        rdfs:comment             "Medical devices -- Quality management systems -- Requirements for regulatory purposes."@en ;
        rdfs:label               "ISO 13485"@en ;
        sto:hasClassification    rami:Safety ;
        sto:hasDBpediaResource   "http://dbpedia.org/page/ISO_13485" ;
        sto:hasOfficialResource  "https://www.iso.org/iso-9001-quality-management.html" ;
        sto:hasPublisher         sto:ISO .

sto:hasStabilityDate  a  owl:DatatypeProperty ;
        rdfs:comment  "The contents of the publications will remain unchanged up to the Stability date. At this date, the publication will be either reconfirmed, withdrawn, replaced by a revised edition or amended. If there is a revision or amendment on-going then this is mentioned under the publication in the \"Work in progress\" tab, if you don't see this tab it means that there is no project under development."@en ;
        rdfs:domain   sto:Publication ;
        rdfs:label    "has Stability Date"@en ;
        rdfs:range    xsd:gYear ;
        rdfs:seeAlso  <https://webstore.iec.ch/webstore/webstore.nsf/xpFAQ.xsp?Open&id=ADMN-7NALM5> ;
        skos:note     "The data specified is not actually a Date but an Year " .

sto:NISTInitiative  a     owl:NamedIndividual , sto:StandardizationFramework ;
        rdfs:comment      "Describes the National Institute of Standards and Technology Initiative, i.e., NIST which provides a standard landascape"@en ;
        rdfs:isDefinedBy  "http://nvlpubs.nist.gov/nistpubs/ir/2016/NIST.IR.8107.pdf" ;
        rdfs:label        "NIST Initiative"@en .

sto:DIN_SPEC_16592  a            owl:NamedIndividual , sto:Standard ;
        rdfs:comment             "Combining OPC Unified Architecture and Automation Markup Language."@en ;
        rdfs:label               "DIN SPEC 16592"@en ;
        prov:wasGeneratedBy      sto:IEC_62541 , sto:IEC_62714 ;
        sto:hasDeveloper         sto:DIN ;
        sto:hasOfficialResource  <https://www.beuth.de/de/technische-regel/din-spec-16592/265597431> ;
        sto:hasPublisher         sto:DIN .

sto:IEC_61784  a                 sto:Standard , owl:NamedIndividual ;
        rdfs:comment             "Industrial communication networks - Profiles - Ethernet-real-time-enabled"@en ;
        rdfs:label               "IEC 61784"@en ;
        dcterms:hasLicense       "Private"@en ;
        sto:hasClassification    rami:Communication , rami:CommunicationSubModel , rami:ControlDevice , rami:FieldDevice ;
        sto:hasDBpediaResource   "http://dbpedia.org/page/Profibus" ;
        sto:hasMotivation        "Information description and communication mapping for fieldbus profiles"@en ;
        sto:hasOfficialResource  "https://webstore.iec.ch/publication/5878" ;
        sto:hasPublicationDate   "2014-08-19"^^xsd:date ;
        sto:hasPublisher         sto:IEC ;
        sto:hasTag               "IEC Fieldbus (Profibus)"@en ;
        sto:relatedTo            sto:IEC_61158 .

sto:ETSI_DECT  a                 owl:NamedIndividual , sto:Standard ;
        rdfs:comment             "Digital Enhanced Cordless Telecommunications (DECT) is the ETSI standard for short-range cordless communications, which can be adapted for many applications and can be used over unlicensed frequency allocations world-wide."@en ;
        rdfs:label               "ETSI DECT" ;
        sto:hasDBpediaResource   "http://dbpedia.org/resource/Digital_Enhanced_Cordless_Telecommunications" ;
        sto:hasDeveloper         sto:ETSI ;
        sto:hasOfficialResource  "http://www.etsi.org/technologies-clusters/technologies/dect" ;
        sto:hasPublisher         sto:ETSI ;
        sto:hasTag               "Digital Enhanced Cordless Telecommunications"@en ;
        sto:hasWikipediaArticle  "https://en.wikipedia.org/wiki/Digital_Enhanced_Cordless_Telecommunications" .

sto:hasICS  a         owl:ObjectProperty ;
        rdfs:comment  "Serves as a catalogue of International Classification For Standards"@en ;
        rdfs:domain   sto:Publication ;
        rdfs:label    "has ICS"@en ;
        rdfs:range    sto:InternationalClassificationForStandards .

sto:FileSizeIEC_60050_2013
        a                      owl:NamedIndividual , om2:Measure ;
        rdfs:comment           "Specifies the file size of the document for standard IEC 60050-351:2013 "@en ;
        rdfs:label             "FileSize IEC 60050-351:2013"@en ;
        om2:hasNumericalValue  "3999.0"^^xsd:float ;
        om2:hasUnit            om2:kilobyte .

sto:TC_56  a          sto:TechnicalCommittee , owl:NamedIndividual ;
        rdfs:comment  "To prepare international standards in the field of dependability, in all appropriate technological areas, including those not normally dealt with by IEC Technical Committees. Dependability covers the availability performance and its influencing factors: reliability performance, maintainability performance and maintenance support performance (including management of obsolescence). The standards provide systematic methods and tools for the dependability assessment and management of equipment, services and systems throughout their life cycles.\nThe standards cover generic aspects on reliability and maintainability programme management, testing and analytical techniques, software and system dependability, life cycle costing, technical risk analysis and project risk management. This includes standards related to product issues from component reliability to guidance for engineering dependability of systems, standards related to process issues from technological risk analysis to integrated logistics support and standards related to management issues from dependability program management to managing for obsolescence.\nThe application of these standards may raise safety related issues, though the standards themselves do not cover safety. They may be applied to business risk analysis but these risk areas are not dealt with by TC 56."@en ;
        rdfs:label    "TC 56"@en ;
        sto:hasTitle  "Dependability"@en .

dbr:_New_York  a  owl:NamedIndividual .

sto:IEC_60204_2000  a                owl:NamedIndividual , sto:Standard ;
        rdfs:comment                 "Applies to the electrical and electronic equipment and systems of machines, including a group of machines working together in a coordinated manner, but excluding higher level system aspects (i.e. communications between systems)."@en ;
        rdfs:label                   "IEC 60204-11:2000"@en ;
        sto:hasAvailableLanguage     "English/French, Spanish"@en ;
        sto:hasEdition               "1.0"^^xsd:float ;
        sto:hasFileSize              sto:FileSizeIEC_60204_2000 ;
        sto:hasICS                   sto:ICS_13_110 , sto:ICS_29_020 ;
        sto:hasImplementationFormat  "Document"@en ;
        sto:hasOfficialResource      <https://webstore.iec.ch/publication/1022> ;
        sto:hasPages                 111 ;
        sto:hasPublicationDate       "2000-07-31"^^xsd:date ;
        sto:hasPublisher             sto:IEC ;
        sto:hasStabilityDate         "2018"^^xsd:gYear ;
        sto:hasStatus                "Valid"@en ;
        sto:hasTag                   "IEC 60204:2000"@en ;
        sto:hasTechnicalCommittee    sto:TC_44 ;
        sto:hasTitle                 "Safety of machinery - Electrical equipment of machines - Part 11: Requirements for HV equipment for voltages above 1 000 V a.c. or 1 500 V d.c. and not exceeding 36 kV"@en .

foaf:Document  a  owl:Class .

sto:OASIS  a                     sto:StandardOrganization , owl:NamedIndividual ;
        rdfs:comment             "The Organization for the Advancement of Structured Information Standards (OASIS) is a global nonprofit consortium that works on the development, convergence, and adoption of standards for security, Internet of Things, energy, content technologies, emergency management, and other areas."@en ;
        sto:abbreviation         "OASIS" ;
        sto:formationDate        "1993-01-01"^^xsd:date ;
        sto:hasDBpediaResource   "http://dbpedia.org/page/OASIS_(organization)" ;
        sto:hasHeadquaterIn      dbr:Boston ;
        sto:hasOfficialResource  "https://www.oasis-open.org/" ;
        sto:hasWikipediaArticle  "https://en.wikipedia.org/wiki/OASIS_(organization)" ;
        sto:orgName              "Organization for the Advancement of Structured Information Standards"@en .

sto:MathML  a                    owl:NamedIndividual , sto:Standard ;
        rdfs:comment             "MathML is a low-level specification for mathematical and scientific content on the Web and beyond"@en ;
        rdfs:label               "MathML"@en ;
        sto:hasDBpediaResource   "http://dbpedia.org/page/MathML" ;
        sto:hasOfficialResource  "https://www.w3.org/Math/" ;
        sto:hasPublisher         sto:W3C ;
        sto:hasWikipediaArticle  "https://en.wikipedia.org/wiki/MathML" .

sto:hasPages  a       owl:DatatypeProperty ;
        rdfs:comment  "Indicates the number of the pages in the document."@en ;
        rdfs:domain   foaf:Document ;
        rdfs:label    "has Pages"@en ;
        rdfs:range    xsd:integer .

sto:FileSizeIEC_60870_P6_S601_1994
        a                      om2:Measure , owl:NamedIndividual ;
        rdfs:comment           "Specifies the file size of the document for standard IEC 60870-6-601:1994"@en ;
        rdfs:label             "FileSize IEC 60870-6-601:1994"@en ;
        om2:hasNumericalValue  "1112.0"^^xsd:float ;
        om2:hasUnit            om2:kilobyte .

sto:IEC_60904  a                 owl:NamedIndividual , sto:Standard ;
        rdfs:comment             "Photovoltaic devices"@en ;
        rdfs:label               "IEC 60904"@en ;
        sto:hasOfficialResource  "https://webstore.iec.ch/publication/3881" ;
        sto:hasPublicationDate   "2017-05-18"^^xsd:date ;
        sto:hasPublisher         sto:IEC .

sto:IEC_61334_P3_S21_1996
        a                          sto:Standard , owl:NamedIndividual ;
        rdfs:comment               "Establishes definitions, requirements, methods of testing and rated values for phase-to-phase isolated capacitive coupling devices to be used in medium-voltage (MV) distribution line carrier systems.\nThis publication is of high relevance for Smart Grid."@en ;
        rdfs:label                 "IEC 61334-3-21:1996 "@en ;
        sto:hasAvailableLanguage   "English/French"@en ;
        sto:hasDBpediaResource     <null//dbpedia.org/resource/IEC_61334> , <https://dbpedia.org/resource/IEC_61334> ;
        sto:hasEdition             "1.0"^^xsd:float ;
        sto:hasFileSize            sto:FileSizeIEC_61334_1996_P3_S1 ;
        sto:hasICS                 sto:ICS_29_240_20 , sto:ICS_33_200 ;
        sto:hasOfficialResource    <https://webstore.iec.ch/publication/5298> , <null//webstore.iec.ch/publication/5298> ;
        sto:hasPages               "33"^^xsd:int ;
        sto:hasPublicationDate     "1996-03-27"^^xsd:date ;
        sto:hasPublisher           sto:IEC ;
        sto:hasStabilityDate       "2018"^^xsd:gYear ;
        sto:hasTag                 "IEC 61334-3-21:1996 "@en ;
        sto:hasTechnicalCommittee  sto:TC_57 ;
        sto:hasTitle               "Distribution automation using distribution line carrier systems - Part 3: Mains signalling requirements - Section 21: MV phase-to-phase isolated capacitive coupling device"@en ;
        sto:hasWikipediaArticle    <null//en.wikipedia.org/wiki/IEC_61334> , <https://en.wikipedia.org/wiki/IEC_61334> .

rami:GeneralAdminShell
        a       owl:NamedIndividual .

sto:IEC_60870_P6_S802_2014
        a                          owl:NamedIndividual , sto:Standard ;
        rdfs:comment               "IEC 60870-6-802:2014 specifies a method of exchanging time-critical control centre data through wide-area and local-area networks using a full ISO compliant protocol stack. It contains provisions for supporting both centralized and distributed architectures. The standard includes the exchange of real-time data indications, control operations, time series data, scheduling and accounting information, remote program control and event notification. This new edition includes the following significant technical changes with respect to the previous edition:\n- certain objects have been changed from informative to normative;\n- certain TASE.2 conformance blocks have been made out of scope."@en ;
        rdfs:label                 "IEC 60870-6-802:2014"@en ;
        sto:hasAvailableLanguage   "English/French"@en ;
        sto:hasDBpediaResource     <null//dbpedia.org/resource/IEC_60870> , <https://dbpedia.org/resource/IEC_60870> ;
        sto:hasEdition             "3.0"^^xsd:float ;
        sto:hasFileSize            sto:FileSizeIEC_60870_P6_S802_2014 ;
        sto:hasICS                 sto:ICS_33_200 ;
        sto:hasOfficialResource    <null//webstore.iec.ch/publication/3769> , <https://webstore.iec.ch/publication/3769> ;
        sto:hasPages               "188"^^xsd:int ;
        sto:hasPublicationDate     "2014-07-196"^^xsd:date ;
        sto:hasPublisher           sto:IEC ;
        sto:hasStabilityDate       "2019"^^xsd:gYear ;
        sto:hasTag                 "IEC 60870-6-802:2014"@en ;
        sto:hasTechnicalCommittee  sto:TC_57 ;
        sto:hasTitle               "Telecontrol equipment and systems - Part 6-802: Telecontrol protocols compatible with ISO standards and ITU-T recommendations - TASE.2 Object models"@en ;
        sto:hasWikipediaArticle    <https://en.wikipedia.org/wiki/IEC_60870> , <null//en.wikipedia.org/wiki/IEC_60870> .

sto:hasDomain  a      owl:ObjectProperty ;
        rdfs:comment  "Describes the domain, in which the standard is used"@en ;
        rdfs:domain   sto:Publication ;
        rdfs:label    "has Domain"@en ;
        rdfs:range    sto:Domain .

sto:W3C_OWL  a                   sto:Standard , owl:NamedIndividual ;
        rdfs:comment             "The W3C Web Ontology Language (OWL) is a Semantic Web language designed to represent rich and complex knowledge about things, groups of things, and relations between things. OWL is a computational logic-based language such that knowledge expressed in OWL can be exploited by computer programs, e.g., to verify the consistency of that knowledge or to make implicit knowledge explicit. OWL documents, known as ontologies, can be published in the World Wide Web and may refer to or be referred from other OWL ontologies. OWL is part of the W3C’s Semantic Web technology stack, which includes RDF, RDFS, SPARQL, etc."@en ;
        rdfs:label               "Web Ontology Language"@en ;
        dcterms:hasLicense       "Public"@en ;
        sto:hasDBpediaResource   "http://dbpedia.org/resource/Web_Ontology_Language" ;
        sto:hasOfficialResource  "https://www.w3.org/OWL/" ;
        sto:hasPublisher         sto:W3C ;
        sto:hasTag               "OWL"@en ;
        sto:hasWikipediaArticle  "https://en.wikipedia.org/wiki/Web_Ontology_Language?oldformat=true" ;
        sto:relatedTo            sto:W3C_RDF .

sto:StandardPart  a      owl:Class ;
        rdfs:comment     "Typically Standards are divided into parts. E.g., ISA 95 has part Part 1: Models and Terminology, Part 2: Object Model Attributes, etc."@en ;
        rdfs:label       "StandardPart" ;
        rdfs:subClassOf  foaf:Document .

sto:hasHeadquaterIn  a  owl:ObjectProperty ;
        rdfs:comment  "Denotes the countries in which the Headquarter of the organization who publishes the Standart"@en ;
        rdfs:domain   sto:StandardOrganization ;
        rdfs:label    "has Headquater In"@en ;
        rdfs:range    dbo:Place .

sto:ConditionMonitoring
        a                  owl:NamedIndividual , rami:AdminShellSubmodel ;
        sto:isDescribedin  sto:AdministrationShell .

rami:Communication  a      owl:NamedIndividual , rami:RAMIITLayer ;
        sto:isDescribedin  sto:RAMI40 .

sto:UN-CEFACT  a                 owl:NamedIndividual , sto:StandardOrganization ;
        rdfs:comment             "UN/CEFACT is the United Nations Centre for Trade Facilitation and Electronic Business. It was established as an intergovernmental body of the United Nations Economic Commission for Europe (UNECE) in 1996 and evolved from UNECE’s long tradition of work in trade facilitation."@en ;
        sto:abbreviation         "UN/CEFACT" ;
        sto:hasDBpediaResource   "http://dbpedia.org/page/UN/CEFACT" ;
        sto:hasHeadquaterIn      dbr:Geneva ;
        sto:hasOfficialResource  "https://www.unece.org/cefact/" ;
        sto:hasWikipediaArticle  "https://en.wikipedia.org/wiki/UN/CEFACT" ;
        sto:orgName              "United Nations Centre for Trade Facilitation and Electronic Business"@en .

sto:FileSizeIEC_60870_1992_P5_S3
        a                      om2:Measure , owl:NamedIndividual ;
        rdfs:comment           "Specifies the file size of the document for standard IEC 60870-5-3:1992"@en ;
        rdfs:label             "FileSize IEC 60870-5-3:1992"@en ;
        om2:hasNumericalValue  "1629.0"^^xsd:float ;
        om2:hasUnit            om2:kilobyte .

sto:IEC_TS_62832  a              owl:NamedIndividual , sto:Standard ;
        rdfs:comment             "Digital Factory Reference model TS"@en ;
        rdfs:label               "IEC TS 62832"@en ;
        dcterms:hasLicense       "Private"@en ;
        sto:hasClassification    rami:GeneralAdminShell , rami:WorkCenter , rami:ControlDevice , rami:Station , rami:FieldDevice , rami:AdminShellGeneral ;
        sto:hasMotivation        "The standards for Digital Factory define methods and information models, which are required for self description of I40-components. IEC TS 62832 defines methods, which allow to validate or plan connections between assets."@en ;
        sto:hasOfficialResource  "https://webstore.iec.ch/publication/33023" ;
        sto:hasPublisher         sto:IEC ;
        sto:hasTag               "DF/TS"@en .

sto:IEC_60946  a                   sto:Standard , owl:NamedIndividual ;
        rdfs:comment               "Applies to non-multiplexed two wire binary direct voltage signals of nominal 24 V level that are used in industrial-process measurement and control systems to transmit information between elements of systems."@en ;
        rdfs:label                 "IEC 60946:1988�"@en , "IEC 60946:1988"@en ;
        sto:hasAvailableLanguage   "English/French"@en ;
        sto:hasEdition             "1.0"^^xsd:float ;
        sto:hasFileSize            sto:FileSizeIEC_60946 ;
        sto:hasICS                 sto:ICS_25_040_40 ;
        sto:hasOfficialResource    <https://webstore.iec.ch/publication/3961> , <null//webstore.iec.ch/publication/3961> ;
        sto:hasPages               "13"^^xsd:int ;
        sto:hasPublicationDate     "1988-09-273"^^xsd:date ;
        sto:hasPublisher           sto:IEC ;
        sto:hasStabilityDate       "2018"^^xsd:gYear ;
        sto:hasTag                 "IEC 60946:1988"@en , "IEC 60946:1988�"@en ;
        sto:hasTechnicalCommittee  sto:TC_65 ;
        sto:hasTitle               "Binary direct voltage signals for process measurement and control systems"@en .

sto:IEC_61334_P4_S61_1998
        a                          owl:NamedIndividual , sto:Standard ;
        rdfs:comment               "Covers the services required by the data communication protocol (DCP) network layer (N) sublayer entity at the logical interfaces with the N user layer and the LLC sublayer, using the connectionless N procedures.\nThis publication is of high relevance for Smart Grid."@en ;
        rdfs:label                 "IEC 61334-4-61:1998"@en ;
        sto:hasAvailableLanguage   "English/French"@en ;
        sto:hasDBpediaResource     <https://dbpedia.org/resource/IEC_61334> , <null//dbpedia.org/resource/IEC_61334> ;
        sto:hasEdition             "1.0"^^xsd:float ;
        sto:hasFileSize            sto:FileSizeIEC_61334_1998_P4_S61 ;
        sto:hasICS                 sto:ICS_33_200 , sto:ICS_29_240_20 ;
        sto:hasOfficialResource    <https://webstore.iec.ch/publication/5307> , <null//webstore.iec.ch/publication/5307> ;
        sto:hasPages               "63"^^xsd:int ;
        sto:hasPublicationDate     "1998-07-191"^^xsd:date ;
        sto:hasPublisher           sto:IEC ;
        sto:hasStabilityDate       "2018"^^xsd:gYear ;
        sto:hasTag                 "IEC 61334-4-61:1998"@en ;
        sto:hasTechnicalCommittee  sto:TC_57 ;
        sto:hasTitle               "Distribution automation using distribution line carrier systems - Part 4-61: Data communication protocols - Network layer - Connectionless protocol"@en ;
        sto:hasWikipediaArticle    <https://en.wikipedia.org/wiki/IEC_61334> , <null//en.wikipedia.org/wiki/IEC_61334> .

sto:IEC_61334_P3_S1_1998
        a                          owl:NamedIndividual , sto:Standard ;
        rdfs:comment               "Applies to electrical equipment used in distribution line carrier systems on both medium-voltage and low-voltage distribution networks. Specifies requirements such as frequency bands, output levels, spurious emissions, etc.\nThis publication is of high relevance for Smart Grid."@en ;
        rdfs:label                 "IEC 61334-3-1:1998 "@en ;
        sto:hasAvailableLanguage   "English/French"@en ;
        sto:hasDBpediaResource     <https://dbpedia.org/resource/IEC_61334> , <null//dbpedia.org/resource/IEC_61334> ;
        sto:hasEdition             "1.0"^^xsd:float ;
        sto:hasFileSize            sto:FileSizeIEC_61334_1998_P3_S1 ;
        sto:hasICS                 sto:ICS_29_240_20 , sto:ICS_33_200 ;
        sto:hasOfficialResource    <null//webstore.iec.ch/publication/5297> , <https://webstore.iec.ch/publication/5297> ;
        sto:hasPages               "27"^^xsd:int ;
        sto:hasPublicationDate     "1998-11-328"^^xsd:date ;
        sto:hasPublisher           sto:IEC ;
        sto:hasStabilityDate       "2018"^^xsd:gYear ;
        sto:hasTag                 "IEC 61334-3-1:1998 "@en ;
        sto:hasTechnicalCommittee  sto:TC_57 ;
        sto:hasTitle               "Distribution automation using distribution line carrier systems - Part 3-1: Mains signalling requirements - Frequency bands and output levels"@en ;
        sto:hasWikipediaArticle    <null//en.wikipedia.org/wiki/IEC_61334> , <https://en.wikipedia.org/wiki/IEC_61334> .

sto:IIRA  a                      owl:NamedIndividual , sto:StandardizationFramework ;
        rdfs:comment             "Industrial Internet Reference Architecture"@en ;
        rdfs:label               "IIRA"@en ;
        sto:hasOfficialResource  "http://www.iiconsortium.org/IIRA.htm" .

sto:W3C_RDF  a                   sto:Standard , owl:NamedIndividual ;
        rdfs:comment             "RDF is a standard model for data interchange on the Web. RDF has features that facilitate data merging even if the underlying schemas differ, and it specifically supports the evolution of schemas over time without requiring all the data consumers to be changed. "@en ;
        rdfs:label               "Resource Description Framework"@en ;
        dcterms:hasLicense       "Public"@en ;
        sto:hasDBpediaResource   "http://dbpedia.org/resource/Resource_Description_Framework" ;
        sto:hasOfficialResource  "https://www.w3.org/RDF/" ;
        sto:hasPublisher         sto:W3C ;
        sto:hasTag               "RDF"@en ;
        sto:hasWikipediaArticle  "https://en.wikipedia.org/wiki/Resource_Description_Framework" .

sto:ISO_15531-2x  a        owl:NamedIndividual , sto:StandardPart ;
        rdfs:comment       "Production data for external exchanges. refering to the representation of product information to be exchanged with the external environment (customers and suppliers), with the aim to model the main production information exchanged between industrial companies, in order to improve exchanges and integration through the use of EDI protocols."@en ;
        rdfs:isDefinedBy   "https://www.researchgate.net/publication/220171079_ISO_15531_MANDATE_a_standardised_data_model_for_manufacturing_management" ;
        rdfs:label         "ISO 15531 2x series"@en ;
        dul:isComponentOf  sto:ISO_15531 .

sto:FileSizeIEC_60848
        a                      om2:Measure , owl:NamedIndividual ;
        rdfs:comment           "Specifies the file size of the document for standard IEC 60848:2013"@en ;
        rdfs:label             "FileSize IEC 60848:2013"@en ;
        om2:hasNumericalValue  "1784.0"^^xsd:float ;
        om2:hasUnit            om2:kilobyte .

sto:Product  a  owl:NamedIndividual .

sto:APICS  a                     sto:StandardOrganization , owl:NamedIndividual ;
        rdfs:comment             "American Production and Inventory Control Society."@en ;
        rdfs:label               "APICS"@en ;
        sto:formationDate        "1957-01-01"^^xsd:date ;
        sto:hasDBpediaResource   <http://dbpedia.org/page/APICS> ;
        sto:hasHeadquaterIn      dbr:Chicago ;
        sto:hasOfficialResource  <http://www.apics.org/apics> ;
        sto:hasWikipediaArticle  <https://en.wikipedia.org/wiki/APICS> ;
        sto:orgName              "American Production and Inventory Control Society"@en .

sto:IEC_60870_P5_S102_1996
        a                          owl:NamedIndividual , sto:Standard ;
        rdfs:comment               "Standardizes the transmission of integrated totals representing the amount of electrical energy transferred between power utilities, or between a power utility and independent producers on a high voltage or medium voltage network.\nThis publication is of high relevance for Smart Grid."@en ;
        rdfs:label                 "IEC 60870-5-102:1996"@en ;
        sto:hasAvailableLanguage   "English/French"@en ;
        sto:hasDBpediaResource     <https://dbpedia.org/resource/IEC_60870> , <null//dbpedia.org/resource/IEC_60870> ;
        sto:hasEdition             "1.0"^^xsd:float ;
        sto:hasFileSize            sto:FileSizeIEC_60870_P5_S102_1996 ;
        sto:hasICS                 sto:ICS_33_200 ;
        sto:hasOfficialResource    <https://webstore.iec.ch/publication/3744> , <null//webstore.iec.ch/publication/3744> ;
        sto:hasPages               "99"^^xsd:int ;
        sto:hasPublicationDate     "1996-06-170"^^xsd:date ;
        sto:hasPublisher           sto:IEC ;
        sto:hasStabilityDate       "2018"^^xsd:gYear ;
        sto:hasTag                 "IEC 60870-5-102:1996"@en ;
        sto:hasTechnicalCommittee  sto:TC_57 ;
        sto:hasTitle               "Telecontrol equipment and systems - Part 5: Transmission protocols - Section 102: Companion standard for the transmission of integrated totals in electric power systems"@en ;
        sto:hasWikipediaArticle    <null//en.wikipedia.org/wiki/IEC_60870> , <https://en.wikipedia.org/wiki/IEC_60870> .

rami:Configuration  a  owl:NamedIndividual .

rami:ConditionMonitoring
        a       owl:NamedIndividual .

sto:ISO  a                       sto:StandardOrganization , owl:NamedIndividual ;
        rdfs:comment             "The International Organization for Standardization (ISO) is an international standard-setting body composed of representatives from various national standards organizations."@en , "Is an independent, non-governmental organization, the members of which are the standards organizations of the 162 member countries. It is the world's largest developer of voluntary international standards and facilitates world trade by providing common standards between nations. Nearly twenty thousand standards have been set covering everything from manufactured products and technology to food safety, agriculture and healthcare."@en ;
        sto:abbreviation         "ISO" ;
        sto:belongsTo            dbr:Switzerland ;
        sto:formationDate        "1947-02-23"^^xsd:date ;
        sto:hasDBpediaResource   <http://dbpedia.org/page/International_Organization_for_Standardization> ;
        sto:hasHeadquaterIn      dbr:Geneva ;
        sto:hasOfficialResource  <https://www.iso.org/about-us.html> , <https://www.iso.org> ;
        sto:hasWikipediaArticle  <https://en.wikipedia.org/wiki/International_Organization_for_Standardization> ;
        sto:orgName              "Internationale Organisation für Normung"@de , "The International Organization for Standardization"@en , "Международная организация по стандартизации"@ru , "Organisation internationale de normalisation"@fr , "International Organization for Standardization"@en .

sto:OMG  a                       owl:NamedIndividual , sto:StandardOrganization ;
        rdfs:comment             "The Object Management Group (OMG) is an international, open membership, not-for-profit technology standards consortium. OMG Task Forces develop enterprise integration standards for a wide range of technologies and industries. OMG modeling standards enable visual design, execution and maintenance of software and other processes. Originally aimed at standardizing distributed object-oriented systems, the company now focuses on modeling (programs, systems and business processes) and model-based standards." ;
        sto:abbreviation         "OMG" ;
        sto:formationDate        "1989-01-01"^^xsd:date ;
        sto:hasDBpediaResource   "http://dbpedia.org/resource/Object_Management_Group" ;
        sto:hasHeadquaterIn      dbr:_Massachusetts ;
        sto:hasOfficialResource  "http://www.omg.org/" ;
        sto:hasWikipediaArticle  "https://en.wikipedia.org/wiki/Object_Management_Group" ;
        sto:orgName              "Object Management Group"@en .

sto:IEC_TR_62794  a              owl:NamedIndividual , sto:Standard ;
        rdfs:comment             "Industrial-process measurement, control and automation - Reference model for representation of production facilities (digital factory)"@en ;
        rdfs:label               "IEC TR 62794"@en ;
        dcterms:hasLicense       "Private"@en ;
        sto:hasClassification    rami:Station , rami:WorkCenter , rami:FieldDevice , rami:AdminShellGeneral , rami:GeneralAdminShell , rami:ControlDevice ;
        sto:hasMotivation        "The standards for Digital Factory define methods and information models, which are required for self description of I40-components. "@en ;
        sto:hasOfficialResource  <https://webstore.iec.ch/publication/7433> ;
        sto:hasPublisher         sto:IEC ;
        sto:hasTag               "DF/TR"@en ;
        sto:relatedTo            sto:IEC_TS_62832 .

sto:FileSizeIEC_61334_1996_P4_S1
        a                      om2:Measure , owl:NamedIndividual ;
        rdfs:comment           "Specifies the file size of the document for standard IEC 61334-4-1:1996"@en ;
        rdfs:label             "FileSize IEC 61334-3-22:2000"@en ;
        om2:hasNumericalValue  "1707.0"^^xsd:float ;
        om2:hasUnit            om2:kilobyte .

sto:IEC_60286_3_2013  a              sto:Standard , owl:NamedIndividual ;
        rdfs:comment                 "IEC 60286-3:2013 is applicable to the tape packaging of electronic components without leads or with lead stumps, intended to be connected to electronic circuits. It includes only those dimensions that are essential for the taping of components intended for the above-mentioned purposes. This standard also includes requirements related to the packaging of singulated die products including bare die and bumped die (flip chips). This fifth edition cancels and replaces the fourth edition, published in 2007, as well as IEC 60286-3-1, published in 2009 and IEC 60286-3-2, published in 2009. It constitutes a full layout revision. In addition, this edition includes the following significant technical changes with respect to the previous edition:a) IEC 60286-3:2013 is applicable to the tape packaging of electronic components without leads or with lead stumps, intended to be connected to electronic circuits. It includes only those dimensions that are essential for the taping of components intended for the above-mentioned purposes. This standard also includes requirements related to the packaging of singulated die products including bare die and bumped die (flip chips). This fifth edition cancels and replaces the fourth edition, published in 2007, as well as IEC 60286-3-1, published in 2009 and IEC 60286-3-2, published in 2009.It constitutes a full layout revision. In addition, this edition includes the following significant technical changes with respect to the previous edition:a) integration of IEC 60286-3-1:2009 as type 1b (Packaging of surface mount components on continuous pressed carrier tapes);b) integration of IEC 60286-3-2:2009 as type 2b (Packaging of surface mount components on blister carrier tapes 4 mm in width).ntegration of IEC 60286-3-1:2009 as type 1b (Packaging of surface mount components on continuous pressed carrier tapes);b) integration of IEC 60286-3-2:2009 as type 2b (Packaging of surface mount components on blister carrier tapes 4 mm in width)."@en ;
        rdfs:label                   "IEC 60286-3:2013"@en ;
        sto:hasAvailableLanguage     "English/French"@en ;
        sto:hasEdition               "5.0"^^xsd:float ;
        sto:hasFileSize              sto:FileSizeIEC_60286_3_2013 ;
        sto:hasICS                   sto:ICS_31_020 , sto:ICS_31_240 ;
        sto:hasImplementationFormat  "Document"@en ;
        sto:hasOfficialResource      <https://webstore.iec.ch/publication/1258> ;
        sto:hasPages                 77 ;
        sto:hasPublicationDate       "2013-05-17"^^xsd:date ;
        sto:hasPublisher             sto:IEC ;
        sto:hasStabilityDate         "2024"^^xsd:gYear ;
        sto:hasStatus                "Valid"@en ;
        sto:hasTag                   "IEC 60286-3:2013"@en ;
        sto:hasTechnicalCommittee    sto:TC_40 ;
        sto:hasTitle                 "Packaging of components for automatic handling - Part 3: Packaging of surface mount components on continuous tapes"@en .

sto:IEC_61010_P2_S012_2016
        a                          sto:Standard , owl:NamedIndividual ;
        rdfs:comment               "IEC 61010-2-012:2016 specifies safety requirements for electrical equipment and their accessories within the categories a) through c), wherever they are intended to be used, whenever that equipment incorporates one or more of the following characteristics:\n- A REFRIGERATING SYSTEM that is acted on or impacted by an integral heating function such that the combined heating and cooling system generates additional and/or more severe HAZARDS than those for the two systems if treated separately.\n- The materials being treated in the intended application introduce significant heat into the REFRIGERATING SYSTEM that the cooling system in the application yield additional and/or more severe HAZARDS than those for the cooling system if operated at the maximum RATED ambient alone.\n- An irradiation function for the materials being treated presenting additional HAZARDS.\n- A function to expose the materials being treated to excessive humidity, carbon dioxide, salt mist, or other substances which may result in additional HAZARDS.\n- A function of MECHANICAL MOVEMENT presenting additional HAZARDS.\n- Provision for an OPERATOR to walk-in to the operating area to load or unload the materials being treated.\nIt has the status of a group safety publication in accordance with IEC Guide 104.\nThis publication is to be read in conjunction with IEC 61010-1:2010."@en ;
        rdfs:label                 "IEC 61010-2-012:2016"@en ;
        sto:hasAvailableLanguage   "English/French"@en ;
        sto:hasEdition             "1.0"^^xsd:float ;
        sto:hasFileSize            sto:FileSizeIEC_61010_P2_S012_2016 ;
        sto:hasICS                 sto:ICS_19_08 ;
        sto:hasOfficialResource    <null//webstore.iec.ch/publication/25400> , <https://webstore.iec.ch/publication/25400> ;
        sto:hasPages               "174"^^xsd:int ;
        sto:hasPublicationDate     "2016-07-194"^^xsd:date ;
        sto:hasPublisher           sto:IEC ;
        sto:hasStabilityDate       "2020"^^xsd:gYear ;
        sto:hasTag                 "IEC 61010-2-012:2016"@en ;
        sto:hasTechnicalCommittee  sto:TC_66 ;
        sto:hasTitle               "Safety requirements for electrical equipment for measurement, control, and laboratory use - Part 2-012: Particular requirements for climatic and environmental testing and other temperature conditioning equipment"@en .

sto:IEC_61334_P5_S1_2001
        a                          owl:NamedIndividual , sto:Standard ;
        rdfs:comment               "Describes the requirements of S-FSK (frequency shift keying modulation) in conjunction with the services provided by the physical layer entity and the MAC sublayer. The transmission medium is assumed to be the distribution network on both MV or LV level. To be used in conjunction with IEC 61334-4-32.\nThis publication is of high relevance for Smart Grid."@en ;
        rdfs:label                 "IEC 61334-5-1:2001"@en ;
        sto:hasAvailableLanguage   "English/French"@en ;
        sto:hasDBpediaResource     <https://dbpedia.org/resource/IEC_61334> , <null//dbpedia.org/resource/IEC_61334> ;
        sto:hasEdition             "2.0"^^xsd:float ;
        sto:hasFileSize            sto:FileSizeIEC_61334_2001_P5_S1 ;
        sto:hasICS                 sto:ICS_33_200 ;
        sto:hasOfficialResource    <https://webstore.iec.ch/publication/5308> , <null//webstore.iec.ch/publication/5308> ;
        sto:hasPages               "123"^^xsd:int ;
        sto:hasPublicationDate     "2001-05-148"^^xsd:date ;
        sto:hasPublisher           sto:IEC ;
        sto:hasStabilityDate       "2018"^^xsd:gYear ;
        sto:hasTag                 "IEC 61334-5-1:2001"@en ;
        sto:hasTechnicalCommittee  sto:TC_57 ;
        sto:hasTitle               "Distribution automation using distribution line carrier systems - Part 5-1: Lower layer profiles - The spread frequency shift keying (S-FSK) profile"@en ;
        sto:hasWikipediaArticle    <https://en.wikipedia.org/wiki/IEC_61334> , <null//en.wikipedia.org/wiki/IEC_61334> .

sto:IndustrialAutomation
        a                        owl:NamedIndividual , sto:Domain ;
        rdfs:comment             "Industrial automation deals primarily with the automation of manufacturing, quality control and material handling processes. General purpose controllers for industrial processes include Programmable logic controllers, stand-alone I/O modules, and computers. Industrial automation is to replace the decision making of humans and manual command-response activities with the use of mechanized equipment and logical programming commands. One trend is increased use of Machine vision to provide automatic inspection and robot guidance functions, another is a continuing increase in the use of robots. Industrial automation is simply done at the industrial level."@en ;
        sto:domainName           "Industrial Automation"@en ;
        sto:hasDBpediaResource   "http://dbpedia.org/resource/Category:IndustrialAutomation" ;
        sto:hasWikipediaArticle  "https://en.wikipedia.org/wiki/Automation" .

sto:stoPartName  a    owl:DatatypeProperty ;
        rdfs:comment  "Name of the standard part."@en ;
        rdfs:domain   sto:StandardPart ;
        rdfs:label    "std Part Name"@en ;
        rdfs:range    xsd:string .

sto:FileSizeIEC_60839_P7_6
        a                      om2:Measure , owl:NamedIndividual ;
        rdfs:comment           "Specifies the file size of the document for standard IEC 60839-7-6:2001"@en ;
        rdfs:label             "FileSize IEC 60839-7-6:2001"@en ;
        om2:hasNumericalValue  "926.0"^^xsd:float ;
        om2:hasUnit            om2:kilobyte .

sto:FileSizeIEC_60864_P1
        a                      om2:Measure , owl:NamedIndividual ;
        rdfs:comment           "Specifies the file size of the document for standard IEC 60864-1:1986 "@en ;
        rdfs:label             "FileSizeIEC 60864-1:1986"@en ;
        om2:hasNumericalValue  "1540.0"^^xsd:float ;
        om2:hasUnit            om2:kilobyte .

sto:SE  a                        sto:StandardOrganization , owl:NamedIndividual ;
        rdfs:comment             "The Broadband Forum is a non-profit industry consortium dedicated to developing broadband network specifications. Members include telecommunications networking and service provider companies, broadband device and equipment vendors, consultants and independent testing labs (ITLs). Service provider members are primarily wire-line service providers (non-mobile) telephone companies."@en ;
        sto:abbreviation         "SE" ;
        sto:formationDate        "1936-01-01"^^xsd:date ;
        sto:hasDBpediaResource   "http://dbpedia.org/page/Schneider_Electric" ;
        sto:hasHeadquaterIn      dbr:Paris ;
        sto:hasOfficialResource  "http://www.schneider-electric.com/ww/en/" ;
        sto:hasWikipediaArticle  "https://en.wikipedia.org/wiki/Schneider_Electric" ;
        sto:orgName              "Schneider Electric"@en .

sto:IEC_61334_P3_S22_2001
        a                          sto:Standard , owl:NamedIndividual ;
        rdfs:comment               "Establishes definitions, requirements, methods of testing and rated values for phase-to-earth capacitive and screen-to-earth intrusive inductive coupling devices to be used in medium voltage DLC systems.\nThis publication is of high relevance for Smart Grid."@en ;
        rdfs:label                 "IEC 61334-3-22:2001�"@en ;
        sto:hasAvailableLanguage   "English/French"@en ;
        sto:hasDBpediaResource     <https://dbpedia.org/resource/IEC_61334> , <null//dbpedia.org/resource/IEC_61334> ;
        sto:hasEdition             "1.0"^^xsd:float ;
        sto:hasFileSize            sto:FileSizeIEC_61334_1996_P3_S22 ;
        sto:hasICS                 sto:ICS_29_240_20 , sto:ICS_33_200 ;
        sto:hasOfficialResource    <https://webstore.iec.ch/publication/5299> , <null//webstore.iec.ch/publication/5299> ;
        sto:hasPages               "35"^^xsd:int ;
        sto:hasPublicationDate     "2001-01-12"^^xsd:date ;
        sto:hasPublisher           sto:IEC ;
        sto:hasStabilityDate       "2018"^^xsd:gYear ;
        sto:hasTag                 "IEC 61334-3-22:2001 "@en ;
        sto:hasTechnicalCommittee  sto:TC_57 ;
        sto:hasTitle               "Distribution automation using distribution line carrier systems - Part 3-22: Mains signalling requirements - MV phase-to-earth and screen-to-earth intrusive coupling devices"@en ;
        sto:hasWikipediaArticle    <null//en.wikipedia.org/wiki/IEC_61334> , <https://en.wikipedia.org/wiki/IEC_61334> .

sto:M2M  a                       owl:NamedIndividual , sto:Domain ;
        rdfs:comment             "Machine to machine refers to direct communication between devices using any communications channel, including wired and wireless"@en ;
        sto:domainName           "Machine to machine Communication"@en ;
        sto:hasDBpediaResource   "http://dbpedia.org/resource/Machine_to_machine" ;
        sto:hasWikipediaArticle  "https://en.wikipedia.org/wiki/Machine_to_machine" .

sto:ISO_18828-2  a               owl:NamedIndividual , sto:Standard ;
        rdfs:comment             "Industrial automation systems and integration -- Standardized procedures for production systems engineering."@en ;
        rdfs:label               "ISO 18828-2"@en ;
        sto:hasClassification    rami:Enterprise , rami:Engineering , rami:ControlDevice , rami:FieldDevice , sto:Prodcut , rami:WorkCenter , rami:Station ;
        sto:hasDomain            sto:IndustrialAutomation ;
        sto:hasOfficialResource  "https://www.iso.org/standard/63505.html" ;
        sto:hasPublicationDate   "2016-10-01"^^xsd:date ;
        sto:hasPublisher         sto:ISO ;
        sto:relatedTo            sto:IEC_61804 .

dcterms:modified  a  owl:AnnotationProperty .

sto:StandardOrganization
        a                owl:Class ;
        rdfs:comment     "Define the standards organizations that develop and publish industry standards"@en ;
        rdfs:label       "StandardOrganization"@en ;
        rdfs:subClassOf  foaf:Organization .

dbr:China  a    owl:NamedIndividual .

sto:ICS_17_020  a     sto:InternationalClassificationForStandards , owl:NamedIndividual ;
        rdfs:comment  "This is ICS for “Metrology and measurement in general ”"@en ;
        rdfs:label    "ICS 17.020"@en ;
        sto:hasTitle  "Metrology and measurement in general "@en .

sto:ebXML  a                     sto:Standard , owl:NamedIndividual ;
        rdfs:comment             "Electronic Business using eXtensible Markup Language, commonly known as e-business XML, or ebXML is a family of XML based standards whose mission is to provide an open, XML-based infrastructure that enables the global use of electronic business information in an interoperable, secure, and consistent manner by all trading partners."@en ;
        rdfs:label               "ebXML"@en ;
        sto:hasClassification    sto:BusinessProcessExecution ;
        sto:hasDBpediaResource   "http://dbpedia.org/resource/EbXML" ;
        sto:hasOfficialResource  "https://webstore.iec.ch/publication/24433" ;
        sto:hasPublisher         sto:UN-CEFACT , sto:OASIS ;
        sto:hasTag               "ebXML"@en ;
        sto:hasWikipediaArticle  "https://en.wikipedia.org/wiki/EbXML" .

sto:ProductLifeCycleManagement
        a                  owl:NamedIndividual , sto:ProductDevelopmentLifeCycle ;
        rdfs:comment       "Product lifecycle data management focuses on the needs of long-term retention and access to data consistently throughout the product lifecycle."@en ;
        rdfs:label         "Production Life Cycle Management"@en ;
        sto:isDescribedin  sto:NISTInitiative .

sto:IEC_14443  a                 owl:NamedIndividual , sto:Standard ;
        rdfs:comment             "The ISO/IEC 14443 standard is a four-part international standard for contact-less smart cards operating at 13.56 MHz in close proximity (~10cm) with a reader antenna. This ISO standard describes the modulation and transmission protocols between card and reader to create interoperability for contact-less smart card products. There are two main communication protocols supported by the ISO/IEC 14443 standard, they are addressed as Type A and Type B. Most High Frequency (13.56 MHz) proximity tags are using these guidelines for their communication."@en ;
        rdfs:label               "ISO/IEC 14443"@en ;
        owl:sameAs               sto:ISO_14443 ;
        sto:hasDBpediaResource   "http://dbpedia.org/resource/ISO/IEC_14443" ;
        sto:hasOfficialResource  "https://www.iso.org/standard/70170.html" ;
        sto:hasPublisher         sto:IEC , sto:ISO ;
        sto:hasTag               "IEC 14443"@en ;
        sto:hasWikipediaArticle  "https://en.wikipedia.org/wiki/ISO/IEC_14443" .

sto:ISO_14306  a                 owl:NamedIndividual , sto:Standard ;
        rdfs:comment             "It provides the description of the structure and content for a binary file having the extension of .jt. A binary file with the .jt extension is generally referred to as a JT file. The JT format described in ISO 14306:2012 is used primarily in industrial use cases as the means for capturing and repurposing lightweight 3D product definition data"@en ;
        rdfs:label               "ISO 14306"@en ;
        sto:hasClassification    rami:Identification , rami:Product , sto:ProductionSystemModelData , rami:Asset , sto:ProcessPlanning , rami:Engineering ;
        sto:hasDomain            sto:CAD ;
        sto:hasOfficialResource  "https://www.iso.org/standard/60572.html" ;
        sto:hasPublicationDate   "2017-07-01"^^xsd:date ;
        sto:hasPublisher         sto:ISO ;
        sto:relatedTo            sto:IEC_62541 .

sto:IEC_62424  a                 owl:NamedIndividual , sto:Standard ;
        rdfs:comment             "CAEX (Computer Aided Engineering Exchange) is a neutral data format that allows storage of hierarchical object information, e.g. the hierarchical architecture of a plant. On a certain abstraction level, a plant consists in modules or components that are interconnected. CAEX allows storage of those modules or components by means of objects. Object oriented concepts as encapsulation, classes, class libraries, instances, instance hierarchies, inheritance, relations, attributes and interfaces are explicitly supported. CAEX bases on XML and is defined as XML schema (xsd file). The original intention of developing CAEX was the industrial lack of a common and established data exchange between process engineering tools and process control engineering tools. However, CAEX can be applied to all types of static object information, e.g. plant topologies, document topologies, product topologies, petri nets, but also for non-technical applications like phylogenetic trees."@en ;
        rdfs:label               "IEC 62424"@en ;
        dcterms:hasLicense       "Private"@en ;
        dul:isComponentOf        sto:IEC_62714 ;
        sto:hasDBpediaResource   "http://dbpedia.org/resource/CAEX" ;
        sto:hasOfficialResource  "https://webstore.iec.ch/publication/25442" ;
        sto:hasPublisher         sto:IEC ;
        sto:hasTag               "CAEX"@en ;
        sto:hasWikipediaArticle  "https://en.wikipedia.org/wiki/CAEX" .

sto:ICS_33_100_20  a  sto:InternationalClassificationForStandards , owl:NamedIndividual ;
        rdfs:comment  "This is ICS for “Immunity”"@en ;
        rdfs:label    "ICS 33.100.20"@en ;
        sto:hasTitle  "Immunity"@en .

dcterms:hasVersion  a  owl:AnnotationProperty .

sto:BBF  a                       sto:StandardOrganization , owl:NamedIndividual ;
        rdfs:comment             "The Broadband Forum is a non-profit industry consortium dedicated to developing broadband network specifications. Members include telecommunications networking and service provider companies, broadband device and equipment vendors, consultants and independent testing labs (ITLs). Service provider members are primarily wire-line service providers (non-mobile) telephone companies."@en ;
        rdfs:label               "Broadband Forum"@en ;
        sto:abbreviation         "BBF" ;
        sto:formationDate        "2008-01-01"^^xsd:date ;
        sto:hasDBpediaResource   "http://dbpedia.org/resource/Broadband_Forum" ;
        sto:hasHeadquaterIn      dbr:_California ;
        sto:hasOfficialResource  "https://www.broadband-forum.org/" ;
        sto:hasWikipediaArticle  "https://en.wikipedia.org/wiki/Broadband_Forum" ;
        sto:orgName              "Broadband Forum"@en .

sto:OAGIS  a                     owl:NamedIndividual , sto:Standard ;
        rdfs:comment             "The Open Applications Group Integration Specification (OAGIS) is an effort to provide a canonical business language for information integration. It uses XML as the common alphabet for defining business messages, and for identifying business processes (scenarios) that allow businesses and business applications to communicate."@en ;
        rdfs:label               "OAGIS"@en ;
        sto:hasOfficialResource  "http://www.oagi.org/dnn2/DownloadsandResources/OAGIS100PublicDownload.aspx" ;
        sto:hasPublisher         sto:OAGi ;
        sto:hasTag               "Open Applications Group Integration Specification"@en ;
        sto:hasWikipediaArticle  "https://de.wikipedia.org/wiki/Open_Application_Group_Integration_Specification" .

sto:eClassAssoc  a               sto:StandardOrganization , owl:NamedIndividual ;
        rdfs:comment             "Der eCl@ss e. V. ist eine Non-Profit-Organisation, die den gleichnamigen Klassifikationsstandard branchenübergreifend international definiert, weiterentwickelt und verbreitet. Der Verein wird getragen von ordentlichen und fördernden Mitgliedern aus Unternehmen, Verbänden und Institutionen."@de ;
        sto:abbreviation         "eClass" , "eCl@ss" ;
        sto:formationDate        "2000-11-14"^^xsd:date ;
        sto:hasHeadquaterIn      dbr:Cologne ;
        sto:hasOfficialResource  "https://www.eclass.eu" ;
        sto:hasWikipediaArticle  "https://www.wikiwand.com/de/ECl@ss" ;
        sto:orgName              "eCl@ss e. V."@de .
